`example_user`
[PROOF STATE]
x y : ℝ
h1: x = 3 - 2 * y
h2: 2 * (3 - 2 * y) - y = 1
⊢
y = 1

[LAST TACTIC]
rw [h2] at h1
[FAILED]
[ERROR MESSAGE]
error: tactic 'rewrite' failed, did not find instance of the pattern in the target expression
  2 * (3 - 2 * y) - y

[INSTRUCTIONS]
Please write the next tactic now.

`example_assistant`
[START TACTIC]
linarith
[END TACTIC]

`example_user`
[PROOF STATE]
n : ℕ
h0 : n < 398
h1 : (n * 7) % 398 = 1
⊢
n = 57

[LAST TACTIC]
norm_num
[FAILED]
[ERROR MESSAGE]
error: unsolved goals

[INSTRUCTIONS]
Please write the next tactic now.

`example_assistant`
[START TACTIC]
have h2 : 1 % 398 = (57 * 7) % 398 := by norm_num
[END TACTIC]

`example_user`
[PROOF STATE]
s : ℕ → ℝ
h0: ∀ n, s (n + 2) = s (n + 1) + s n
h1 : s 9 = 110
h2 : s 7 = 42
h : ∀ (n : ℕ), s n = s (n + 2) - s (n + 1)
h3 : s 9 = s 8 + s 7
h4 : s 8 = 68
⊢
s 5 = 16

[LAST TACTIC]
linarith
[FAILED]
[ERROR MESSAGE]
error: linarith failed to find a contradiction

[INSTRUCTIONS]
Please write the next tactic now.

`example_assistant`
[START TACTIC]
rw [(h 5)]
[END TACTIC]

`example_user`
[PROOF STATE]
d : ℕ
ih : 3 ∣ d ^ 3 + 2 * d
ih_expanded : (d + 1) ^ 3 + 2 * (d + 1) = d ^ 3 + 3 * d ^ 2 + 5 * d + 3
ih_factored : d ^ 3 + 3 * d ^ 2 + 5 * d + 3 = d ^ 3 + 2 * d + 3 * (d ^ 2 + d + 1)
⊢
3 ∣ d ^ 3 + 2 * d + 3 * (d ^ 2 + d + 1)

[LAST TACTIC]
rw [ih_factored]
[STATE CHANGED]

[INSTRUCTIONS]
Please write the next tactic now.

`example_assistant`
[START TACTIC]
apply dvd_add ih
[END TACTIC]

`example_user`
[PROOF STATE]
b : ℝ
f : ℝ → ℝ
h₀ : ∀ (x : ℝ), f x = 3 * x ^ 4 - 7 * x ^ 3 + 2 * x ^ 2 - b * x + 1
h₁ : 3 * 1 ^ 4 - 7 * 1 ^ 3 + 2 * 1 ^ 2 - b * 1 + 1 = 1
⊢
b = -2

[LAST TACTIC]
rw h₀ at h₁
[STATE CHANGED]

[INSTRUCTIONS]
Please write the next tactic now.

`example_assistant`
[START TACTIC]
norm_num at h₁
[END TACTIC]
