`conv start`

`example_user`
Goals to prove:
[GOALS]
[GOAL] 1
(0 ≤ if x < 0 then -x else x) ∧
  ((if 0 < x then x else -x) = if x < 0 then -x else x) ∧
    ((if x < 0 then -x else x) = 0 ↔ x = 0) ∧
      (0 ≤ x → ((if 0 < x then x else -x) + if x < 0 then -x else x) = 2 * x) ∧
        (x ≤ 0 → ((if 0 < x then x else -x) + if x < 0 then -x else x) = -(2 * x))
[HYPOTHESES] 1
[HYPOTHESIS] x : ℤ
[HYPOTHESIS] result : ℤ := implementation x

[INFORMAL-THEOREM]
Given an integer x, your task is to find the magnitude of x.
The magnitude of an integer is defined as the absolute value of the integer.

[FORMAL-THEOREM]
def problem_spec
(impl: Int → Int)
(x: Int) :=
let spec (result: Int) :=
(result ≥ 0) ∧
(impl (-x) = result) ∧
(result = 0 ↔ x = 0) ∧
(0 ≤ x → impl (-x) + result = 2 * x) ∧
(x ≤ 0 → impl (-x) + result = -2 * x)
∃ result, impl x = result ∧
spec result

def implementation (x: Int) : Int :=
if x < 0 then -x else x

theorem correctness
(x: Int)
: problem_spec implementation x

[INFORMAL-PROOF]
1. Start by unfolding the `problem_spec` and assigning the implementation's output to a temporary variable `result`.
2. Early on, you will want to break the proof up into cases based on whether `x` is positive, negative, or zero.
3. Many of the intermediate goals can likely be proven using `linarith`.

[STEPS]
[STEP] unfold problem_spec
[STEP] let result := implementation x
[STEP] use result
[STEP] simp [result]
[STEP] simp [implementation]

[INCORRECT STEPS]
[STEP] cases x with n

[LAST STEP]
cases lt_or_ge x 0 with hx hx

[ERROR MESSAGE]
unknown tactic
[END]

`example_assistant`
[RUN TACTIC]
by_cases h_0_eq_x: x = 0
[END]


`example_user`
Goals to prove:
[GOALS]
[GOAL] 1
∀ (f₁ f₂ : ℕ), fibonacci_non_computable n f₁ → fibonacci_non_computable n f₂ → f₁ = f₂
[HYPOTHESES] 1
[HYPOTHESIS] n : ℕ

[INFORMAL-THEOREM]
Given an integer n, your task is to find the nth Fibonacci number.
The Fibonacci sequence is defined as follows:
- F(0) = 1
- F(1) = 1
- F(n) = F(n-1) + F(n-2) for n > 1

[FORMAL-THEOREM]
def problem_spec
(impl: Nat → Nat)
(n: Nat) :=
let spec (result: Nat) :=
fibonacci_non_computable n result
∃ result, impl n = result ∧
spec result

def implementation (n: Nat) : Nat :=
match n with
| 0 => 0
| 1 => 1
| n' + 2 => implementation n' + implementation (n' + 1)

lemma fib_comp_to_non_comp (n : ℕ)
(f : Nat → Nat)
(h_f_0: f 0 = 0)
(h_f_1: f 1 = 1)
(h_f_step: ∀ n, f (n + 2) = f n + f (n + 1))
: fibonacci_non_computable n (f n)

[INFORMAL-PROOF]
Prove a `fib_comp_to_non_comp` lemma that states that given a computable function `f : Nat → Nat` that follows the Fibonacci base cases (`f 0 = 1`, `f 1 = 1`) and recursive case (`∀ n, f (n + 2) = f n + f (n + 1)`), the built-in Lean 4 function `fibonacci_non_computable` called on `n` and `(f n)` outputs `True` (for all `n`).
1. Use induction and break the proof up into the base cases and the recursive case.

[LAST STEP]
revert f₁ f₂
[SUCCESS]
[END]

`example_assistant`
[RUN TACTIC]
induction' n using Nat.strong_induction_on with n' ih
[END]


`example_user`
Goals to prove:
[GOALS]
[GOAL] 1
fibonacci_non_computable n' (f n')
[HYPOTHESES] 1
[HYPOTHESIS] f : ℕ → ℕ
[HYPOTHESIS] h_f_0 : f 0 = 0
[HYPOTHESIS] h_f_1 : f 1 = 1
[HYPOTHESIS] h_f_step : ∀ (n : ℕ), f (n + 2) = f n + f (n + 1)
[HYPOTHESIS] n' : ℕ
[HYPOTHESIS] ih : ∀ m < n', fibonacci_non_computable m (f m)
[HYPOTHESIS] h_n'_lt_1 : n' < 2
[HYPOTHESIS] h_n'_eq_0 : n' = 0

[GOAL] 2
fibonacci_non_computable n' (f n')
[HYPOTHESES] 1
[HYPOTHESIS] f : ℕ → ℕ
[HYPOTHESIS] h_f_0 : f 0 = 0
[HYPOTHESIS] h_f_1 : f 1 = 1
[HYPOTHESIS] h_f_step : ∀ (n : ℕ), f (n + 2) = f n + f (n + 1)
[HYPOTHESIS] n' : ℕ
[HYPOTHESIS] ih : ∀ m < n', fibonacci_non_computable m (f m)
[HYPOTHESIS] h_n'_lt_1 : n' < 2
[HYPOTHESIS] h✝ : n' = 1

[GOAL] 3
fibonacci_non_computable n' (f n')
[HYPOTHESES] 1
[HYPOTHESIS] f : ℕ → ℕ
[HYPOTHESIS] h_f_0 : f 0 = 0
[HYPOTHESIS] h_f_1 : f 1 = 1
[HYPOTHESIS] h_f_step : ∀ (n : ℕ), f (n + 2) = f n + f (n + 1)
[HYPOTHESIS] n' : ℕ
[HYPOTHESIS] ih : ∀ m < n', fibonacci_non_computable m (f m)
[HYPOTHESIS] h_n'_lt_1 : ¬n' < 2

[INFORMAL-THEOREM]
Given an integer n, your task is to find the nth Fibonacci number.
The Fibonacci sequence is defined as follows:
- F(0) = 1
- F(1) = 1
- F(n) = F(n-1) + F(n-2) for n > 1

[FORMAL-THEOREM]
def problem_spec
(impl: Nat → Nat)
(n: Nat) :=
let spec (result: Nat) :=
fibonacci_non_computable n result
∃ result, impl n = result ∧
spec result

def implementation (n: Nat) : Nat :=
match n with
| 0 => 0
| 1 => 1
| n' + 2 => implementation n' + implementation (n' + 1)

lemma fib_comp_to_non_comp (n : ℕ)
(f : Nat → Nat)
(h_f_0: f 0 = 0)
(h_f_1: f 1 = 1)
(h_f_step: ∀ n, f (n + 2) = f n + f (n + 1))
: fibonacci_non_computable n (f n)

[INFORMAL-PROOF]
Prove a `fib_comp_to_non_comp` lemma that states that given a computable function `f : Nat → Nat` that follows the Fibonacci base cases (`f 0 = 1`, `f 1 = 1`) and recursive case (`∀ n, f (n + 2) = f n + f (n + 1)`), the built-in Lean 4 function `fibonacci_non_computable` called on `n` and `(f n)` outputs `True` (for all `n`).
1. Use induction and break the proof up into the base cases and the recursive case.

[STEPS]
[STEP] induction' n using Nat.strong_induction_on with n' ih
[STEP] by_cases h_n'_lt_1: n' < 2
[STEP] -- if n' < 2 then
have h_n'_eq_0: n' = 0 ∨ n' = 1 := by
[STEP]   interval_cases n'
[STEP]   all_goals simp
[STEP] cases h_n'_eq_0

[LAST STEP]
rename_i h_n'_eq_0
[SUCCESS]
[END]

`example_assistant`
[RUN TACTIC]
simp [h_n'_eq_0, h_f_0, fibonacci_non_computable.base0]
[END]


`example_user`
Goals to prove:
[GOALS]
[GOAL] 1
fibonacci_non_computable n' (f n')
[HYPOTHESES] 1
[HYPOTHESIS] f : ℕ → ℕ
[HYPOTHESIS] h_f_0 : f 0 = 0
[HYPOTHESIS] h_f_1 : f 1 = 1
[HYPOTHESIS] h_f_step : ∀ (n : ℕ), f (n + 2) = f n + f (n + 1)
[HYPOTHESIS] n' : ℕ
[HYPOTHESIS] ih : ∀ m < n', fibonacci_non_computable m (f m)
[HYPOTHESIS] h_n'_lt_1 : ¬n' < 2
[HYPOTHESIS] n'' : ℕ := n' - 2
[HYPOTHESIS] h_n''_eq_n_plus_2 : n' = n'' + 2
[HYPOTHESIS] h_n''_lt_n' : n'' < n'
[HYPOTHESIS] h_fib_n'' : f (n'' + 2) = f n'' + f (n'' + 1)
[HYPOTHESIS] h_fib_n''_non_computable : fibonacci_non_computable n'' (f n'')
[HYPOTHESIS] h_fib_n''_plus_1_non_computable : fibonacci_non_computable (n'' + 1) (f (n'' + 1))
[HYPOTHESIS] h_fib_n''_plus_2_non_computable : fibonacci_non_computable (n'' + 2) (f (n'' + 2))

[INFORMAL-THEOREM]
Given an integer n, your task is to find the nth Fibonacci number.
The Fibonacci sequence is defined as follows:
- F(0) = 1
- F(1) = 1
- F(n) = F(n-1) + F(n-2) for n > 1

[FORMAL-THEOREM]
def problem_spec
(impl: Nat → Nat)
(n: Nat) :=
let spec (result: Nat) :=
fibonacci_non_computable n result
∃ result, impl n = result ∧
spec result

def implementation (n: Nat) : Nat :=
match n with
| 0 => 0
| 1 => 1
| n' + 2 => implementation n' + implementation (n' + 1)

lemma fib_comp_to_non_comp (n : ℕ)
(f : Nat → Nat)
(h_f_0: f 0 = 0)
(h_f_1: f 1 = 1)
(h_f_step: ∀ n, f (n + 2) = f n + f (n + 1))
: fibonacci_non_computable n (f n)

[INFORMAL-PROOF]
Prove a `fib_comp_to_non_comp` lemma that states that given a computable function `f : Nat → Nat` that follows the Fibonacci base cases (`f 0 = 1`, `f 1 = 1`) and recursive case (`∀ n, f (n + 2) = f n + f (n + 1)`), the built-in Lean 4 function `fibonacci_non_computable` called on `n` and `(f n)` outputs `True` (for all `n`).
1. Use induction and break the proof up into the base cases and the recursive case.

[STEPS]
[STEP] induction' n using Nat.strong_induction_on with n' ih
[STEP] by_cases h_n'_lt_1: n' < 2
[STEP] -- if n' < 2 then
have h_n'_eq_0: n' = 0 ∨ n' = 1 := by
[STEP]   interval_cases n'
[STEP]   all_goals simp
[STEP] cases h_n'_eq_0
[STEP] rename_i h_n'_eq_0
[STEP] simp [h_n'_eq_0, h_f_0, fibonacci_non_computable.base0]
[STEP] rename_i h_n'_eq_1
[STEP] simp [h_n'_eq_1, h_f_1, fibonacci_non_computable.base1]
[STEP] set n'' := n' - 2
[STEP] have h_n''_eq_n_plus_2: n' = n'' + 2 := by
[STEP]   rw [Nat.sub_add_cancel]
[STEP]   linarith
[STEP] have h_n''_lt_n': n'' < n' := by
[STEP]   linarith
[STEP] have h_fib_n'':= h_f_step n''
[STEP] have h_fib_n''_non_computable := ih n'' h_n''_lt_n'
[STEP] have h_fib_n''_plus_1_non_computable := ih (n'' + 1) (by linarith)
[STEP] have h_fib_n''_plus_2_non_computable :=
  fibonacci_non_computable.step _ _ _ h_fib_n''_non_computable h_fib_n''_plus_1_non_computable

[LAST STEP]
rw [←h_fib_n''] at h_fib_n''_plus_2_non_computable
[SUCCESS]
[END]

`example_assistant`
[RUN TACTIC]
rw [←h_n''_eq_n_plus_2] at h_fib_n''_plus_2_non_computable
[END]


`example_user`
Goals to prove:
[GOALS]
[GOAL] 1
fibonacci_non_computable n (implementation n)
[HYPOTHESES] 1
[HYPOTHESIS] n : ℕ
[HYPOTHESIS] result : ℕ := implementation n

[INFORMAL-THEOREM]
Given an integer n, your task is to find the nth Fibonacci number.
The Fibonacci sequence is defined as follows:
- F(0) = 1
- F(1) = 1
- F(n) = F(n-1) + F(n-2) for n > 1

[FORMAL-THEOREM]
def problem_spec
(impl: Nat → Nat)
(n: Nat) :=
let spec (result: Nat) :=
fibonacci_non_computable n result
∃ result, impl n = result ∧
spec result

def implementation (n: Nat) : Nat :=
match n with
| 0 => 0
| 1 => 1
| n' + 2 => implementation n' + implementation (n' + 1)

theorem correctness
(n: Nat)
: problem_spec implementation n

[INFORMAL-PROOF]
1. Start by unfolding the `problem_spec` and assigning the implementation's output to a temporary variable `result`.
2. Use the `have` keyword three times to show that `implementation` follows the three properties of the Fibonacci function:
  - `implementation 0 = 1`
  - `implementation 1 = 1`
  - `∀ n', implementation (n' + 2) = implementation n' + implementation (n' + 1)`
3. Then use these three hypotheses and the `fib_comp_to_non_comp` lemma to show that `implementation` satisfies `fibonacci_non_computable`, as required by the `spec`.

Throughout the proof, you can freely use any of the below helper lemmas, which you can assume to be true:
[HELPER LEMMAS]
[HELPER LEMMA]
lemma fib_comp_to_non_comp (n : ℕ)
(f : Nat → Nat)
(h_f_0: f 0 = 1)
(h_f_1: f 1 = 1)
(h_f_step: ∀ n, f (n + 2) = f n + f (n + 1))
: fibonacci_non_computable n (f n) :=

[STEPS]
[STEP] unfold problem_spec
[STEP] let result := implementation n
[STEP] use result
[STEP] simp [result]

[LAST STEP]
simp [implementation]

[ERROR MESSAGE]
simp made no progress
[END]

`example_assistant`
[RUN TACTIC]
have h_impl_n : ∀ n', implementation (n' + 2) = implementation n' + implementation (n' + 1) := by
[END]


`example_user`
Goals to prove:
[GOALS]
[GOAL] 1
fibonacci_non_computable n (implementation n)
[HYPOTHESES] 1
[HYPOTHESIS] n : ℕ
[HYPOTHESIS] result : ℕ := implementation n
[HYPOTHESIS] h_impl_n : ∀ (n' : ℕ), implementation (n' + 2) = implementation n' + implementation (n' + 1)
[HYPOTHESIS] h_impl_0 : implementation 0 = 0
[HYPOTHESIS] h_impl_1 : implementation 1 = 1

[INFORMAL-THEOREM]
Given an integer n, your task is to find the nth Fibonacci number.
The Fibonacci sequence is defined as follows:
- F(0) = 1
- F(1) = 1
- F(n) = F(n-1) + F(n-2) for n > 1

[FORMAL-THEOREM]
def problem_spec
(impl: Nat → Nat)
(n: Nat) :=
let spec (result: Nat) :=
fibonacci_non_computable n result
∃ result, impl n = result ∧
spec result

def implementation (n: Nat) : Nat :=
match n with
| 0 => 0
| 1 => 1
| n' + 2 => implementation n' + implementation (n' + 1)

theorem correctness
(n: Nat)
: problem_spec implementation n

[INFORMAL-PROOF]
1. Start by unfolding the `problem_spec` and assigning the implementation's output to a temporary variable `result`.
2. Use the `have` keyword three times to show that `implementation` follows the three properties of the Fibonacci function:
  - `implementation 0 = 1`
  - `implementation 1 = 1`
  - `∀ n', implementation (n' + 2) = implementation n' + implementation (n' + 1)`
3. Then use these three hypotheses and the `fib_comp_to_non_comp` lemma to show that `implementation` satisfies `fibonacci_non_computable`, as required by the `spec`.

Throughout the proof, you can freely use any of the below helper lemmas, which you can assume to be true:
[HELPER LEMMAS]
[HELPER LEMMA]
lemma fib_comp_to_non_comp (n : ℕ)
(f : Nat → Nat)
(h_f_0: f 0 = 1)
(h_f_1: f 1 = 1)
(h_f_step: ∀ n, f (n + 2) = f n + f (n + 1))
: fibonacci_non_computable n (f n) :=

[STEPS]
[STEP] unfold problem_spec
[STEP] let result := implementation n
[STEP] use result
[STEP] simp [result]
[STEP] have h_impl_n : ∀ n', implementation (n' + 2) = implementation n' + implementation (n' + 1) := by
[STEP]   intro n'
[STEP]   rw [implementation]
[STEP] have h_impl_0 : implementation 0 = 0 := by
[STEP]   rw [implementation]
[STEP] have h_impl_1 : implementation 1 = 1 := by
[STEP]   rw [implementation]

[LAST STEP]
apply fib_comp_to_non_comp n implementation (by rw [h_impl_0,←Nat.zero_add (1 : ℕ)]) h_impl_1 h_impl_n

[ERROR MESSAGE]
tactic 'rewrite' failed, did not find instance of the pattern in the target expression
 1
n : ℕ
result : ℕ := implementation n
h_impl_n : ∀ (n' : ℕ), implementation (n' + 2) = implementation n' + implementation (n' + 1)
h_impl_0 : implementation 0 = 0
h_impl_1 : implementation 1 = 1
⊢ 0 = 0
[END]

`example_assistant`
[RUN TACTIC]
apply fib_comp_to_non_comp
[END]


`example_user`
Goals to prove:
[GOALS]
[GOAL] 1
implementation.loop score_changes (threshold - k) score coins =
  implementation.loop score_changes threshold (score + k) coins
[HYPOTHESES] 1
[HYPOTHESIS] score_changes : List ℤ
[HYPOTHESIS] threshold score : ℤ
[HYPOTHESIS] coins : ℕ
[HYPOTHESIS] k : ℤ
[HYPOTHESIS] h_rounds_played : score_changes.length > 0

[INFORMAL-THEOREM]
In a game, a player's score starts at 0 and is updated round by round using values from the list
score_changes (where positive numbers add to the score and negative numbers subtract).
After each round, as long as the player's cumulative score is greater than or equal to the given threshold,
the player wins a coin for that round.
Your task is to compute and return the total number of coins won by the player by the end of the game.

[FORMAL-THEOREM]
def problem_spec
(impl: List Int → Int → Nat)
(score_changes: List Int)
(threshold: Int) :=
let spec (score_changes' : List Int) (threshold' : Int) (result: Nat) :=
score_changes'.length > 0 →
if result = 0 then
  ∀ i, 1 ≤ i ∧ i ≤ score_changes'.length →
  (score_changes'.take i).sum < threshold'
else
  (∃ i, 1 ≤ i ∧ i ≤ score_changes'.length →
  (score_changes'.take i).sum ≥ threshold' →
  ( let score_changes'' := score_changes'.drop i;
    let threshold'' := threshold' - (score_changes'.take i).sum;
    let result' := impl score_changes'' threshold'';
    result = 1 + result') →
  ∀ i', 1 ≤ i' ∧ i' < i → (score_changes'.take i').sum < threshold
  );
∃ result, impl score_changes threshold = result ∧
spec score_changes threshold result

def implementation (score_changes: List Int) (threshold: Int) : Nat :=
let rec loop (score_changes: List Int) (threshold: Int) (score: Int) (coins: Nat) : Nat :=
  match score_changes with
  | [] => coins
  | head :: tail =>
    let score' := head + score
    let coins' := if score' ≥ threshold then coins + 1 else coins
    loop tail threshold score' coins'
loop score_changes threshold 0 0

lemma implementation_loop_threshold_invariant
(score_changes: List Int)
(threshold: Int)
(score: Int)
(coins: Nat)
(k: Int)
(h_rounds_played: score_changes.length > 0)
: implementation.loop score_changes (threshold - k) score coins
= implementation.loop score_changes threshold (score + k) coins

[INFORMAL-PROOF]
Prove an `implementation_loop_threshold_invariant` lemma that states that for all integers `k`, decreasing the threshold by `k` yields the same output of `implementation.loop` as increasing the score by `k`.
1. Use induction and break the proof up into cases based on whether the head plus the cumulative score reaches the threshold.

`example_assistant`
[RUN TACTIC]
induction' score_changes generalizing score coins
[END]


`example_user`
Goals to prove:
[GOALS]
[GOAL] 1
implementation.loop tail (threshold - k) (head + score) (coins + 1) =
  implementation.loop tail threshold (head + score + k) (coins + 1)
[HYPOTHESES] 1
[HYPOTHESIS] threshold k head : ℤ
[HYPOTHESIS] tail : List ℤ
[HYPOTHESIS] ih : ∀ (score : ℤ) (coins : ℕ),
[HYPOTHESIS]   tail.length > 0 →
[HYPOTHESIS]     implementation.loop tail (threshold - k) score coins = implementation.loop tail threshold (score + k) coins
[HYPOTHESIS] score : ℤ
[HYPOTHESIS] coins : ℕ
[HYPOTHESIS] h_rounds_played : (head :: tail).length > 0
[HYPOTHESIS] h_head_ge_threshold : head + score ≥ threshold - k
[HYPOTHESIS] h_head_ge_threshold' : threshold ≤ head + score + k
[HYPOTHESIS] h_head_ge_threshold'' : threshold ≤ head + (score + k)
[HYPOTHESIS] h_tail_len_0 : tail.length = 0

[GOAL] 2
implementation.loop tail (threshold - k) (head + score) (coins + 1) =
  implementation.loop tail threshold (head + score + k) (coins + 1)
[HYPOTHESES] 1
[HYPOTHESIS] threshold k head : ℤ
[HYPOTHESIS] tail : List ℤ
[HYPOTHESIS] ih : ∀ (score : ℤ) (coins : ℕ),
[HYPOTHESIS]   tail.length > 0 →
[HYPOTHESIS]     implementation.loop tail (threshold - k) score coins = implementation.loop tail threshold (score + k) coins
[HYPOTHESIS] score : ℤ
[HYPOTHESIS] coins : ℕ
[HYPOTHESIS] h_rounds_played : (head :: tail).length > 0
[HYPOTHESIS] h_head_ge_threshold : head + score ≥ threshold - k
[HYPOTHESIS] h_head_ge_threshold' : threshold ≤ head + score + k
[HYPOTHESIS] h_head_ge_threshold'' : threshold ≤ head + (score + k)
[HYPOTHESIS] h_tail_len_0 : ¬tail.length ≤ 0

[GOAL] 3
implementation.loop (head :: tail) (threshold - k) score coins =
  implementation.loop (head :: tail) threshold (score + k) coins
[HYPOTHESES] 1
[HYPOTHESIS] threshold k head : ℤ
[HYPOTHESIS] tail : List ℤ
[HYPOTHESIS] ih : ∀ (score : ℤ) (coins : ℕ),
[HYPOTHESIS]   tail.length > 0 →
[HYPOTHESIS]     implementation.loop tail (threshold - k) score coins = implementation.loop tail threshold (score + k) coins
[HYPOTHESIS] score : ℤ
[HYPOTHESIS] coins : ℕ
[HYPOTHESIS] h_rounds_played : (head :: tail).length > 0
[HYPOTHESIS] h_head_ge_threshold : ¬head + score ≥ threshold - k

[INFORMAL-THEOREM]
In a game, a player's score starts at 0 and is updated round by round using values from the list
score_changes (where positive numbers add to the score and negative numbers subtract).
After each round, as long as the player's cumulative score is greater than or equal to the given threshold,
the player wins a coin for that round.
Your task is to compute and return the total number of coins won by the player by the end of the game.

[FORMAL-THEOREM]
def problem_spec
(impl: List Int → Int → Nat)
(score_changes: List Int)
(threshold: Int) :=
let spec (score_changes' : List Int) (threshold' : Int) (result: Nat) :=
score_changes'.length > 0 →
if result = 0 then
  ∀ i, 1 ≤ i ∧ i ≤ score_changes'.length →
  (score_changes'.take i).sum < threshold'
else
  (∃ i, 1 ≤ i ∧ i ≤ score_changes'.length →
  (score_changes'.take i).sum ≥ threshold' →
  ( let score_changes'' := score_changes'.drop i;
    let threshold'' := threshold' - (score_changes'.take i).sum;
    let result' := impl score_changes'' threshold'';
    result = 1 + result') →
  ∀ i', 1 ≤ i' ∧ i' < i → (score_changes'.take i').sum < threshold
  );
∃ result, impl score_changes threshold = result ∧
spec score_changes threshold result

def implementation (score_changes: List Int) (threshold: Int) : Nat :=
let rec loop (score_changes: List Int) (threshold: Int) (score: Int) (coins: Nat) : Nat :=
  match score_changes with
  | [] => coins
  | head :: tail =>
    let score' := head + score
    let coins' := if score' ≥ threshold then coins + 1 else coins
    loop tail threshold score' coins'
loop score_changes threshold 0 0

lemma implementation_loop_threshold_invariant
(score_changes: List Int)
(threshold: Int)
(score: Int)
(coins: Nat)
(k: Int)
(h_rounds_played: score_changes.length > 0)
: implementation.loop score_changes (threshold - k) score coins
= implementation.loop score_changes threshold (score + k) coins

[INFORMAL-PROOF]
Prove an `implementation_loop_threshold_invariant` lemma that states that for all integers `k`, decreasing the threshold by `k` yields the same output of `implementation.loop` as increasing the score by `k`.
1. Use induction and break the proof up into cases based on whether the head plus the cumulative score reaches the threshold.

[STEPS]
[STEP] induction' score_changes generalizing score coins
[STEP] simp at h_rounds_played
[STEP] rename_i head tail ih
[STEP] by_cases h_head_ge_threshold: head + score ≥ threshold - k
[STEP] -- case where head + score ≥ threshold
simp [implementation.loop]
[STEP] have h_head_ge_threshold': threshold ≤ head + score + k := by
[STEP]   linarith
[STEP] simp [h_head_ge_threshold']
[STEP] have h_head_ge_threshold'': threshold ≤ head + (score + k) := by
[STEP]   linarith
[STEP] simp [h_head_ge_threshold'']
[STEP] simp [←Int.add_assoc]
[STEP] by_cases h_tail_len_0: tail.length ≤ 0

[LAST STEP]
-- case where tail.length ≤ 0
rw [Nat.le_zero] at h_tail_len_0
[SUCCESS]
[END]

`example_assistant`
[RUN TACTIC]
have h_tail_nil := List.eq_nil_of_length_eq_zero h_tail_len_0
[END]


`example_user`
Goals to prove:
[GOALS]
[GOAL] 1
implementation.loop tail (threshold - k) (head + score) (if threshold ≤ head + score + k then coins + 1 else coins) =
  implementation.loop tail threshold (head + (score + k)) (if threshold ≤ head + (score + k) then coins + 1 else coins)
[HYPOTHESES] 1
[HYPOTHESIS] threshold k head : ℤ
[HYPOTHESIS] tail : List ℤ
[HYPOTHESIS] score : ℤ
[HYPOTHESIS] coins : ℕ
[HYPOTHESIS] h_rounds_played : (head :: tail).length > 0
[HYPOTHESIS] h_perm' : head + score + k = head + (score + k)
[HYPOTHESIS] h_tail_len_0 : ¬tail.length ≤ 0
[HYPOTHESIS] h_tail_len_gt_0 : tail.length > 0
[HYPOTHESIS] ih : implementation.loop tail (threshold - k) (head + score) coins =
[HYPOTHESIS]   implementation.loop tail threshold (head + score + k) coins
[HYPOTHESIS] h_head_ge_threshold : head + score + k < threshold

[INFORMAL-THEOREM]
In a game, a player's score starts at 0 and is updated round by round using values from the list
score_changes (where positive numbers add to the score and negative numbers subtract).
After each round, as long as the player's cumulative score is greater than or equal to the given threshold,
the player wins a coin for that round.
Your task is to compute and return the total number of coins won by the player by the end of the game.

[FORMAL-THEOREM]
def problem_spec
(impl: List Int → Int → Nat)
(score_changes: List Int)
(threshold: Int) :=
let spec (score_changes' : List Int) (threshold' : Int) (result: Nat) :=
score_changes'.length > 0 →
if result = 0 then
  ∀ i, 1 ≤ i ∧ i ≤ score_changes'.length →
  (score_changes'.take i).sum < threshold'
else
  (∃ i, 1 ≤ i ∧ i ≤ score_changes'.length →
  (score_changes'.take i).sum ≥ threshold' →
  ( let score_changes'' := score_changes'.drop i;
    let threshold'' := threshold' - (score_changes'.take i).sum;
    let result' := impl score_changes'' threshold'';
    result = 1 + result') →
  ∀ i', 1 ≤ i' ∧ i' < i → (score_changes'.take i').sum < threshold
  );
∃ result, impl score_changes threshold = result ∧
spec score_changes threshold result

def implementation (score_changes: List Int) (threshold: Int) : Nat :=
let rec loop (score_changes: List Int) (threshold: Int) (score: Int) (coins: Nat) : Nat :=
  match score_changes with
  | [] => coins
  | head :: tail =>
    let score' := head + score
    let coins' := if score' ≥ threshold then coins + 1 else coins
    loop tail threshold score' coins'
loop score_changes threshold 0 0

lemma implementation_loop_threshold_invariant
(score_changes: List Int)
(threshold: Int)
(score: Int)
(coins: Nat)
(k: Int)
(h_rounds_played: score_changes.length > 0)
: implementation.loop score_changes (threshold - k) score coins
= implementation.loop score_changes threshold (score + k) coins

[INFORMAL-PROOF]
Prove an `implementation_loop_threshold_invariant` lemma that states that for all integers `k`, decreasing the threshold by `k` yields the same output of `implementation.loop` as increasing the score by `k`.
1. Use induction and break the proof up into cases based on whether the head plus the cumulative score reaches the threshold.

[STEPS]
[STEP] induction' score_changes generalizing score coins
[STEP] simp at h_rounds_played
[STEP] rename_i head tail ih
[STEP] by_cases h_head_ge_threshold: head + score ≥ threshold - k
[STEP] -- case where head + score ≥ threshold
simp [implementation.loop]
[STEP] have h_head_ge_threshold': threshold ≤ head + score + k := by
[STEP]   linarith
[STEP] simp [h_head_ge_threshold']
[STEP] have h_head_ge_threshold'': threshold ≤ head + (score + k) := by
[STEP]   linarith
[STEP] simp [h_head_ge_threshold'']
[STEP] simp [←Int.add_assoc]
[STEP] by_cases h_tail_len_0: tail.length ≤ 0
[STEP] -- case where tail.length ≤ 0
rw [Nat.le_zero] at h_tail_len_0
[STEP] have h_tail_nil := List.eq_nil_of_length_eq_zero h_tail_len_0
[STEP] simp [h_tail_nil]
[STEP] simp [implementation.loop]
[STEP] -- case where tail.length > 0
[STEP] have h_tail_len_gt_0: tail.length > 0 := by
[STEP]   linarith
[STEP] simp [h_tail_len_gt_0] at ih
[STEP] specialize ih (head + score) (coins + 1)
[STEP] simp [←ih]
[STEP] -- case where head + score < threshold
have h_perm': head + score + k = head + (score + k) := by
[STEP]   linarith
[STEP] by_cases h_tail_len_0: tail.length ≤ 0
[STEP] rw [Nat.le_zero] at h_tail_len_0
[STEP] have h_tail_nil := List.eq_nil_of_length_eq_zero h_tail_len_0
[STEP] simp [h_tail_nil]
[STEP] simp [implementation.loop]
[STEP] rw [h_perm']
[STEP] have h_tail_len_gt_0: tail.length > 0 := by
[STEP]   linarith
[STEP] simp [h_tail_len_gt_0] at ih
[STEP] specialize ih (head + score) coins
[STEP] simp [implementation.loop]

[LAST STEP]
simp at h_head_ge_threshold
[SUCCESS]
[END]

`example_assistant`
[RUN TACTIC]
have h_head_lt_threshold: ¬ (threshold ≤ head + score + k) := by
[END]


`example_user`
Goals to prove:
[GOALS]
[GOAL] 1
if implementation.loop score_changes threshold 0 0 = 0 then
  ∀ (i : ℕ), 1 ≤ i → i ≤ score_changes.length → (List.take i score_changes).sum < threshold
else
  ∃ i,
    1 ≤ i →
      i ≤ score_changes.length →
        threshold ≤ (List.take i score_changes).sum →
          implementation.loop score_changes threshold 0 0 =
              1 + implementation.loop (List.drop i score_changes) (threshold - (List.take i score_changes).sum) 0 0 →
            ∀ (i' : ℕ), 1 ≤ i' → i' < i → (List.take i' score_changes).sum < threshold
[HYPOTHESES] 1
[HYPOTHESIS] score_changes : List ℤ
[HYPOTHESIS] threshold : ℤ
[HYPOTHESIS] result : ℕ := implementation score_changes threshold
[HYPOTHESIS] h_rounds_played : 0 < score_changes.length
[HYPOTHESIS] h_stop : 0 = implementation.loop score_changes threshold 0 0 →
[HYPOTHESIS]   ∀ (i : ℕ), 1 ≤ i ∧ i ≤ score_changes.length → 0 + (List.take i score_changes).sum < threshold

[INFORMAL-THEOREM]
In a game, a player's score starts at 0 and is updated round by round using values from the list
score_changes (where positive numbers add to the score and negative numbers subtract).
After each round, as long as the player's cumulative score is greater than or equal to the given threshold,
the player wins a coin for that round.
Your task is to compute and return the total number of coins won by the player by the end of the game.

[FORMAL-THEOREM]
def problem_spec
(impl: List Int → Int → Nat)
(score_changes: List Int)
(threshold: Int) :=
let spec (score_changes' : List Int) (threshold' : Int) (result: Nat) :=
score_changes'.length > 0 →
if result = 0 then
  ∀ i, 1 ≤ i ∧ i ≤ score_changes'.length →
  (score_changes'.take i).sum < threshold'
else
  (∃ i, 1 ≤ i ∧ i ≤ score_changes'.length →
  (score_changes'.take i).sum ≥ threshold' →
  ( let score_changes'' := score_changes'.drop i;
    let threshold'' := threshold' - (score_changes'.take i).sum;
    let result' := impl score_changes'' threshold'';
    result = 1 + result') →
  ∀ i', 1 ≤ i' ∧ i' < i → (score_changes'.take i').sum < threshold
  );
∃ result, impl score_changes threshold = result ∧
spec score_changes threshold result

def implementation (score_changes: List Int) (threshold: Int) : Nat :=
let rec loop (score_changes: List Int) (threshold: Int) (score: Int) (coins: Nat) : Nat :=
  match score_changes with
  | [] => coins
  | head :: tail =>
    let score' := head + score
    let coins' := if score' ≥ threshold then coins + 1 else coins
    loop tail threshold score' coins'
loop score_changes threshold 0 0

theorem correctness
(score_changes: List Int)
(threshold: Int)
: problem_spec implementation score_changes threshold

[INFORMAL-PROOF]
1. Start by unfolding the `problem_spec` and assigning the implementation's output to a temporary variable `result`.
2. Early on, you will want to break the proof up into cases based on whether the output of `implementation_loop` (with initial values as input) is 0.
3. Use the `implementation_loop_threshold_invariant`, `implementation_loop_invariant_stop`, and `implementation_loop_invariant_continue` lemmas in the proof.

Throughout the proof, you can freely use any of the below helper lemmas, which you can assume to be true:
[HELPER LEMMAS]
[HELPER LEMMA]
lemma implementation_loop_threshold_invariant
(score_changes: List Int)
(threshold: Int)
(score: Int)
(coins: Nat)
(k: Int)
(h_rounds_played: score_changes.length > 0)
: implementation.loop score_changes (threshold - k) score coins
= implementation.loop score_changes threshold (score + k) coins :=
[HELPER LEMMA]
lemma implementation_loop_simple_increment
(head: Int)
(score_changes_tail: List Int)
(threshold: Int)
(score: Int)
(coins: Nat)
: (head + score < threshold →
implementation.loop (head :: score_changes_tail) threshold score coins =
implementation.loop (score_changes_tail) threshold (head + score) coins) ∧
(head + score ≥ threshold →
implementation.loop (head :: score_changes_tail) threshold score coins =
1 + implementation.loop (score_changes_tail) threshold (head + score) coins) :=
[HELPER LEMMA]
lemma implementation_loop_coin_monotonic_increasing
(score_changes: List Int)
(threshold: Int)
(score: Int)
(coins: Nat)
(h_rounds_played: score_changes.length > 0)
: coins ≤ implementation.loop score_changes threshold score coins :=
[HELPER LEMMA]
lemma implementation_loop_invariant_stop
(score_changes: List Int)
(threshold: Int)
(score: Int)
(coins: Nat)
(h_rounds_played: score_changes.length > 0)
(h_within_threshold: coins = implementation.loop score_changes threshold score coins)
: ∀ i, 1 ≤ i ∧ i ≤ score_changes.length →
score + (score_changes.take i).sum < threshold :=
[HELPER LEMMA]
lemma implementation_loop_invariant_continue
(score_changes: List Int)
(threshold: Int)
(score: Int)
(coins: Nat)
(h_rounds_played: score_changes.length > 0)
(h_within_threshold: coins < implementation.loop score_changes threshold score coins)
:∃ i', 1 ≤ i' ∧ i' ≤ score_changes.length →
(score + (score_changes.take i').sum ≥ threshold) →
implementation.loop score_changes threshold score coins =
1 + implementation.loop (score_changes.drop i') threshold
(score + (score_changes.take i').sum) coins →
∀ i, 1 ≤ i ∧ i < i' → score + (score_changes.take i).sum < threshold :=

[STEPS]
[STEP] -- sometimes we have to create a temporary variable to use in the proof
unfold problem_spec
[STEP] let result := implementation score_changes threshold
[STEP] use result
[STEP] simp [result]
[STEP] simp [implementation]
[STEP] intros h_rounds_played

[LAST STEP]
have h_stop := implementation_loop_invariant_stop score_changes threshold 0 0 h_rounds_played
[SUCCESS]
[END]

`example_assistant`
[RUN TACTIC]
by_cases h_implementation_stop: implementation.loop score_changes threshold 0 0 = 0
[END]


`example_user`
Goals to prove:
[GOALS]
[GOAL] 1
problem_spec implementation x y
[HYPOTHESES] 1
[HYPOTHESIS] x y : ℤ

[INFORMAL-THEOREM]
Given two integers x and y, your task is to find if x is a square of y.
The function should return true if x is a square of y, otherwise false.

[FORMAL-THEOREM]
def problem_spec
(impl: Int → Int → Bool)
(x: Int)
(y: Int) :=
let spec (result: Bool) :=
result = true ↔ x = y^2;
∃ result, impl x y = result ∧
spec result

def implementation (x: Int) (y: Int) : Bool :=
if x = y * y then
  true
else
  false

theorem correctness
(x: Int)
(y: Int)
: problem_spec implementation x y

[INFORMAL-PROOF]
1. Start by unfolding the `problem_spec` and assigning the implementation's output to a temporary variable `result`.
2. Simplify the goal.
3. Use the `have` keyword to create a new hypothesis equating the operation of squaring a variable to that of multiplying the variable by itself.
4. Use this new hypothesis to rewrite the goal.
[END]

`example_assistant`
[RUN TACTIC]
unfold problem_spec
[END]


`example_user`
Goals to prove:
[GOALS]
[GOAL] 1
let spec := fun result => result = true ↔ x = y ^ 2;
∃ result, implementation x y = result ∧ spec result
[HYPOTHESES] 1
[HYPOTHESIS] x y : ℤ

[INFORMAL-THEOREM]
Given two integers x and y, your task is to find if x is a square of y.
The function should return true if x is a square of y, otherwise false.

[FORMAL-THEOREM]
def problem_spec
(impl: Int → Int → Bool)
(x: Int)
(y: Int) :=
let spec (result: Bool) :=
result = true ↔ x = y^2;
∃ result, impl x y = result ∧
spec result

def implementation (x: Int) (y: Int) : Bool :=
if x = y * y then
  true
else
  false

theorem correctness
(x: Int)
(y: Int)
: problem_spec implementation x y

[INFORMAL-PROOF]
1. Start by unfolding the `problem_spec` and assigning the implementation's output to a temporary variable `result`.
2. Simplify the goal.
3. Use the `have` keyword to create a new hypothesis equating the operation of squaring a variable to that of multiplying the variable by itself.
4. Use this new hypothesis to rewrite the goal.

[LAST STEP]
unfold problem_spec
[SUCCESS]
[END]

`example_assistant`
[RUN TACTIC]
let result := implementation x y
[END]


`example_user`
Goals to prove:
[GOALS]
[GOAL] 1
let spec := fun result => result = true ↔ x = y ^ 2;
∃ result, implementation x y = result ∧ spec result
[HYPOTHESES] 1
[HYPOTHESIS] x y : ℤ
[HYPOTHESIS] result : Bool := implementation x y

[INFORMAL-THEOREM]
Given two integers x and y, your task is to find if x is a square of y.
The function should return true if x is a square of y, otherwise false.

[FORMAL-THEOREM]
def problem_spec
(impl: Int → Int → Bool)
(x: Int)
(y: Int) :=
let spec (result: Bool) :=
result = true ↔ x = y^2;
∃ result, impl x y = result ∧
spec result

def implementation (x: Int) (y: Int) : Bool :=
if x = y * y then
  true
else
  false

theorem correctness
(x: Int)
(y: Int)
: problem_spec implementation x y

[INFORMAL-PROOF]
1. Start by unfolding the `problem_spec` and assigning the implementation's output to a temporary variable `result`.
2. Simplify the goal.
3. Use the `have` keyword to create a new hypothesis equating the operation of squaring a variable to that of multiplying the variable by itself.
4. Use this new hypothesis to rewrite the goal.

[STEPS]
[STEP] unfold problem_spec

[LAST STEP]
let result := implementation x y
[SUCCESS]
[END]

`example_assistant`
[RUN TACTIC]
use result
[END]


`example_user`
Goals to prove:
[GOALS]
[GOAL] 1
implementation x y = result ∧ (fun result => result = true ↔ x = y ^ 2) result
[HYPOTHESES] 1
[HYPOTHESIS] x y : ℤ
[HYPOTHESIS] result : Bool := implementation x y

[INFORMAL-THEOREM]
Given two integers x and y, your task is to find if x is a square of y.
The function should return true if x is a square of y, otherwise false.

[FORMAL-THEOREM]
def problem_spec
(impl: Int → Int → Bool)
(x: Int)
(y: Int) :=
let spec (result: Bool) :=
result = true ↔ x = y^2;
∃ result, impl x y = result ∧
spec result

def implementation (x: Int) (y: Int) : Bool :=
if x = y * y then
  true
else
  false

theorem correctness
(x: Int)
(y: Int)
: problem_spec implementation x y

[INFORMAL-PROOF]
1. Start by unfolding the `problem_spec` and assigning the implementation's output to a temporary variable `result`.
2. Simplify the goal.
3. Use the `have` keyword to create a new hypothesis equating the operation of squaring a variable to that of multiplying the variable by itself.
4. Use this new hypothesis to rewrite the goal.

[STEPS]
[STEP] unfold problem_spec
[STEP] let result := implementation x y

[LAST STEP]
use result
[SUCCESS]
[END]

`example_assistant`
[RUN TACTIC]
simp [result]
[END]


`example_user`
Goals to prove:
[GOALS]
[GOAL] 1
implementation x y = true ↔ x = y ^ 2
[HYPOTHESES] 1
[HYPOTHESIS] x y : ℤ
[HYPOTHESIS] result : Bool := implementation x y

[INFORMAL-THEOREM]
Given two integers x and y, your task is to find if x is a square of y.
The function should return true if x is a square of y, otherwise false.

[FORMAL-THEOREM]
def problem_spec
(impl: Int → Int → Bool)
(x: Int)
(y: Int) :=
let spec (result: Bool) :=
result = true ↔ x = y^2;
∃ result, impl x y = result ∧
spec result

def implementation (x: Int) (y: Int) : Bool :=
if x = y * y then
  true
else
  false

theorem correctness
(x: Int)
(y: Int)
: problem_spec implementation x y

[INFORMAL-PROOF]
1. Start by unfolding the `problem_spec` and assigning the implementation's output to a temporary variable `result`.
2. Simplify the goal.
3. Use the `have` keyword to create a new hypothesis equating the operation of squaring a variable to that of multiplying the variable by itself.
4. Use this new hypothesis to rewrite the goal.

[STEPS]
[STEP] unfold problem_spec
[STEP] let result := implementation x y
[STEP] use result

[LAST STEP]
simp [result]
[SUCCESS]
[END]

`example_assistant`
[RUN TACTIC]
simp [implementation]
[END]


`example_user`
Goals to prove:
[GOALS]
[GOAL] 1
x = y * y ↔ x = y ^ 2
[HYPOTHESES] 1
[HYPOTHESIS] x y : ℤ
[HYPOTHESIS] result : Bool := implementation x y

[INFORMAL-THEOREM]
Given two integers x and y, your task is to find if x is a square of y.
The function should return true if x is a square of y, otherwise false.

[FORMAL-THEOREM]
def problem_spec
(impl: Int → Int → Bool)
(x: Int)
(y: Int) :=
let spec (result: Bool) :=
result = true ↔ x = y^2;
∃ result, impl x y = result ∧
spec result

def implementation (x: Int) (y: Int) : Bool :=
if x = y * y then
  true
else
  false

theorem correctness
(x: Int)
(y: Int)
: problem_spec implementation x y

[INFORMAL-PROOF]
1. Start by unfolding the `problem_spec` and assigning the implementation's output to a temporary variable `result`.
2. Simplify the goal.
3. Use the `have` keyword to create a new hypothesis equating the operation of squaring a variable to that of multiplying the variable by itself.
4. Use this new hypothesis to rewrite the goal.

[STEPS]
[STEP] unfold problem_spec
[STEP] let result := implementation x y
[STEP] use result
[STEP] simp [result]

[LAST STEP]
simp [implementation]
[SUCCESS]
[END]

`example_assistant`
[RUN TACTIC]
have h_eq: y ^ 2 = y * y := by
[END]


`example_user`
Goals to prove:
[GOALS]
[DESCRIPTION]
IMPORTANT NOTE: Working on the sub-goal with have tactic:
have h_eq: y ^ 2 = y * y := by.

[GOAL] 1
y ^ 2 = y * y
[HYPOTHESES] 1
[HYPOTHESIS] x y : ℤ
[HYPOTHESIS] result : Bool := implementation x y

[INFORMAL-THEOREM]
Given two integers x and y, your task is to find if x is a square of y.
The function should return true if x is a square of y, otherwise false.

[FORMAL-THEOREM]
def problem_spec
(impl: Int → Int → Bool)
(x: Int)
(y: Int) :=
let spec (result: Bool) :=
result = true ↔ x = y^2;
∃ result, impl x y = result ∧
spec result

def implementation (x: Int) (y: Int) : Bool :=
if x = y * y then
  true
else
  false

theorem correctness
(x: Int)
(y: Int)
: problem_spec implementation x y

[INFORMAL-PROOF]
1. Start by unfolding the `problem_spec` and assigning the implementation's output to a temporary variable `result`.
2. Simplify the goal.
3. Use the `have` keyword to create a new hypothesis equating the operation of squaring a variable to that of multiplying the variable by itself.
4. Use this new hypothesis to rewrite the goal.

[STEPS]
[STEP] unfold problem_spec
[STEP] let result := implementation x y
[STEP] use result
[STEP] simp [result]
[STEP] simp [implementation]

[LAST STEP]
have h_eq: y ^ 2 = y * y := by
[SUCCESS]
[END]

`example_assistant`
[RUN TACTIC]
ring
[END]


`example_user`
Goals to prove:
[GOALS]
[GOAL] 1
x = y * y ↔ x = y ^ 2
[HYPOTHESES] 1
[HYPOTHESIS] x y : ℤ
[HYPOTHESIS] result : Bool := implementation x y
[HYPOTHESIS] h_eq : y ^ 2 = y * y

[INFORMAL-THEOREM]
Given two integers x and y, your task is to find if x is a square of y.
The function should return true if x is a square of y, otherwise false.

[FORMAL-THEOREM]
def problem_spec
(impl: Int → Int → Bool)
(x: Int)
(y: Int) :=
let spec (result: Bool) :=
result = true ↔ x = y^2;
∃ result, impl x y = result ∧
spec result

def implementation (x: Int) (y: Int) : Bool :=
if x = y * y then
  true
else
  false

theorem correctness
(x: Int)
(y: Int)
: problem_spec implementation x y

[INFORMAL-PROOF]
1. Start by unfolding the `problem_spec` and assigning the implementation's output to a temporary variable `result`.
2. Simplify the goal.
3. Use the `have` keyword to create a new hypothesis equating the operation of squaring a variable to that of multiplying the variable by itself.
4. Use this new hypothesis to rewrite the goal.

[STEPS]
[STEP] unfold problem_spec
[STEP] let result := implementation x y
[STEP] use result
[STEP] simp [result]
[STEP] simp [implementation]
[STEP] have h_eq: y ^ 2 = y * y := by

[LAST STEP]
ring
[SUCCESS]
[END]

`example_assistant`
[RUN TACTIC]
rw [h_eq]
[END]

`conv end`