`conv start`

`example_user`
Goals to prove:
[GOALS]
[GOAL] 1
(∀ (x y : ℤ), problem_spec impl x y) → ∀ (x y : ℤ), generated_spec impl x y
[HYPOTHESES] 1
[HYPOTHESIS] impl : ℤ → ℤ → Bool

[INFORMAL-THEOREM]
Given two integers x and y, your task is to find if x is a square of y.
The function should return true if x is a square of y, otherwise false.

[FORMAL-THEOREM]
def problem_spec
(impl: Int → Int → Bool)
(x: Int)
(y: Int) :=
let spec (result: Bool) :=
result = true ↔ x = y^2;
∃ result, impl x y = result ∧
spec result

def generated_spec
(impl: Int → Int → Bool)
(x: Int)
(y: Int) : Prop :=
impl x y = if x = y * y then true else false

theorem spec_isomorphism:
∀ impl,
(∀ x y, problem_spec impl x y) ↔
(∀ x y, generated_spec impl x y)

[INFORMAL-PROOF]
1. Start by analyzing the generated specification. The main idea is to create a specific instance of the generated specification and show that it satisfies the properties of the problem specification and vice versa.
2. Use `by_cases` to handle the case when x = y * y and when x ≠ y * y.
3. Then simplify `if-else` statements and use an instance of the problem specification to show that the two specifications are equivalent. You might also have to show that y * y = y ^ 2, this can be done using `ring`.
4. For the reverse direction, you can use similar reasoning.
5. Introduce the `h_specialized_spec` variable to represent the specialized version of the problem specification and show that it satisfies the generated specification.

[STEPS]
[STEP] intro impl
[STEP] apply Iff.intro

[LAST STEP]
unfold problem_spec
[ERROR MESSAGE]
The proof-step does NOT simplify the goal. Try stepping back with different proof-step.
[END]

`example_assistant`
[RUN TACTIC]
intro h_prob_spec
[END]


`example_user`
Goals to prove:
[GOALS]
[GOAL] 1
impl x = if x < 0 then -x else x
[HYPOTHESES] 1
[HYPOTHESIS] impl : ℤ → ℤ
[HYPOTHESIS] h_prob_spec : ∀ (x : ℤ),
[HYPOTHESIS]   0 ≤ impl x ∧
[HYPOTHESIS]     impl (-x) = impl x ∧
[HYPOTHESIS]       (impl x = 0 ↔ x = 0) ∧ (0 ≤ x → impl (-x) + impl x = 2 * x) ∧ (x ≤ 0 → impl (-x) + impl x = -(2 * x))
[HYPOTHESIS] x : ℤ

[GOAL] 2
(∀ (x : ℤ), impl x = if x < 0 then -x else x) →
  ∀ (x : ℤ),
    0 ≤ impl x ∧
      impl (-x) = impl x ∧
        (impl x = 0 ↔ x = 0) ∧ (0 ≤ x → impl (-x) + impl x = 2 * x) ∧ (x ≤ 0 → impl (-x) + impl x = -(2 * x))
[HYPOTHESES] 1
[HYPOTHESIS] impl : ℤ → ℤ

[INFORMAL-THEOREM]
Given an integer x, your task is to find the magnitude of x.
The magnitude of an integer is defined as the absolute value of the integer.

[FORMAL-THEOREM]
def problem_spec
(impl: Int → Int)
(x: Int) :=
let spec (result: Int) :=
(result ≥ 0) ∧
(impl (-x) = result) ∧
(result = 0 ↔ x = 0) ∧
(0 ≤ x → impl (-x) + result = 2 * x) ∧
(x ≤ 0 → impl (-x) + result = -2 * x)
∃ result, impl x = result ∧
spec result

def generated_spec
(impl: Int → Int)
(x: Int) : Prop :=
impl x = if x < 0 then -x else x

theorem spec_isomorphism:
∀ impl,
(∀ x y, problem_spec impl x y) ↔
(∀ x y, generated_spec impl x y)

[INFORMAL-PROOF]
1. Start by analyzing the generated specification. The original specification doesn't reveal the implementation details, but you can see that the generated specification is a simple if-else statement that checks if `x` is less than 0.
2. Use this information to write a proof that shows that the two specifications are equivalent.
3. Try different cases for `x`, and show that the properties of the generated specification hold true for the original specification as well.

[STEPS]
[STEP] unfold problem_spec
[STEP] unfold generated_spec
[STEP] simp
[STEP] intro impl
[STEP] apply Iff.intro
[STEP] intro h_prob_spec
[STEP] intro x

[INCORRECT STEPS]
[STEP] cases lt_or_ge x 0 with h_lt h_ge

[LAST STEP]
rw [h_prob_spec]

[ERROR MESSAGE]
tactic 'rewrite' failed, equality or iff proof expected
 0 ≤ impl ?x ∧
   impl (-?x) = impl ?x ∧
     (impl ?x = 0 ↔ ?x = 0) ∧ (0 ≤ ?x → impl (-?x) + impl ?x = 2 * ?x) ∧ (?x ≤ 0 → impl (-?x) + impl ?x = -(2 * ?x))
case mp
impl : ℤ → ℤ
h_prob_spec :
 ∀ (x : ℤ),
   0 ≤ impl x ∧
     impl (-x) = impl x ∧
       (impl x = 0 ↔ x = 0) ∧ (0 ≤ x → impl (-x) + impl x = 2 * x) ∧ (x ≤ 0 → impl (-x) + impl x = -(2 * x))
x : ℤ
⊢ impl x = if x < 0 then -x else x
[END]

`example_assistant`
[RUN TACTIC]
by_cases h_x_lt_0: x < 0
[END]


`example_user`
Goals to prove:
[GOALS]
[GOAL] 1
impl (-x) = impl x ∧
  (impl x = 0 ↔ x = 0) ∧ (0 ≤ x → impl (-x) + impl x = 2 * x) ∧ (x ≤ 0 → impl (-x) + impl x = -(2 * x))
[HYPOTHESES] 1
[HYPOTHESIS] impl : ℤ → ℤ
[HYPOTHESIS] h_generated_spec : ∀ (x : ℤ), impl x = if x < 0 then -x else x
[HYPOTHESIS] x : ℤ
[HYPOTHESIS] h_x_lt_0 : x < 0
[HYPOTHESIS] h_not_0_lt_x : ¬0 < x
[HYPOTHESIS] h_impl : impl x = -x
[HYPOTHESIS] h_0_le_impl_x : 0 ≤ impl x

[GOAL] 2
0 ≤ impl x ∧
  impl (-x) = impl x ∧
    (impl x = 0 ↔ x = 0) ∧ (0 ≤ x → impl (-x) + impl x = 2 * x) ∧ (x ≤ 0 → impl (-x) + impl x = -(2 * x))
[HYPOTHESES] 1
[HYPOTHESIS] impl : ℤ → ℤ
[HYPOTHESIS] h_generated_spec : ∀ (x : ℤ), impl x = if x < 0 then -x else x
[HYPOTHESIS] x : ℤ
[HYPOTHESIS] h_x_lt_0 : ¬x < 0

[INFORMAL-THEOREM]
Given an integer x, your task is to find the magnitude of x.
The magnitude of an integer is defined as the absolute value of the integer.

[FORMAL-THEOREM]
def problem_spec
(impl: Int → Int)
(x: Int) :=
let spec (result: Int) :=
(result ≥ 0) ∧
(impl (-x) = result) ∧
(result = 0 ↔ x = 0) ∧
(0 ≤ x → impl (-x) + result = 2 * x) ∧
(x ≤ 0 → impl (-x) + result = -2 * x)
∃ result, impl x = result ∧
spec result

def generated_spec
(impl: Int → Int)
(x: Int) : Prop :=
impl x = if x < 0 then -x else x

theorem spec_isomorphism:
∀ impl,
(∀ x y, problem_spec impl x y) ↔
(∀ x y, generated_spec impl x y)

[INFORMAL-PROOF]
1. Start by analyzing the generated specification. The original specification doesn't reveal the implementation details, but you can see that the generated specification is a simple if-else statement that checks if `x` is less than 0.
2. Use this information to write a proof that shows that the two specifications are equivalent.
3. Try different cases for `x`, and show that the properties of the generated specification hold true for the original specification as well.

[STEPS]
[STEP] unfold problem_spec
[STEP] unfold generated_spec
[STEP] simp
[STEP] intro impl
[STEP] apply Iff.intro
[STEP] intro h_prob_spec
[STEP] intro x
[STEP] by_cases h_x_lt_0: x < 0
[STEP] -- if x < 0 then
have h_x_le_0: x ≤ 0 := by
[STEP]   linarith
[STEP] simp [h_x_lt_0]
[STEP] have h_impl := h_prob_spec x
[STEP] simp [h_x_lt_0 ] at h_impl
[STEP] have h_neg_impl := h_impl.2.2.2
[STEP] simp [h_x_le_0] at h_neg_impl
[STEP] linarith
[STEP] simp [h_x_lt_0]
[STEP] have h_impl := h_prob_spec x
[STEP] simp at h_x_lt_0
[STEP] simp [h_x_lt_0] at h_impl
[STEP] have h_pos_impl := h_impl.2.2.2.1
[STEP] linarith
[STEP] intro h_generated_spec
[STEP] intro x
[STEP] by_cases h_x_lt_0: x < 0
[STEP] -- if x < 0 then
have h_not_0_lt_x: ¬ (0 < x) := by
[STEP]   linarith
[STEP] have h_impl := h_generated_spec x
[STEP] simp [h_x_lt_0] at h_impl
[STEP] have h_0_le_impl_x: 0 ≤ impl x := by
[STEP]   simp [h_impl]
[STEP]   linarith
[STEP] simp [h_0_le_impl_x]

[LAST STEP]
linarith [h_impl, h_0_le_impl_x, h_not_0_lt_x]

[ERROR MESSAGE]
linarith failed to find a contradiction
case pos
impl : ℤ → ℤ
h_generated_spec : ∀ (x : ℤ), impl x = if x < 0 then -x else x
x : ℤ
h_x_lt_0 : x < 0
h_not_0_lt_x : ¬0 < x
h_impl : impl x = -x
h_0_le_impl_x : 0 ≤ impl x
⊢ False
failed
[END]

`example_assistant`
[RUN TACTIC]
have h_impl_neg_x := h_generated_spec (-x)
[END]


`example_user`
Goals to prove:
[GOALS]
[GOAL] 1
impl (-x) = impl x ∧
  (impl x = 0 ↔ x = 0) ∧ (0 ≤ x → impl (-x) + impl x = 2 * x) ∧ (x ≤ 0 → impl (-x) + impl x = -(2 * x))
[HYPOTHESES] 1
[HYPOTHESIS] impl : ℤ → ℤ
[HYPOTHESIS] h_generated_spec : ∀ (x : ℤ), impl x = if x < 0 then -x else x
[HYPOTHESIS] x : ℤ
[HYPOTHESIS] h_x_lt_0 : x < 0
[HYPOTHESIS] h_not_0_lt_x : ¬0 < x
[HYPOTHESIS] h_impl : impl x = -x
[HYPOTHESIS] h_0_le_impl_x : 0 ≤ impl x
[HYPOTHESIS] h_impl_neg_x : impl (-x) = -x

[GOAL] 2
0 ≤ impl x ∧
  impl (-x) = impl x ∧
    (impl x = 0 ↔ x = 0) ∧ (0 ≤ x → impl (-x) + impl x = 2 * x) ∧ (x ≤ 0 → impl (-x) + impl x = -(2 * x))
[HYPOTHESES] 1
[HYPOTHESIS] impl : ℤ → ℤ
[HYPOTHESIS] h_generated_spec : ∀ (x : ℤ), impl x = if x < 0 then -x else x
[HYPOTHESIS] x : ℤ
[HYPOTHESIS] h_x_lt_0 : ¬x < 0

[INFORMAL-THEOREM]
Given an integer x, your task is to find the magnitude of x.
The magnitude of an integer is defined as the absolute value of the integer.

[FORMAL-THEOREM]
def problem_spec
(impl: Int → Int)
(x: Int) :=
let spec (result: Int) :=
(result ≥ 0) ∧
(impl (-x) = result) ∧
(result = 0 ↔ x = 0) ∧
(0 ≤ x → impl (-x) + result = 2 * x) ∧
(x ≤ 0 → impl (-x) + result = -2 * x)
∃ result, impl x = result ∧
spec result

def generated_spec
(impl: Int → Int)
(x: Int) : Prop :=
impl x = if x < 0 then -x else x

theorem spec_isomorphism:
∀ impl,
(∀ x y, problem_spec impl x y) ↔
(∀ x y, generated_spec impl x y)

[INFORMAL-PROOF]
1. Start by analyzing the generated specification. The original specification doesn't reveal the implementation details, but you can see that the generated specification is a simple if-else statement that checks if `x` is less than 0.
2. Use this information to write a proof that shows that the two specifications are equivalent.
3. Try different cases for `x`, and show that the properties of the generated specification hold true for the original specification as well.

[STEPS]
[STEP] unfold problem_spec
[STEP] unfold generated_spec
[STEP] simp
[STEP] intro impl
[STEP] apply Iff.intro
[STEP] intro h_prob_spec
[STEP] intro x
[STEP] by_cases h_x_lt_0: x < 0
[STEP] -- if x < 0 then
have h_x_le_0: x ≤ 0 := by
[STEP]   linarith
[STEP] simp [h_x_lt_0]
[STEP] have h_impl := h_prob_spec x
[STEP] simp [h_x_lt_0 ] at h_impl
[STEP] have h_neg_impl := h_impl.2.2.2
[STEP] simp [h_x_le_0] at h_neg_impl
[STEP] linarith
[STEP] simp [h_x_lt_0]
[STEP] have h_impl := h_prob_spec x
[STEP] simp at h_x_lt_0
[STEP] simp [h_x_lt_0] at h_impl
[STEP] have h_pos_impl := h_impl.2.2.2.1
[STEP] linarith
[STEP] intro h_generated_spec
[STEP] intro x
[STEP] by_cases h_x_lt_0: x < 0
[STEP] -- if x < 0 then
have h_not_0_lt_x: ¬ (0 < x) := by
[STEP]   linarith
[STEP] have h_impl := h_generated_spec x
[STEP] simp [h_x_lt_0] at h_impl
[STEP] have h_0_le_impl_x: 0 ≤ impl x := by
[STEP]   simp [h_impl]
[STEP]   linarith
[STEP] simp [h_0_le_impl_x]
[STEP] have h_impl_neg_x := h_generated_spec (-x)
[STEP] simp [h_x_lt_0] at h_impl_neg_x

[LAST STEP]
simp [h_not_0_lt_x] at h_impl_neg_x
[SUCCESS]
[END]

`example_assistant`
[RUN TACTIC]
rw [←h_impl_neg_x] at h_impl
[END]


`example_user`
Goals to prove:
[GOALS]
[GOAL] 1
impl (y * y) y = true
[HYPOTHESES] 1
[HYPOTHESIS] impl : ℤ → ℤ → Bool
[HYPOTHESIS] h_prob_spec : ∀ (x y : ℤ), problem_spec impl x y
[HYPOTHESIS] x y : ℤ
[HYPOTHESIS] h_specialized_spec : problem_spec impl x y
[HYPOTHESIS] h : x = y * y

[GOAL] 2
impl x y = decide (x = y * y)
[HYPOTHESES] 1
[HYPOTHESIS] impl : ℤ → ℤ → Bool
[HYPOTHESIS] h_prob_spec : ∀ (x y : ℤ), problem_spec impl x y
[HYPOTHESIS] x y : ℤ
[HYPOTHESIS] h_specialized_spec : problem_spec impl x y
[HYPOTHESIS] h : ¬x = y * y

[GOAL] 3
(∀ (x y : ℤ), generated_spec impl x y) → ∀ (x y : ℤ), problem_spec impl x y
[HYPOTHESES] 1
[HYPOTHESIS] impl : ℤ → ℤ → Bool

[INFORMAL-THEOREM]
Given two integers x and y, your task is to find if x is a square of y.
The function should return true if x is a square of y, otherwise false.

[FORMAL-THEOREM]
def problem_spec
(impl: Int → Int → Bool)
(x: Int)
(y: Int) :=
let spec (result: Bool) :=
result = true ↔ x = y^2;
∃ result, impl x y = result ∧
spec result

def generated_spec
(impl: Int → Int → Bool)
(x: Int)
(y: Int) : Prop :=
impl x y = if x = y * y then true else false

theorem spec_isomorphism:
∀ impl,
(∀ x y, problem_spec impl x y) ↔
(∀ x y, generated_spec impl x y)

[INFORMAL-PROOF]
1. Start by analyzing the generated specification. The main idea is to create a specific instance of the generated specification and show that it satisfies the properties of the problem specification and vice versa.
2. Use `by_cases` to handle the case when x = y * y and when x ≠ y * y.
3. Then simplify `if-else` statements and use an instance of the problem specification to show that the two specifications are equivalent. You might also have to show that y * y = y ^ 2, this can be done using `ring`.
4. For the reverse direction, you can use similar reasoning.
5. Introduce the `h_specialized_spec` variable to represent the specialized version of the problem specification and show that it satisfies the generated specification.

[STEPS]
[STEP] intro impl
[STEP] apply Iff.intro
[STEP] intro h_prob_spec
[STEP] intro x y
[STEP] have h_specialized_spec := h_prob_spec x y
[STEP] simp [generated_spec]
[STEP] by_cases h: x = y * y

[LAST STEP]
simp [h]
[SUCCESS]
[END]

`example_assistant`
[RUN TACTIC]
simp [problem_spec] at h_specialized_spec
[END]


`example_user`
Goals to prove:
[GOALS]
[GOAL] 1
impl x y = false
[HYPOTHESES] 1
[HYPOTHESIS] impl : ℤ → ℤ → Bool
[HYPOTHESIS] h_prob_spec : ∀ (x y : ℤ), problem_spec impl x y
[HYPOTHESIS] x y : ℤ
[HYPOTHESIS] h : ¬x = y * y
[HYPOTHESIS] h_specialized_spec : impl x y = true ↔ x = y ^ 2

[GOAL] 2
(∀ (x y : ℤ), generated_spec impl x y) → ∀ (x y : ℤ), problem_spec impl x y
[HYPOTHESES] 1
[HYPOTHESIS] impl : ℤ → ℤ → Bool

[INFORMAL-THEOREM]
Given two integers x and y, your task is to find if x is a square of y.
The function should return true if x is a square of y, otherwise false.

[FORMAL-THEOREM]
def problem_spec
(impl: Int → Int → Bool)
(x: Int)
(y: Int) :=
let spec (result: Bool) :=
result = true ↔ x = y^2;
∃ result, impl x y = result ∧
spec result

def generated_spec
(impl: Int → Int → Bool)
(x: Int)
(y: Int) : Prop :=
impl x y = if x = y * y then true else false

theorem spec_isomorphism:
∀ impl,
(∀ x y, problem_spec impl x y) ↔
(∀ x y, generated_spec impl x y)

[INFORMAL-PROOF]
1. Start by analyzing the generated specification. The main idea is to create a specific instance of the generated specification and show that it satisfies the properties of the problem specification and vice versa.
2. Use `by_cases` to handle the case when x = y * y and when x ≠ y * y.
3. Then simplify `if-else` statements and use an instance of the problem specification to show that the two specifications are equivalent. You might also have to show that y * y = y ^ 2, this can be done using `ring`.
4. For the reverse direction, you can use similar reasoning.
5. Introduce the `h_specialized_spec` variable to represent the specialized version of the problem specification and show that it satisfies the generated specification.

[STEPS]
[STEP] intro impl
[STEP] apply Iff.intro
[STEP] intro h_prob_spec
[STEP] intro x y
[STEP] have h_specialized_spec := h_prob_spec x y
[STEP] simp [generated_spec]
[STEP] by_cases h: x = y * y
[STEP] simp [h]
[STEP] simp [problem_spec] at h_specialized_spec
[STEP] rw [h] at h_specialized_spec
[STEP] simp [h_specialized_spec]
[STEP] ring
[STEP] simp [h]

[LAST STEP]
simp [problem_spec] at h_specialized_spec
[SUCCESS]
[END]

`example_assistant`
[RUN TACTIC]
have h_eq: y ^ 2 = y * y := by
[END]


`example_user`
Goals to prove:
[GOALS]
[DESCRIPTION]
IMPORTANT NOTE: Working on the sub-goal with have tactic:
have h_eq: y ^ 2 = y * y := by.

[GOAL] 1
y ^ 2 = y * y
[HYPOTHESES] 1
[HYPOTHESIS] impl : ℤ → ℤ → Bool
[HYPOTHESIS] h_prob_spec : ∀ (x y : ℤ), problem_spec impl x y
[HYPOTHESIS] x y : ℤ
[HYPOTHESIS] h : ¬x = y * y
[HYPOTHESIS] h_specialized_spec : impl x y = true ↔ x = y ^ 2

[INFORMAL-THEOREM]
Given two integers x and y, your task is to find if x is a square of y.
The function should return true if x is a square of y, otherwise false.

[FORMAL-THEOREM]
def problem_spec
(impl: Int → Int → Bool)
(x: Int)
(y: Int) :=
let spec (result: Bool) :=
result = true ↔ x = y^2;
∃ result, impl x y = result ∧
spec result

def generated_spec
(impl: Int → Int → Bool)
(x: Int)
(y: Int) : Prop :=
impl x y = if x = y * y then true else false

theorem spec_isomorphism:
∀ impl,
(∀ x y, problem_spec impl x y) ↔
(∀ x y, generated_spec impl x y)

[INFORMAL-PROOF]
1. Start by analyzing the generated specification. The main idea is to create a specific instance of the generated specification and show that it satisfies the properties of the problem specification and vice versa.
2. Use `by_cases` to handle the case when x = y * y and when x ≠ y * y.
3. Then simplify `if-else` statements and use an instance of the problem specification to show that the two specifications are equivalent. You might also have to show that y * y = y ^ 2, this can be done using `ring`.
4. For the reverse direction, you can use similar reasoning.
5. Introduce the `h_specialized_spec` variable to represent the specialized version of the problem specification and show that it satisfies the generated specification.

[STEPS]
[STEP] intro impl
[STEP] apply Iff.intro
[STEP] intro h_prob_spec
[STEP] intro x y
[STEP] have h_specialized_spec := h_prob_spec x y
[STEP] simp [generated_spec]
[STEP] by_cases h: x = y * y
[STEP] simp [h]
[STEP] simp [problem_spec] at h_specialized_spec
[STEP] rw [h] at h_specialized_spec
[STEP] simp [h_specialized_spec]
[STEP] ring
[STEP] simp [h]
[STEP] simp [problem_spec] at h_specialized_spec

[LAST STEP]
have h_eq: y ^ 2 = y * y := by
[SUCCESS]
[END]

`example_assistant`
[RUN TACTIC]
ring
[END]

`example_user`
Goals to prove:
[GOALS]
[GOAL] 1
generated_spec impl x y
[HYPOTHESES] 1
[HYPOTHESIS] impl : ℤ → ℤ → Bool
[HYPOTHESIS] h_prob_spec : ∀ (x y : ℤ), problem_spec impl x y
[HYPOTHESIS] x y : ℤ

[INFORMAL-THEOREM]
Given two integers x and y, your task is to find if x is a square of y.
The function should return true if x is a square of y, otherwise false.

[FORMAL-THEOREM]
def problem_spec
(impl: Int → Int → Bool)
(x: Int)
(y: Int) :=
let spec (result: Bool) :=
result = true ↔ x = y^2;
∃ result, impl x y = result ∧
spec result

def generated_spec
(impl: Int → Int → Bool)
(x: Int)
(y: Int) : Prop :=
impl x y = if x = y * y then true else false

theorem spec_isomorphism:
∀ impl,
(∀ x y, generated_spec impl x y) ↔
(∀ x y, problem_spec impl x y)

[INFORMAL-PROOF]
1. Start by analyzing the generated specification. The main idea is to create a specific instance of the generated specification and show that it satisfies the properties of the problem specification and vice versa.
2. Use `by_cases` to handle the case when x = y * y and when x ≠ y * y.
3. Then simplify `if-else` statements and use an instance of the problem specification to show that the two specifications are equivalent. You might also have to show that y * y = y ^ 2, this can be done using `ring`.
4. For the reverse direction, you can use similar reasoning.
5. Introduce the `h_specialized_spec` variable to represent the specialized version of the problem specification and show that it satisfies the generated specification.

[STEPS]
[STEP] intro impl
[STEP] apply Iff.intro
[STEP] intro h_prob_spec

[LAST STEP]
intro x y
[SUCCESS]
[END]

`example_assistant`
[RUN TACTIC]
have h_specialized_spec := h_prob_spec x y
[END]

`example_user`
Goals to prove:
[GOALS]
[GOAL] 1
∃ result, impl x y = result ∧ (result = true ↔ x = y ^ 2)
[HYPOTHESES] 1
[HYPOTHESIS] impl : ℤ → ℤ → Bool
[HYPOTHESIS] h_gen_spec : ∀ (x y : ℤ), generated_spec impl x y
[HYPOTHESIS] x y : ℤ

[INFORMAL-THEOREM]
Given two integers x and y, your task is to find if x is a square of y.
The function should return true if x is a square of y, otherwise false.

[FORMAL-THEOREM]
def problem_spec
(impl: Int → Int → Bool)
(x: Int)
(y: Int) :=
let spec (result: Bool) :=
result = true ↔ x = y^2;
∃ result, impl x y = result ∧
spec result

def generated_spec
(impl: Int → Int → Bool)
(x: Int)
(y: Int) : Prop :=
impl x y = if x = y * y then true else false

theorem spec_isomorphism:
∀ impl,
(∀ x y, generated_spec impl x y) ↔
(∀ x y, problem_spec impl x y)

[INFORMAL-PROOF]
1. Start by analyzing the generated specification. The main idea is to create a specific instance of the generated specification and show that it satisfies the properties of the problem specification and vice versa.
2. It is important to note that we should not use specific implementation details in the proof because the specification has to be proven for all implementations. So assuming a specific implementation is not a good idea.
3. Use `by_cases` to handle the case when x = y * y and when x ≠ y * y.
4. Then simplify `if-else` statements and use an instance of the problem specification to show that the two specifications are equivalent. You might also have to show that y * y = y ^ 2, this can be done using `ring`.
5. For the reverse direction, you can use similar reasoning.
6. Introduce the `h_specialized_spec` variable to represent the specialized version of the problem specification and show that it satisfies the generated specification.

[STEPS]
[STEP] intro impl
[STEP] apply Iff.intro
[STEP] intro h_gen_spec
[STEP] intro x y
[STEP] unfold problem_spec
[STEP] simp only

[LAST STEP]
use y * y = x
[ERROR MESSAGE]
The proof-step does NOT simplify the goal. Try stepping back with different proof-step.
[END]

`example_assistant`
[RUN TACTIC]
-- let's use generic implementation rather than specific implementation 
use (impl x y)
[END]

`example_user`
Goals to prove:
[GOALS]
[GOAL] 1
impl x y = true ↔ x = y ^ 2
[HYPOTHESES] 1
[HYPOTHESIS] impl : ℤ → ℤ → Bool
[HYPOTHESIS] h_gen_spec : ∀ (x y : ℤ), generated_spec impl x y
[HYPOTHESIS] x y : ℤ

[INFORMAL-THEOREM]
Given two integers x and y, your task is to find if x is a square of y.
The function should return true if x is a square of y, otherwise false.

[FORMAL-THEOREM]
def problem_spec
(impl: Int → Int → Bool)
(x: Int)
(y: Int) :=
let spec (result: Bool) :=
result = true ↔ x = y^2;
∃ result, impl x y = result ∧
spec result

def generated_spec
(impl: Int → Int → Bool)
(x: Int)
(y: Int) : Prop :=
impl x y = if x = y * y then true else false

theorem spec_isomorphism:
∀ impl,
(∀ x y, generated_spec impl x y) ↔
(∀ x y, problem_spec impl x y)

[INFORMAL-PROOF]
1. Start by analyzing the generated specification. The main idea is to create a specific instance of the generated specification and show that it satisfies the properties of the problem specification and vice versa.
2. It is important to note that we should not use specific implementation details in the proof because the specification has to be proven for all implementations. So assuming a specific implementation is not a good idea.
3. Use `by_cases` to handle the case when x = y * y and when x ≠ y * y.
4. Then simplify `if-else` statements and use an instance of the problem specification to show that the two specifications are equivalent. You might also have to show that y * y = y ^ 2, this can be done using `ring`.
5. For the reverse direction, you can use similar reasoning.
6. Introduce the `h_specialized_spec` variable to represent the specialized version of the problem specification and show that it satisfies the generated specification.

[STEPS]
[STEP] intro impl
[STEP] apply Iff.intro
[STEP] intro h_gen_spec
[STEP] intro x y
[STEP] unfold problem_spec
[STEP] simp only
[STEP] use (impl x y)
[STEP] simp

[LAST STEP]
simp
[SUCCESS]
[END]

`example_assistant`
[RUN TACTIC]
-- it is not possible to further simplify the goal without using the generated_spec, so let's expand it and see how it looks like
unfold generated_spec at h_gen_spec
[END]

`example_user`
Goals to prove:
[GOALS]
[GOAL] 1
(∀ (x y : ℤ), problem_spec impl x y) → ∀ (x y : ℤ), generated_spec impl x y

[INFORMAL-THEOREM]
Given two integers x and y, your task is to find if x is a square of y.
The function should return true if x is a square of y, otherwise false.

[FORMAL-THEOREM]
def problem_spec
(impl: Int → Int → Bool)
(x: Int)
(y: Int) :=
let spec (result: Bool) :=
result = true ↔ x = y^2;
∃ result, impl x y = result ∧
spec result

def generated_spec
(impl: Int → Int → Bool)
(x: Int)
(y: Int) : Prop :=
impl x y = if x = y * y then true else false

theorem spec_isomorphism:
∀ impl,
(∀ x y, generated_spec impl x y) ↔
(∀ x y, problem_spec impl x y)

[INFORMAL-PROOF]
1. Start by analyzing the generated specification. The main idea is to create a specific instance of the generated specification and show that it satisfies the properties of the problem specification and vice versa.
2. It is important to note that we should not use specific implementation details in the proof because the specification has to be proven for all implementations. So assuming a specific implementation is not a good idea.
3. Use `by_cases` to handle the case when x = y * y and when x ≠ y * y.
4. Then simplify `if-else` statements and use an instance of the problem specification to show that the two specifications are equivalent. You might also have to show that y * y = y ^ 2, this can be done using `ring`.
5. For the reverse direction, you can use similar reasoning.
6. Introduce the `h_specialized_spec` variable to represent the specialized version of the problem specification and show that it satisfies the generated specification.

[STEPS]
[STEP] intro impl
[STEP] apply Iff.intro
[STEP] intro h_gen_spec
[STEP] intro x y
[STEP] unfold problem_spec
[STEP] simp only
[STEP] use (impl x y)
[STEP] simp
[STEP] unfold generated_spec at h_gen_spec
[STEP] have h_specialized_spec := h_gen_spec x y
[STEP] simp [h_specialized_spec]
[STEP] apply Iff.intro
[STEP] intro h_y_times_y
[STEP] linarith
[STEP] intro h_y_square
[STEP] simp [h_y_square]

[LAST STEP]
ring
[SUCCESS]
[END]

`example_assistant`
[RUN TACTIC]
-- we need to prove the reverse direction, so let's introduce the problem_spec
intro h_prob_spec
[END]


`example_user`
Goals to prove:
[GOALS]
[GOAL] 1
∃ f₁ f₂, fibonacci_non_computable n f₁ ∧ fibonacci_non_computable (n + 1) f₂ ∧ f₁✝ + f₂✝ = f₁ + f₂
[HYPOTHESES] 1
[HYPOTHESIS] n f₁✝ f₂✝ : ℕ
[HYPOTHESIS] a✝¹ : fibonacci_non_computable n f₁✝
[HYPOTHESIS] a✝ : fibonacci_non_computable (n + 1) f₂✝

[GOAL] 2
(∃ f₁ f₂, fibonacci_non_computable n f₁ ∧ fibonacci_non_computable (n + 1) f₂ ∧ m = f₁ + f₂) →
  fibonacci_non_computable (n + 2) m
[HYPOTHESES] 1
[HYPOTHESIS] n m : ℕ

[INFORMAL-THEOREM]
Prove a `fib_rec_unique` lemma that states the recursive property of Fibonacci numbers fully using `fibonacci_non_computable`.

[FORMAL-THEOREM]
inductive fibonacci_non_computable : ℕ → ℕ → Prop
| base0 : fibonacci_non_computable 0 0
| base1 : fibonacci_non_computable 1 1
| step  : ∀ n f₁ f₂, fibonacci_non_computable n f₁ →
fibonacci_non_computable (n + 1) f₂ →
fibonacci_non_computable (n + 2) (f₁ + f₂)

def problem_spec
(impl: Nat → Nat)
(n: Nat) :=
let spec (result: Nat) :=
fibonacci_non_computable n result
∃ result, impl n = result ∧
spec result

def generated_spec
(impl: Nat → Nat)
(n: Nat) : Prop :=
let spec (result: Nat) :=
match n with
| 0 => result = 0
| 1 => result = 1
| n' + 2 => result = impl n' + impl (n' + 1)
∃ result, impl n = result ∧
spec result

lemma fib_rec_unique (n m : ℕ):
  fibonacci_non_computable (n + 2) m ↔
  ∃ f₁ f₂, fibonacci_non_computable n f₁ ∧
  fibonacci_non_computable (n + 1) f₂ ∧
  m = f₁ + f₂

[INFORMAL-PROOF]
1. Start by splitting the "iff".
2. Use `fibonacci_non_computable.step`.

Throughout the proof, you can freely use any of the below helper lemmas, which you can assume to be true:
[HELPER LEMMAS]
[HELPER LEMMA]
lemma fib0_unique (n : ℕ) (h : fibonacci_non_computable 0 n) : n = 0 :=
[HELPER LEMMA]
lemma fib1_unique (n : ℕ) (h : fibonacci_non_computable 1 n) : n = 1 :=

[STEPS]
[STEP] apply Iff.intro
[STEP] intro h

[LAST STEP]
cases h
[SUCCESS]
[END]

`example_assistant`
[RUN TACTIC]
rename_i f₁ f₂ h₁ h₂
[END]


`example_user`
Goals to prove:
[GOALS]
[GOAL] 1
fibonacci_non_computable (n + 2) m
[HYPOTHESES] 1
[HYPOTHESIS] n m : ℕ
[HYPOTHESIS] h : ∃ f₁ f₂, fibonacci_non_computable n f₁ ∧ fibonacci_non_computable (n + 1) f₂ ∧ m = f₁ + f₂

[INFORMAL-THEOREM]
Prove a `fib_rec_unique` lemma that states the recursive property of Fibonacci numbers fully using `fibonacci_non_computable`.

[FORMAL-THEOREM]
inductive fibonacci_non_computable : ℕ → ℕ → Prop
| base0 : fibonacci_non_computable 0 0
| base1 : fibonacci_non_computable 1 1
| step  : ∀ n f₁ f₂, fibonacci_non_computable n f₁ →
fibonacci_non_computable (n + 1) f₂ →
fibonacci_non_computable (n + 2) (f₁ + f₂)

def problem_spec
(impl: Nat → Nat)
(n: Nat) :=
let spec (result: Nat) :=
fibonacci_non_computable n result
∃ result, impl n = result ∧
spec result

def generated_spec
(impl: Nat → Nat)
(n: Nat) : Prop :=
let spec (result: Nat) :=
match n with
| 0 => result = 0
| 1 => result = 1
| n' + 2 => result = impl n' + impl (n' + 1)
∃ result, impl n = result ∧
spec result

lemma fib_rec_unique (n m : ℕ):
  fibonacci_non_computable (n + 2) m ↔
  ∃ f₁ f₂, fibonacci_non_computable n f₁ ∧
  fibonacci_non_computable (n + 1) f₂ ∧
  m = f₁ + f₂

[INFORMAL-PROOF]
1. Start by splitting the "iff".
2. Use `fibonacci_non_computable.step`.

Throughout the proof, you can freely use any of the below helper lemmas, which you can assume to be true:
[HELPER LEMMAS]
[HELPER LEMMA]
lemma fib0_unique (n : ℕ) (h : fibonacci_non_computable 0 n) : n = 0 :=
[HELPER LEMMA]
lemma fib1_unique (n : ℕ) (h : fibonacci_non_computable 1 n) : n = 1 :=

[STEPS]
[STEP] apply Iff.intro
[STEP] intro h
[STEP] cases h
[STEP] rename_i f₁ f₂ h₁ h₂
[STEP] use f₁
[STEP] use f₂

[LAST STEP]
intro h
[SUCCESS]
[END]

`example_assistant`
[RUN TACTIC]
obtain ⟨f₁, f₂, h₁, h₂, h_eq⟩ := h
[END]


`example_user`
Goals to prove:
[GOALS]
[GOAL] 1
fibonacci_non_computable (n + 2) (f₁ + f₂)
[HYPOTHESES] 1
[HYPOTHESIS] n m f₁ f₂ : ℕ
[HYPOTHESIS] h₁ : fibonacci_non_computable n f₁
[HYPOTHESIS] h₂ : fibonacci_non_computable (n + 1) f₂
[HYPOTHESIS] h_eq : m = f₁ + f₂

[INFORMAL-THEOREM]
Prove a `fib_rec_unique` lemma that states the recursive property of Fibonacci numbers fully using `fibonacci_non_computable`.

[FORMAL-THEOREM]
inductive fibonacci_non_computable : ℕ → ℕ → Prop
| base0 : fibonacci_non_computable 0 0
| base1 : fibonacci_non_computable 1 1
| step  : ∀ n f₁ f₂, fibonacci_non_computable n f₁ →
fibonacci_non_computable (n + 1) f₂ →
fibonacci_non_computable (n + 2) (f₁ + f₂)

def problem_spec
(impl: Nat → Nat)
(n: Nat) :=
let spec (result: Nat) :=
fibonacci_non_computable n result
∃ result, impl n = result ∧
spec result

def generated_spec
(impl: Nat → Nat)
(n: Nat) : Prop :=
let spec (result: Nat) :=
match n with
| 0 => result = 0
| 1 => result = 1
| n' + 2 => result = impl n' + impl (n' + 1)
∃ result, impl n = result ∧
spec result

lemma fib_rec_unique (n m : ℕ):
  fibonacci_non_computable (n + 2) m ↔
  ∃ f₁ f₂, fibonacci_non_computable n f₁ ∧
  fibonacci_non_computable (n + 1) f₂ ∧
  m = f₁ + f₂

[INFORMAL-PROOF]
1. Start by splitting the "iff".
2. Use `fibonacci_non_computable.step`.

Throughout the proof, you can freely use any of the below helper lemmas, which you can assume to be true:
[HELPER LEMMAS]
[HELPER LEMMA]
lemma fib0_unique (n : ℕ) (h : fibonacci_non_computable 0 n) : n = 0 :=
[HELPER LEMMA]
lemma fib1_unique (n : ℕ) (h : fibonacci_non_computable 1 n) : n = 1 :=

[STEPS]
[STEP] apply Iff.intro
[STEP] intro h
[STEP] cases h
[STEP] rename_i f₁ f₂ h₁ h₂
[STEP] use f₁
[STEP] use f₂
[STEP] intro h
[STEP] obtain ⟨f₁, f₂, h₁, h₂, h_eq⟩ := h

[LAST STEP]
rw [h_eq]
[SUCCESS]
[END]

`example_assistant`
[RUN TACTIC]
exact fibonacci_non_computable.step _ _ _ h₁ h₂
[END]


`example_user`
Goals to prove:
[GOALS]
[GOAL] 1
∀ (f₁ f₂ : ℕ), fibonacci_non_computable n f₁ → fibonacci_non_computable n f₂ → f₁ = f₂
[HYPOTHESES] 1
[HYPOTHESIS] n : ℕ

[INFORMAL-THEOREM]
Prove a `fib_inversion` lemma that states that the `n`th Fibonacci number is unique, according to `fibonacci_non_computable`.

[FORMAL-THEOREM]
inductive fibonacci_non_computable : ℕ → ℕ → Prop
| base0 : fibonacci_non_computable 0 0
| base1 : fibonacci_non_computable 1 1
| step  : ∀ n f₁ f₂, fibonacci_non_computable n f₁ →
fibonacci_non_computable (n + 1) f₂ →
fibonacci_non_computable (n + 2) (f₁ + f₂)

def problem_spec
(impl: Nat → Nat)
(n: Nat) :=
let spec (result: Nat) :=
fibonacci_non_computable n result
∃ result, impl n = result ∧
spec result

def generated_spec
(impl: Nat → Nat)
(n: Nat) : Prop :=
let spec (result: Nat) :=
match n with
| 0 => result = 0
| 1 => result = 1
| n' + 2 => result = impl n' + impl (n' + 1)
∃ result, impl n = result ∧
spec result

lemma fib_inversion (n f₁ f₂ : ℕ)
(h : fibonacci_non_computable n f₁) (h' : fibonacci_non_computable n f₂) :
  f₁ = f₂

[INFORMAL-PROOF]
1. Use strong induction on `n`.
2. Use the `fib_rec_unique` lemma.

Throughout the proof, you can freely use any of the below helper lemmas, which you can assume to be true:
[HELPER LEMMAS]
[HELPER LEMMA]
lemma fib0_unique (n : ℕ) (h : fibonacci_non_computable 0 n) : n = 0 :=
[HELPER LEMMA]
lemma fib1_unique (n : ℕ) (h : fibonacci_non_computable 1 n) : n = 1 :=
[HELPER LEMMA]
lemma fib_rec_unique (n m : ℕ):
  fibonacci_non_computable (n + 2) m ↔
  ∃ f₁ f₂, fibonacci_non_computable n f₁ ∧
  fibonacci_non_computable (n + 1) f₂ ∧
  m = f₁ + f₂ :=

[LAST STEP]
revert f₁ f₂
[SUCCESS]
[END]

`example_assistant`
[RUN TACTIC]
induction' n using Nat.strong_induction_on with n' ih
[END]


`example_user`
Goals to prove:
[GOALS]
[DESCRIPTION]
IMPORTANT NOTE: Working on the sub-goal with have tactic:
have h_n'_eq_0: n' = 0 ∨ n' = 1 := by.

[GOAL] 1
n' = 0 ∨ n' = 1
[HYPOTHESES] 1
[HYPOTHESIS] n' : ℕ
[HYPOTHESIS] ih : ∀ m < n', ∀ (f₁ f₂ : ℕ), fibonacci_non_computable m f₁ → fibonacci_non_computable m f₂ → f₁ = f₂
[HYPOTHESIS] f₁ f₂ : ℕ
[HYPOTHESIS] h_n'_lt_1 : n' < 2
[HYPOTHESIS] h : fibonacci_non_computable n' f₁
[HYPOTHESIS] h' : fibonacci_non_computable n' f₂

[INFORMAL-THEOREM]
Prove a `fib_inversion` lemma that states that the `n`th Fibonacci number is unique, according to `fibonacci_non_computable`.

[FORMAL-THEOREM]
inductive fibonacci_non_computable : ℕ → ℕ → Prop
| base0 : fibonacci_non_computable 0 0
| base1 : fibonacci_non_computable 1 1
| step  : ∀ n f₁ f₂, fibonacci_non_computable n f₁ →
fibonacci_non_computable (n + 1) f₂ →
fibonacci_non_computable (n + 2) (f₁ + f₂)

def problem_spec
(impl: Nat → Nat)
(n: Nat) :=
let spec (result: Nat) :=
fibonacci_non_computable n result
∃ result, impl n = result ∧
spec result

def generated_spec
(impl: Nat → Nat)
(n: Nat) : Prop :=
let spec (result: Nat) :=
match n with
| 0 => result = 0
| 1 => result = 1
| n' + 2 => result = impl n' + impl (n' + 1)
∃ result, impl n = result ∧
spec result

lemma fib_inversion (n f₁ f₂ : ℕ)
(h : fibonacci_non_computable n f₁) (h' : fibonacci_non_computable n f₂) :
  f₁ = f₂

[INFORMAL-PROOF]
1. Use strong induction on `n`.
2. Use the `fib_rec_unique` lemma.

Throughout the proof, you can freely use any of the below helper lemmas, which you can assume to be true:
[HELPER LEMMAS]
[HELPER LEMMA]
lemma fib0_unique (n : ℕ) (h : fibonacci_non_computable 0 n) : n = 0 :=
[HELPER LEMMA]
lemma fib1_unique (n : ℕ) (h : fibonacci_non_computable 1 n) : n = 1 :=
[HELPER LEMMA]
lemma fib_rec_unique (n m : ℕ):
  fibonacci_non_computable (n + 2) m ↔
  ∃ f₁ f₂, fibonacci_non_computable n f₁ ∧
  fibonacci_non_computable (n + 1) f₂ ∧
  m = f₁ + f₂ :=

[STEPS]
[STEP] revert f₁ f₂
[STEP] induction' n using Nat.strong_induction_on with n' ih
[STEP] intro f₁ f₂
[STEP] by_cases h_n'_lt_1: n' < 2
[STEP] intro h h'

[LAST STEP]
-- if n' < 1 then
have h_n'_eq_0: n' = 0 ∨ n' = 1 := by
[SUCCESS]
[END]

`example_assistant`
[RUN TACTIC]
interval_cases n'
[END]


`example_user`
Goals to prove:
[GOALS]
[GOAL] 1
f₁ = f₂
[HYPOTHESES] 1
[HYPOTHESIS] n' f₁ f₂ : ℕ
[HYPOTHESIS] n'' : ℕ := n' - 2
[HYPOTHESIS] ih : ∀ m < n'' + 2, ∀ (f₁ f₂ : ℕ), fibonacci_non_computable m f₁ → fibonacci_non_computable m f₂ → f₁ = f₂
[HYPOTHESIS] h : fibonacci_non_computable (n'' + 2) f₁
[HYPOTHESIS] h' : fibonacci_non_computable (n'' + 2) f₂

[INFORMAL-THEOREM]
Prove a `fib_inversion` lemma that states that the `n`th Fibonacci number is unique, according to `fibonacci_non_computable`.

[FORMAL-THEOREM]
inductive fibonacci_non_computable : ℕ → ℕ → Prop
| base0 : fibonacci_non_computable 0 0
| base1 : fibonacci_non_computable 1 1
| step  : ∀ n f₁ f₂, fibonacci_non_computable n f₁ →
fibonacci_non_computable (n + 1) f₂ →
fibonacci_non_computable (n + 2) (f₁ + f₂)

def problem_spec
(impl: Nat → Nat)
(n: Nat) :=
let spec (result: Nat) :=
fibonacci_non_computable n result
∃ result, impl n = result ∧
spec result

def generated_spec
(impl: Nat → Nat)
(n: Nat) : Prop :=
let spec (result: Nat) :=
match n with
| 0 => result = 0
| 1 => result = 1
| n' + 2 => result = impl n' + impl (n' + 1)
∃ result, impl n = result ∧
spec result

lemma fib_inversion (n f₁ f₂ : ℕ)
(h : fibonacci_non_computable n f₁) (h' : fibonacci_non_computable n f₂) :
  f₁ = f₂

[INFORMAL-PROOF]
1. Use strong induction on `n`.
2. Use the `fib_rec_unique` lemma.

Throughout the proof, you can freely use any of the below helper lemmas, which you can assume to be true:
[HELPER LEMMAS]
[HELPER LEMMA]
lemma fib0_unique (n : ℕ) (h : fibonacci_non_computable 0 n) : n = 0 :=
[HELPER LEMMA]
lemma fib1_unique (n : ℕ) (h : fibonacci_non_computable 1 n) : n = 1 :=
[HELPER LEMMA]
lemma fib_rec_unique (n m : ℕ):
  fibonacci_non_computable (n + 2) m ↔
  ∃ f₁ f₂, fibonacci_non_computable n f₁ ∧
  fibonacci_non_computable (n + 1) f₂ ∧
  m = f₁ + f₂ :=

[STEPS]
[STEP] revert f₁ f₂
[STEP] induction' n using Nat.strong_induction_on with n' ih
[STEP] intro f₁ f₂
[STEP] by_cases h_n'_lt_1: n' < 2
[STEP] intro h h'
[STEP] -- if n' < 1 then
have h_n'_eq_0: n' = 0 ∨ n' = 1 := by
[STEP]   interval_cases n'
[STEP]   all_goals simp
[STEP] cases h_n'_eq_0
[STEP] rename_i h_n'_eq_0
[STEP] simp [h_n'_eq_0] at *
[STEP] cases h
[STEP] cases h'
[STEP] rfl
[STEP] rename_i h_n'_eq_1
[STEP] simp [h_n'_eq_1] at *
[STEP] clear h_n'_eq_1
[STEP] cases h
[STEP] cases h'
[STEP] rfl
[STEP] set n'' := n' - 2
[STEP] have h_n''_eq_n_plus_2: n' = n'' + 2 := by
[STEP]   rw [Nat.sub_add_cancel]
[STEP]   linarith
[STEP] simp [h_n''_eq_n_plus_2] at *
[STEP] clear h_n''_eq_n_plus_2 h_n'_lt_1

[LAST STEP]
intro h h'
[SUCCESS]
[END]

`example_assistant`
[RUN TACTIC]
rw [fib_rec_unique] at h
[END]


`example_user`
Goals to prove:
[GOALS]
[GOAL] 1
fibonacci_non_computable n (impl n)
[HYPOTHESES] 1
[HYPOTHESIS] impl : ℕ → ℕ
[HYPOTHESIS] h_generated_spec : ∀ (n : ℕ),
[HYPOTHESIS]   let spec := fun result =>
[HYPOTHESIS]     match n with
[HYPOTHESIS]     | 0 => result = 0
[HYPOTHESIS]     | 1 => result = 1
[HYPOTHESIS]     | n'.succ.succ => result = impl n' + impl (n' + 1);
[HYPOTHESIS]   ∃ result, impl n = result ∧ spec result
[HYPOTHESIS] n : ℕ
[HYPOTHESIS] h_impl_n' : ∀ (n : ℕ), impl (n + 2) = impl n + impl (n + 1)
[HYPOTHESIS] h_impl_0 : impl 0 = 0
[HYPOTHESIS] h_impl_1 : impl 1 = 1

[INFORMAL-THEOREM]
Given an integer n, your task is to find the nth Fibonacci number.
The Fibonacci sequence is defined as follows:
- F(0) = 1
- F(1) = 1
- F(n) = F(n-1) + F(n-2) for n > 1

[FORMAL-THEOREM]
inductive fibonacci_non_computable : ℕ → ℕ → Prop
| base0 : fibonacci_non_computable 0 0
| base1 : fibonacci_non_computable 1 1
| step  : ∀ n f₁ f₂, fibonacci_non_computable n f₁ →
fibonacci_non_computable (n + 1) f₂ →
fibonacci_non_computable (n + 2) (f₁ + f₂)

def problem_spec
(impl: Nat → Nat)
(n: Nat) :=
let spec (result: Nat) :=
fibonacci_non_computable n result
∃ result, impl n = result ∧
spec result

def generated_spec
(impl: Nat → Nat)
(n: Nat) : Prop :=
let spec (result: Nat) :=
match n with
| 0 => result = 0
| 1 => result = 1
| n' + 2 => result = impl n' + impl (n' + 1)
∃ result, impl n = result ∧
spec result

theorem spec_isomorphism:
∀ impl,
(∀ x y, problem_spec impl x y) ↔
(∀ x y, generated impl x y)

[INFORMAL-PROOF]
1. Start by unfolding both the `problem_spec` and `generated_spec` and splitting the "iff".
2. Break the proof up into the base cases and the recursive case using `by_cases` and then `have`.
3. Use the lemmas `fib0_unique`, `fib1_unique`, `fib_inversion`, and `fib_rec_unique_seq`.

Throughout the proof, you can freely use any of the below helper lemmas, which you can assume to be true:
[HELPER LEMMAS]
[HELPER LEMMA]
lemma fib0_unique (n : ℕ) (h : fibonacci_non_computable 0 n) : n = 0 :=
[HELPER LEMMA]
lemma fib1_unique (n : ℕ) (h : fibonacci_non_computable 1 n) : n = 1 :=
[HELPER LEMMA]
lemma fib_rec_unique (n m : ℕ):
  fibonacci_non_computable (n + 2) m ↔
  ∃ f₁ f₂, fibonacci_non_computable n f₁ ∧
  fibonacci_non_computable (n + 1) f₂ ∧
  m = f₁ + f₂ :=
[HELPER LEMMA]
lemma fib_inversion (n f₁ f₂ : ℕ)
(h : fibonacci_non_computable n f₁) (h' : fibonacci_non_computable n f₂) :
  f₁ = f₂ :=
[HELPER LEMMA]
lemma fib_rec_unique_seq (n : ℕ)
(f : Nat → Nat)
(h_f_0: f 0 = 0)
(h_f_1: f 1 = 1)
(h_f_step: ∀ n, f (n + 2) = f n + f (n + 1))
: fibonacci_non_computable n (f n) :=

[STEPS]
[STEP] unfold problem_spec
[STEP] unfold generated_spec
[STEP] intro impl
[STEP] apply Iff.intro
[STEP] intro h_prob_spec
[STEP] intro n
[STEP] have h_impl_n_eq_0 := h_prob_spec n
[STEP] simp at h_impl_n_eq_0
[STEP] simp
[STEP] by_cases h_n_lt_1: n < 2
[STEP] -- if n = 0 then
  have h_n_eq_0_or_1: n = 0 ∨ n = 1 := by
[STEP] interval_cases n
[STEP] all_goals simp
[STEP] cases h_n_eq_0_or_1
[STEP] rename_i h_n_eq_0
[STEP] simp [h_n_eq_0] at *
[STEP] apply fib0_unique
[STEP] assumption
[STEP] rename_i h_n_eq_1
[STEP] simp [h_n_eq_1] at *
[STEP] apply fib1_unique
[STEP] assumption
[STEP] set n' := n - 2
[STEP] have h_n'_eq_n_plus_2: n = n' + 2 := by
[STEP] rw [Nat.sub_add_cancel]
[STEP] linarith
[STEP] simp [h_n'_eq_n_plus_2] at *
[STEP] clear h_n'_eq_n_plus_2 h_n_lt_1
[STEP] have h_fib_n' := h_prob_spec n'
[STEP] have h_fib_n'_1 := h_prob_spec (n' + 1)
[STEP] simp at h_fib_n'
[STEP] simp at h_fib_n'_1
[STEP] have h_fib_combination := fibonacci_non_computable.step _ _ _ h_fib_n' h_fib_n'_1
[STEP] have h_fib_inv := fib_inversion (n' + 2) _ _ h_fib_combination h_impl_n_eq_0
[STEP] linarith
[STEP] intro h_generated_spec
[STEP] simp
[STEP] intro n
[STEP] have h_impl_n': ∀ n, impl (n + 2) = impl n + impl (n + 1) := by
[STEP] intro n
[STEP] have h_impl_temp := h_generated_spec (n + 2)
[STEP] simp at h_impl_temp
[STEP] assumption
[STEP] have h_impl_0 := h_generated_spec 0
[STEP] have h_impl_1 := h_generated_spec 1
[STEP] simp at h_impl_0

[LAST STEP]
simp at h_impl_1
[SUCCESS]
[END]

`example_assistant`
[RUN TACTIC]
-- the goal looks very similar to the helper lemma fib_rec_unique_seq, so let's use it with the right arguments
simp [(fib_rec_unique_seq n impl h_impl_0 h_impl_1 h_impl_n')]
[END]

`conv end`