`conv start`

`example_user`
Goals to prove:
[GOALS]
[GOAL] 1
(∀ (x y : ℤ), problem_spec impl x y) → ∀ (x y : ℤ), generated_spec impl x y
[HYPOTHESES] 1
[HYPOTHESIS] impl : ℤ → ℤ → Bool

[STEPS]
[STEP] intro impl
[STEP] apply Iff.intro

[LAST STEP]
unfold problem_spec
[ERROR MESSAGE]
The proof-step does NOT simplify the goal. Try stepping back with different proof-step.
[END]

`example_assistant`
[RUN TACTIC]
intro h_prob_spec
[END]


`example_user`
Goals to prove:
[GOALS]
[GOAL] 1
impl x = if x < 0 then -x else x
[HYPOTHESES] 1
[HYPOTHESIS] impl : ℤ → ℤ
[HYPOTHESIS] h_prob_spec : ∀ (x : ℤ),
[HYPOTHESIS]   0 ≤ impl x ∧
[HYPOTHESIS]     impl (-x) = impl x ∧
[HYPOTHESIS]       (impl x = 0 ↔ x = 0) ∧ (0 ≤ x → impl (-x) + impl x = 2 * x) ∧ (x ≤ 0 → impl (-x) + impl x = -(2 * x))
[HYPOTHESIS] x : ℤ

[GOAL] 2
(∀ (x : ℤ), impl x = if x < 0 then -x else x) →
  ∀ (x : ℤ),
    0 ≤ impl x ∧
      impl (-x) = impl x ∧
        (impl x = 0 ↔ x = 0) ∧ (0 ≤ x → impl (-x) + impl x = 2 * x) ∧ (x ≤ 0 → impl (-x) + impl x = -(2 * x))
[HYPOTHESES] 1
[HYPOTHESIS] impl : ℤ → ℤ

[STEPS]
[STEP] unfold problem_spec
[STEP] unfold generated_spec
[STEP] simp
[STEP] intro impl
[STEP] apply Iff.intro
[STEP] intro h_prob_spec
[STEP] intro x

[INCORRECT STEPS]
[STEP] cases lt_or_ge x 0 with h_lt h_ge

[LAST STEP]
rw [h_prob_spec]

[ERROR MESSAGE]
tactic 'rewrite' failed, equality or iff proof expected
 0 ≤ impl ?x ∧
   impl (-?x) = impl ?x ∧
     (impl ?x = 0 ↔ ?x = 0) ∧ (0 ≤ ?x → impl (-?x) + impl ?x = 2 * ?x) ∧ (?x ≤ 0 → impl (-?x) + impl ?x = -(2 * ?x))
case mp
impl : ℤ → ℤ
h_prob_spec :
 ∀ (x : ℤ),
   0 ≤ impl x ∧
     impl (-x) = impl x ∧
       (impl x = 0 ↔ x = 0) ∧ (0 ≤ x → impl (-x) + impl x = 2 * x) ∧ (x ≤ 0 → impl (-x) + impl x = -(2 * x))
x : ℤ
⊢ impl x = if x < 0 then -x else x
[END]

`example_assistant`
[RUN TACTIC]
by_cases h_x_lt_0: x < 0
[END]


`example_user`
Goals to prove:
[GOALS]
[GOAL] 1
impl (-x) = impl x ∧
  (impl x = 0 ↔ x = 0) ∧ (0 ≤ x → impl (-x) + impl x = 2 * x) ∧ (x ≤ 0 → impl (-x) + impl x = -(2 * x))
[HYPOTHESES] 1
[HYPOTHESIS] impl : ℤ → ℤ
[HYPOTHESIS] h_generated_spec : ∀ (x : ℤ), impl x = if x < 0 then -x else x
[HYPOTHESIS] x : ℤ
[HYPOTHESIS] h_x_lt_0 : x < 0
[HYPOTHESIS] h_not_0_lt_x : ¬0 < x
[HYPOTHESIS] h_impl : impl x = -x
[HYPOTHESIS] h_0_le_impl_x : 0 ≤ impl x

[GOAL] 2
0 ≤ impl x ∧
  impl (-x) = impl x ∧
    (impl x = 0 ↔ x = 0) ∧ (0 ≤ x → impl (-x) + impl x = 2 * x) ∧ (x ≤ 0 → impl (-x) + impl x = -(2 * x))
[HYPOTHESES] 1
[HYPOTHESIS] impl : ℤ → ℤ
[HYPOTHESIS] h_generated_spec : ∀ (x : ℤ), impl x = if x < 0 then -x else x
[HYPOTHESIS] x : ℤ
[HYPOTHESIS] h_x_lt_0 : ¬x < 0

[STEPS]
[STEP] unfold problem_spec
[STEP] unfold generated_spec
[STEP] simp
[STEP] intro impl
[STEP] apply Iff.intro
[STEP] intro h_prob_spec
[STEP] intro x
[STEP] by_cases h_x_lt_0: x < 0
[STEP] -- if x < 0 then
have h_x_le_0: x ≤ 0 := by
[STEP]   linarith
[STEP] simp [h_x_lt_0]
[STEP] have h_impl := h_prob_spec x
[STEP] simp [h_x_lt_0 ] at h_impl
[STEP] have h_neg_impl := h_impl.2.2.2
[STEP] simp [h_x_le_0] at h_neg_impl
[STEP] linarith
[STEP] simp [h_x_lt_0]
[STEP] have h_impl := h_prob_spec x
[STEP] simp at h_x_lt_0
[STEP] simp [h_x_lt_0] at h_impl
[STEP] have h_pos_impl := h_impl.2.2.2.1
[STEP] linarith
[STEP] intro h_generated_spec
[STEP] intro x
[STEP] by_cases h_x_lt_0: x < 0
[STEP] -- if x < 0 then
have h_not_0_lt_x: ¬ (0 < x) := by
[STEP]   linarith
[STEP] have h_impl := h_generated_spec x
[STEP] simp [h_x_lt_0] at h_impl
[STEP] have h_0_le_impl_x: 0 ≤ impl x := by
[STEP]   simp [h_impl]
[STEP]   linarith
[STEP] simp [h_0_le_impl_x]

[LAST STEP]
linarith [h_impl, h_0_le_impl_x, h_not_0_lt_x]

[ERROR MESSAGE]
linarith failed to find a contradiction
case pos
impl : ℤ → ℤ
h_generated_spec : ∀ (x : ℤ), impl x = if x < 0 then -x else x
x : ℤ
h_x_lt_0 : x < 0
h_not_0_lt_x : ¬0 < x
h_impl : impl x = -x
h_0_le_impl_x : 0 ≤ impl x
⊢ False
failed
[END]

`example_assistant`
[RUN TACTIC]
have h_impl_neg_x := h_generated_spec (-x)
[END]


`example_user`
Goals to prove:
[GOALS]
[GOAL] 1
impl (-x) = impl x ∧
  (impl x = 0 ↔ x = 0) ∧ (0 ≤ x → impl (-x) + impl x = 2 * x) ∧ (x ≤ 0 → impl (-x) + impl x = -(2 * x))
[HYPOTHESES] 1
[HYPOTHESIS] impl : ℤ → ℤ
[HYPOTHESIS] h_generated_spec : ∀ (x : ℤ), impl x = if x < 0 then -x else x
[HYPOTHESIS] x : ℤ
[HYPOTHESIS] h_x_lt_0 : x < 0
[HYPOTHESIS] h_not_0_lt_x : ¬0 < x
[HYPOTHESIS] h_impl : impl x = -x
[HYPOTHESIS] h_0_le_impl_x : 0 ≤ impl x
[HYPOTHESIS] h_impl_neg_x : impl (-x) = -x

[GOAL] 2
0 ≤ impl x ∧
  impl (-x) = impl x ∧
    (impl x = 0 ↔ x = 0) ∧ (0 ≤ x → impl (-x) + impl x = 2 * x) ∧ (x ≤ 0 → impl (-x) + impl x = -(2 * x))
[HYPOTHESES] 1
[HYPOTHESIS] impl : ℤ → ℤ
[HYPOTHESIS] h_generated_spec : ∀ (x : ℤ), impl x = if x < 0 then -x else x
[HYPOTHESIS] x : ℤ
[HYPOTHESIS] h_x_lt_0 : ¬x < 0

[STEPS]
[STEP] unfold problem_spec
[STEP] unfold generated_spec
[STEP] simp
[STEP] intro impl
[STEP] apply Iff.intro
[STEP] intro h_prob_spec
[STEP] intro x
[STEP] by_cases h_x_lt_0: x < 0
[STEP] -- if x < 0 then
have h_x_le_0: x ≤ 0 := by
[STEP]   linarith
[STEP] simp [h_x_lt_0]
[STEP] have h_impl := h_prob_spec x
[STEP] simp [h_x_lt_0 ] at h_impl
[STEP] have h_neg_impl := h_impl.2.2.2
[STEP] simp [h_x_le_0] at h_neg_impl
[STEP] linarith
[STEP] simp [h_x_lt_0]
[STEP] have h_impl := h_prob_spec x
[STEP] simp at h_x_lt_0
[STEP] simp [h_x_lt_0] at h_impl
[STEP] have h_pos_impl := h_impl.2.2.2.1
[STEP] linarith
[STEP] intro h_generated_spec
[STEP] intro x
[STEP] by_cases h_x_lt_0: x < 0
[STEP] -- if x < 0 then
have h_not_0_lt_x: ¬ (0 < x) := by
[STEP]   linarith
[STEP] have h_impl := h_generated_spec x
[STEP] simp [h_x_lt_0] at h_impl
[STEP] have h_0_le_impl_x: 0 ≤ impl x := by
[STEP]   simp [h_impl]
[STEP]   linarith
[STEP] simp [h_0_le_impl_x]
[STEP] have h_impl_neg_x := h_generated_spec (-x)
[STEP] simp [h_x_lt_0] at h_impl_neg_x

[LAST STEP]
simp [h_not_0_lt_x] at h_impl_neg_x
[SUCCESS]
[END]

`example_assistant`
[RUN TACTIC]
rw [←h_impl_neg_x] at h_impl
[END]


`example_user`
Goals to prove:
[GOALS]
[GOAL] 1
generated_spec.loop score_changes (threshold - k) score coins =
  generated_spec.loop score_changes threshold (score + k) coins
[HYPOTHESES] 1
[HYPOTHESIS] score_changes : List ℤ
[HYPOTHESIS] threshold score : ℤ
[HYPOTHESIS] coins : ℕ
[HYPOTHESIS] k : ℤ
[HYPOTHESIS] h_rounds_played : score_changes.length > 0

`example_assistant`
[RUN TACTIC]
induction' score_changes generalizing score coins
[END]


`example_user`
Goals to prove:
[GOALS]
[GOAL] 1
generated_spec.loop tail (threshold - k) (head + score) (coins + 1) =
  generated_spec.loop tail threshold (head + score + k) (coins + 1)
[HYPOTHESES] 1
[HYPOTHESIS] threshold k head : ℤ
[HYPOTHESIS] tail : List ℤ
[HYPOTHESIS] ih : ∀ (score : ℤ) (coins : ℕ),
[HYPOTHESIS]   tail.length > 0 →
[HYPOTHESIS]     generated_spec.loop tail (threshold - k) score coins = generated_spec.loop tail threshold (score + k) coins
[HYPOTHESIS] score : ℤ
[HYPOTHESIS] coins : ℕ
[HYPOTHESIS] h_rounds_played : (head :: tail).length > 0
[HYPOTHESIS] h_head_ge_threshold : head + score ≥ threshold - k
[HYPOTHESIS] h_head_ge_threshold' : threshold ≤ head + score + k
[HYPOTHESIS] h_head_ge_threshold'' : threshold ≤ head + (score + k)
[HYPOTHESIS] h_tail_len_0 : tail.length = 0

[GOAL] 2
generated_spec.loop tail (threshold - k) (head + score) (coins + 1) =
  generated_spec.loop tail threshold (head + score + k) (coins + 1)
[HYPOTHESES] 1
[HYPOTHESIS] threshold k head : ℤ
[HYPOTHESIS] tail : List ℤ
[HYPOTHESIS] ih : ∀ (score : ℤ) (coins : ℕ),
[HYPOTHESIS]   tail.length > 0 →
[HYPOTHESIS]     generated_spec.loop tail (threshold - k) score coins = generated_spec.loop tail threshold (score + k) coins
[HYPOTHESIS] score : ℤ
[HYPOTHESIS] coins : ℕ
[HYPOTHESIS] h_rounds_played : (head :: tail).length > 0
[HYPOTHESIS] h_head_ge_threshold : head + score ≥ threshold - k
[HYPOTHESIS] h_head_ge_threshold' : threshold ≤ head + score + k
[HYPOTHESIS] h_head_ge_threshold'' : threshold ≤ head + (score + k)
[HYPOTHESIS] h_tail_len_0 : ¬tail.length ≤ 0

[GOAL] 3
generated_spec.loop (head :: tail) (threshold - k) score coins =
  generated_spec.loop (head :: tail) threshold (score + k) coins
[HYPOTHESES] 1
[HYPOTHESIS] threshold k head : ℤ
[HYPOTHESIS] tail : List ℤ
[HYPOTHESIS] ih : ∀ (score : ℤ) (coins : ℕ),
[HYPOTHESIS]   tail.length > 0 →
[HYPOTHESIS]     generated_spec.loop tail (threshold - k) score coins = generated_spec.loop tail threshold (score + k) coins
[HYPOTHESIS] score : ℤ
[HYPOTHESIS] coins : ℕ
[HYPOTHESIS] h_rounds_played : (head :: tail).length > 0
[HYPOTHESIS] h_head_ge_threshold : ¬head + score ≥ threshold - k

[STEPS]
[STEP] induction' score_changes generalizing score coins
[STEP] simp at h_rounds_played
[STEP] rename_i head tail ih
[STEP] by_cases h_head_ge_threshold: head + score ≥ threshold - k
[STEP] -- case where head + score ≥ threshold
simp [generated_spec.loop]
[STEP] have h_head_ge_threshold': threshold ≤ head + score + k := by
[STEP]   linarith
[STEP] simp [h_head_ge_threshold']
[STEP] have h_head_ge_threshold'': threshold ≤ head + (score + k) := by
[STEP]   linarith
[STEP] simp [h_head_ge_threshold'']
[STEP] simp [←Int.add_assoc]
[STEP] by_cases h_tail_len_0: tail.length ≤ 0

[LAST STEP]
-- case where tail.length ≤ 0
rw [Nat.le_zero] at h_tail_len_0
[SUCCESS]
[END]

`example_assistant`
[RUN TACTIC]
have h_tail_nil := List.eq_nil_of_length_eq_zero h_tail_len_0
[END]


`example_user`
Goals to prove:
[GOALS]
[GOAL] 1
generated_spec.loop tail (threshold - k) (head + score) (if threshold ≤ head + score + k then coins + 1 else coins) =
  generated_spec.loop tail threshold (head + (score + k)) (if threshold ≤ head + (score + k) then coins + 1 else coins)
[HYPOTHESES] 1
[HYPOTHESIS] threshold k head : ℤ
[HYPOTHESIS] tail : List ℤ
[HYPOTHESIS] score : ℤ
[HYPOTHESIS] coins : ℕ
[HYPOTHESIS] h_rounds_played : (head :: tail).length > 0
[HYPOTHESIS] h_perm' : head + score + k = head + (score + k)
[HYPOTHESIS] h_tail_len_0 : ¬tail.length ≤ 0
[HYPOTHESIS] h_tail_len_gt_0 : tail.length > 0
[HYPOTHESIS] ih : generated_spec.loop tail (threshold - k) (head + score) coins =
[HYPOTHESIS]   generated_spec.loop tail threshold (head + score + k) coins
[HYPOTHESIS] h_head_ge_threshold : head + score + k < threshold

[STEPS]
[STEP] induction' score_changes generalizing score coins
[STEP] simp at h_rounds_played
[STEP] rename_i head tail ih
[STEP] by_cases h_head_ge_threshold: head + score ≥ threshold - k
[STEP] -- case where head + score ≥ threshold
simp [generated_spec.loop]
[STEP] have h_head_ge_threshold': threshold ≤ head + score + k := by
[STEP]   linarith
[STEP] simp [h_head_ge_threshold']
[STEP] have h_head_ge_threshold'': threshold ≤ head + (score + k) := by
[STEP]   linarith
[STEP] simp [h_head_ge_threshold'']
[STEP] simp [←Int.add_assoc]
[STEP] by_cases h_tail_len_0: tail.length ≤ 0
[STEP] -- case where tail.length ≤ 0
rw [Nat.le_zero] at h_tail_len_0
[STEP] have h_tail_nil := List.eq_nil_of_length_eq_zero h_tail_len_0
[STEP] simp [h_tail_nil]
[STEP] simp [generated_spec.loop]
[STEP] -- case where tail.length > 0
[STEP] have h_tail_len_gt_0: tail.length > 0 := by
[STEP]   linarith
[STEP] simp [h_tail_len_gt_0] at ih
[STEP] specialize ih (head + score) (coins + 1)
[STEP] simp [←ih]
[STEP] -- case where head + score < threshold
have h_perm': head + score + k = head + (score + k) := by
[STEP]   linarith
[STEP] by_cases h_tail_len_0: tail.length ≤ 0
[STEP] rw [Nat.le_zero] at h_tail_len_0
[STEP] have h_tail_nil := List.eq_nil_of_length_eq_zero h_tail_len_0
[STEP] simp [h_tail_nil]
[STEP] simp [generated_spec.loop]
[STEP] rw [h_perm']
[STEP] have h_tail_len_gt_0: tail.length > 0 := by
[STEP]   linarith
[STEP] simp [h_tail_len_gt_0] at ih
[STEP] specialize ih (head + score) coins
[STEP] simp [generated_spec.loop]

[LAST STEP]
simp at h_head_ge_threshold
[SUCCESS]
[END]

`example_assistant`
[RUN TACTIC]
have h_head_lt_threshold: ¬ (threshold ≤ head + score + k) := by
[END]


`example_user`
Goals to prove:
[GOALS]
[GOAL] 1
∃ i',
  1 ≤ i' ∧ i' ≤ (head :: tail).length →
    score + (List.take i' (head :: tail)).sum ≥ threshold →
      generated_spec.loop (head :: tail) threshold score coins =
          1 +
            generated_spec.loop (List.drop i' (head :: tail)) threshold (score + (List.take i' (head :: tail)).sum)
              coins →
        ∀ (i : ℕ), 1 ≤ i ∧ i < i' → score + (List.take i (head :: tail)).sum < threshold
[HYPOTHESES] 1
[HYPOTHESIS] threshold head : ℤ
[HYPOTHESIS] tail : List ℤ
[HYPOTHESIS] ih : ∀ (score : ℤ) (coins : ℕ),
[HYPOTHESIS]   tail.length > 0 →
[HYPOTHESIS]     coins < generated_spec.loop tail threshold score coins →
[HYPOTHESIS]       ∃ i',
[HYPOTHESIS]         1 ≤ i' ∧ i' ≤ tail.length →
[HYPOTHESIS]           score + (List.take i' tail).sum ≥ threshold →
[HYPOTHESIS]             generated_spec.loop tail threshold score coins =
[HYPOTHESIS]                 1 + generated_spec.loop (List.drop i' tail) threshold (score + (List.take i' tail).sum) coins →
[HYPOTHESIS]               ∀ (i : ℕ), 1 ≤ i ∧ i < i' → score + (List.take i tail).sum < threshold
[HYPOTHESIS] score : ℤ
[HYPOTHESIS] coins : ℕ
[HYPOTHESIS] h_rounds_played : (head :: tail).length > 0
[HYPOTHESIS] h_within_threshold : coins < generated_spec.loop (head :: tail) threshold score coins
[HYPOTHESIS] h_head_ge_threshold : head + score ≥ threshold
[HYPOTHESIS] h_threshold_lt_head_score : threshold ≤ score + head

[GOAL] 2
∃ i',
  1 ≤ i' ∧ i' ≤ (head :: tail).length →
    score + (List.take i' (head :: tail)).sum ≥ threshold →
      generated_spec.loop (head :: tail) threshold score coins =
          1 +
            generated_spec.loop (List.drop i' (head :: tail)) threshold (score + (List.take i' (head :: tail)).sum)
              coins →
        ∀ (i : ℕ), 1 ≤ i ∧ i < i' → score + (List.take i (head :: tail)).sum < threshold
[HYPOTHESES] 1
[HYPOTHESIS] threshold head : ℤ
[HYPOTHESIS] tail : List ℤ
[HYPOTHESIS] ih : ∀ (score : ℤ) (coins : ℕ),
[HYPOTHESIS]   tail.length > 0 →
[HYPOTHESIS]     coins < generated_spec.loop tail threshold score coins →
[HYPOTHESIS]       ∃ i',
[HYPOTHESIS]         1 ≤ i' ∧ i' ≤ tail.length →
[HYPOTHESIS]           score + (List.take i' tail).sum ≥ threshold →
[HYPOTHESIS]             generated_spec.loop tail threshold score coins =
[HYPOTHESIS]                 1 + generated_spec.loop (List.drop i' tail) threshold (score + (List.take i' tail).sum) coins →
[HYPOTHESIS]               ∀ (i : ℕ), 1 ≤ i ∧ i < i' → score + (List.take i tail).sum < threshold
[HYPOTHESIS] score : ℤ
[HYPOTHESIS] coins : ℕ
[HYPOTHESIS] h_rounds_played : (head :: tail).length > 0
[HYPOTHESIS] h_within_threshold : coins < generated_spec.loop (head :: tail) threshold score coins
[HYPOTHESIS] h_head_ge_threshold : ¬head + score ≥ threshold

[STEPS]
[STEP] induction' score_changes generalizing score coins
[STEP] simp at h_rounds_played
[STEP] rename_i head tail ih
[STEP] by_cases h_head_ge_threshold: head + score ≥ threshold
[STEP] -- Case 1: where head + score ≥ threshold
have h_threshold_lt_head_score: threshold ≤ score + head := by

[LAST STEP]
linarith
[SUCCESS]
[END]

`example_assistant`
[RUN TACTIC]
have h_simple_increment := (generated_spec_loop_simple_increment head tail threshold score coins).right h_head_ge_threshold
[END]


`example_user`
Goals to prove:
[GOALS]
[GOAL] 1
∀ (i : ℕ), 1 ≤ i → i < i₁ + 1 → score + (List.take i (head :: tail)).sum < threshold
[HYPOTHESES] 1
[HYPOTHESIS] threshold head : ℤ
[HYPOTHESIS] tail : List ℤ
[HYPOTHESIS] score : ℤ
[HYPOTHESIS] coins : ℕ
[HYPOTHESIS] h_rounds_played : (head :: tail).length > 0
[HYPOTHESIS] h_head_ge_threshold : ¬head + score ≥ threshold
[HYPOTHESIS] h_simple_increment : head + score < threshold →
[HYPOTHESIS]   generated_spec.loop (head :: tail) threshold score coins = generated_spec.loop tail threshold (head + score) coins
[HYPOTHESIS] h_within_threshold : coins < generated_spec.loop tail threshold (head + score) coins
[HYPOTHESIS] h_tail_len_0 : ¬tail.length ≤ 0
[HYPOTHESIS] h_tail_len_gt_0 : tail.length > 0
[HYPOTHESIS] i₁ : ℕ
[HYPOTHESIS] i₁h : 1 ≤ i₁ →
[HYPOTHESIS]   i₁ ≤ tail.length →
[HYPOTHESIS]     threshold ≤ head + score + (List.take i₁ tail).sum →
[HYPOTHESIS]       generated_spec.loop tail threshold (head + score) coins =
[HYPOTHESIS]           1 + generated_spec.loop (List.drop i₁ tail) threshold (head + score + (List.take i₁ tail).sum) coins →
[HYPOTHESIS]         ∀ (i : ℕ), 1 ≤ i → i < i₁ → head + score + (List.take i tail).sum < threshold
[HYPOTHESIS] h_score_head_ge_threshold : score + (List.take (i₁ + 1) (head :: tail)).sum ≥ threshold
[HYPOTHESIS] h_perm_sum' : score + (head + (List.take i₁ tail).sum) = head + score + (List.take i₁ tail).sum
[HYPOTHESIS] h_to_prove : generated_spec.loop tail threshold (head + score) coins =
[HYPOTHESIS]   1 + generated_spec.loop (List.drop i₁ tail) threshold (head + score + (List.take i₁ tail).sum) coins
[HYPOTHESIS] h_1_le_i' : i₁ ≤ tail.length

Throughout the proof, you can freely use any of the below helper lemmas, which you can assume to be true:
[HELPER LEMMAS]
[HELPER LEMMA]
lemma generated_spec_loop_threshold_invariant
(score_changes: List Int)
(threshold: Int)
(score: Int)
(coins: Nat)
(k: Int)
(h_rounds_played: score_changes.length > 0)
: generated_spec.loop score_changes (threshold - k) score coins
= generated_spec.loop score_changes threshold (score + k) coins :=
[HELPER LEMMA]
lemma generated_spec_loop_simple_increment
(head: Int)
(score_changes_tail: List Int)
(threshold: Int)
(score: Int)
(coins: Nat)
: (head + score < threshold →
generated_spec.loop (head :: score_changes_tail) threshold score coins =
generated_spec.loop (score_changes_tail) threshold (head + score) coins) ∧
(head + score ≥ threshold →
generated_spec.loop (head :: score_changes_tail) threshold score coins =
1 + generated_spec.loop (score_changes_tail) threshold (head + score) coins) :=
[HELPER LEMMA]
lemma generated_spec_loop_coin_monotonic_increasing
(score_changes: List Int)
(threshold: Int)
(score: Int)
(coins: Nat)
(h_rounds_played: score_changes.length > 0)
: coins ≤ generated_spec.loop score_changes threshold score coins :=
[HELPER LEMMA]
lemma generated_spec_loop_invariant_stop
(score_changes: List Int)
(threshold: Int)
(score: Int)
(coins: Nat)
(h_rounds_played: score_changes.length > 0)
(h_within_threshold: coins = generated_spec.loop score_changes threshold score coins)
: ∀ i, 1 ≤ i ∧ i ≤ score_changes.length →
score + (score_changes.take i).sum < threshold :=

[STEPS]
[STEP] induction' score_changes generalizing score coins
[STEP] simp at h_rounds_played
[STEP] rename_i head tail ih
[STEP] by_cases h_head_ge_threshold: head + score ≥ threshold
[STEP] -- Case 1: where head + score ≥ threshold
have h_threshold_lt_head_score: threshold ≤ score + head := by
[STEP]   linarith
[STEP] have h_simple_increment := (generated_spec_loop_simple_increment head tail threshold score coins).right h_head_ge_threshold
[STEP] have h_sum_perm: score + head = head + score := by
[STEP]   linarith
[STEP] use 1
[STEP] simp
[STEP] simp [h_threshold_lt_head_score]
[STEP] simp [h_simple_increment]
[STEP] simp [←h_sum_perm]
[STEP] intro i h_1_le_1 h_i_le_1
[STEP] linarith
[STEP] -- Case 2: where head + score < threshold
have h_simple_increment := (generated_spec_loop_simple_increment head tail threshold score coins).left
[STEP] simp [h_simple_increment (by linarith)] at h_within_threshold
[STEP] by_cases h_tail_len_0: tail.length ≤ 0
[STEP] -- Case 2.1: where tail.length ≤ 0
rw [Nat.le_zero] at h_tail_len_0
[STEP] have h_tail_nil := List.eq_nil_of_length_eq_zero h_tail_len_0
[STEP] simp [h_tail_nil] at h_within_threshold
[STEP] simp [generated_spec.loop] at h_within_threshold
[STEP] -- Case 2.2: where tail.length > 0
have h_tail_len_gt_0: tail.length > 0 := by
[STEP]   linarith
[STEP] simp [h_tail_len_gt_0] at ih
[STEP] specialize ih (head + score) coins
[STEP] simp [h_within_threshold ] at ih
[STEP] -- i₁
obtain ⟨i₁, i₁h⟩ := ih
[STEP] -- h_1_le_i', h_i'_le_len, h_to_prove
use i₁ + 1
[STEP] intro h_1_le_i'
[STEP] intro h_score_head_ge_threshold
[STEP] simp [h_simple_increment (by linarith)]
[STEP] have h_perm_sum': score + (head + (List.take i₁ tail).sum) = head + score + (List.take i₁ tail).sum := by
[STEP]   linarith
[STEP] simp [h_perm_sum']
[STEP] intro h_to_prove

[LAST STEP]
simp at h_1_le_i'
[SUCCESS]
[END]

`example_assistant`
[RUN TACTIC]
by_cases h_1_le_i'_lt_i₁: 1 ≤ i₁
[END]


`example_user`
Goals to prove:
[GOALS]
[GOAL] 1
score + (head + (List.take i' tail).sum) < threshold
[HYPOTHESES] 1
[HYPOTHESIS] threshold head : ℤ
[HYPOTHESIS] tail : List ℤ
[HYPOTHESIS] score : ℤ
[HYPOTHESIS] coins : ℕ
[HYPOTHESIS] h_rounds_played : (head :: tail).length > 0
[HYPOTHESIS] h_head_ge_threshold : ¬head + score ≥ threshold
[HYPOTHESIS] h_simple_increment : head + score < threshold →
[HYPOTHESIS]   generated_spec.loop (head :: tail) threshold score coins = generated_spec.loop tail threshold (head + score) coins
[HYPOTHESIS] h_within_threshold : coins < generated_spec.loop tail threshold (head + score) coins
[HYPOTHESIS] h_tail_len_0 : ¬tail.length ≤ 0
[HYPOTHESIS] h_tail_len_gt_0 : tail.length > 0
[HYPOTHESIS] i₁ : ℕ
[HYPOTHESIS] h_score_head_ge_threshold : score + (List.take (i₁ + 1) (head :: tail)).sum ≥ threshold
[HYPOTHESIS] h_perm_sum' : score + (head + (List.take i₁ tail).sum) = head + score + (List.take i₁ tail).sum
[HYPOTHESIS] h_to_prove : generated_spec.loop tail threshold (head + score) coins =
[HYPOTHESIS]   1 + generated_spec.loop (List.drop i₁ tail) threshold (head + score + (List.take i₁ tail).sum) coins
[HYPOTHESIS] h_1_le_i'✝ : i₁ ≤ tail.length
[HYPOTHESIS] h_1_le_i'_lt_i₁ : 1 ≤ i₁
[HYPOTHESIS] h_threshold_head_score_i₁ : threshold ≤ head + score + (List.take i₁ tail).sum
[HYPOTHESIS] i₁h : ∀ (i : ℕ), 1 ≤ i → i < i₁ → head + score + (List.take i tail).sum < threshold
[HYPOTHESIS] i : ℕ
[HYPOTHESIS] h_1_le_i : 1 ≤ i
[HYPOTHESIS] i' : ℕ := i - 1
[HYPOTHESIS] h_1_le_i_plus_1 : i = i' + 1
[HYPOTHESIS] h_i_lt_i₁_plus_1 : i' < i₁
[HYPOTHESIS] h_1_le_i' : 1 ≤ i'
[HYPOTHESIS] h_i₁_h : head + score + (List.take i' tail).sum < threshold

[GOAL] 2
score + (head + (List.take i' tail).sum) < threshold
[HYPOTHESES] 1
[HYPOTHESIS] threshold head : ℤ
[HYPOTHESIS] tail : List ℤ
[HYPOTHESIS] score : ℤ
[HYPOTHESIS] coins : ℕ
[HYPOTHESIS] h_rounds_played : (head :: tail).length > 0
[HYPOTHESIS] h_head_ge_threshold : ¬head + score ≥ threshold
[HYPOTHESIS] h_simple_increment : head + score < threshold →
[HYPOTHESIS]   generated_spec.loop (head :: tail) threshold score coins = generated_spec.loop tail threshold (head + score) coins
[HYPOTHESIS] h_within_threshold : coins < generated_spec.loop tail threshold (head + score) coins
[HYPOTHESIS] h_tail_len_0 : ¬tail.length ≤ 0
[HYPOTHESIS] h_tail_len_gt_0 : tail.length > 0
[HYPOTHESIS] i₁ : ℕ
[HYPOTHESIS] h_score_head_ge_threshold : score + (List.take (i₁ + 1) (head :: tail)).sum ≥ threshold
[HYPOTHESIS] h_perm_sum' : score + (head + (List.take i₁ tail).sum) = head + score + (List.take i₁ tail).sum
[HYPOTHESIS] h_to_prove : generated_spec.loop tail threshold (head + score) coins =
[HYPOTHESIS]   1 + generated_spec.loop (List.drop i₁ tail) threshold (head + score + (List.take i₁ tail).sum) coins
[HYPOTHESIS] h_1_le_i'✝ : i₁ ≤ tail.length
[HYPOTHESIS] h_1_le_i'_lt_i₁ : 1 ≤ i₁
[HYPOTHESIS] h_threshold_head_score_i₁ : threshold ≤ head + score + (List.take i₁ tail).sum
[HYPOTHESIS] i₁h : ∀ (i : ℕ), 1 ≤ i → i < i₁ → head + score + (List.take i tail).sum < threshold
[HYPOTHESIS] i : ℕ
[HYPOTHESIS] h_1_le_i : 1 ≤ i
[HYPOTHESIS] i' : ℕ := i - 1
[HYPOTHESIS] h_1_le_i_plus_1 : i = i' + 1
[HYPOTHESIS] h_i_lt_i₁_plus_1 : i' < i₁
[HYPOTHESIS] h_1_le_i' : ¬1 ≤ i'

[GOAL] 3
∀ (i : ℕ), 1 ≤ i → i < i₁ + 1 → score + (List.take i (head :: tail)).sum < threshold
[HYPOTHESES] 1
[HYPOTHESIS] threshold head : ℤ
[HYPOTHESIS] tail : List ℤ
[HYPOTHESIS] score : ℤ
[HYPOTHESIS] coins : ℕ
[HYPOTHESIS] h_rounds_played : (head :: tail).length > 0
[HYPOTHESIS] h_head_ge_threshold : ¬head + score ≥ threshold
[HYPOTHESIS] h_simple_increment : head + score < threshold →
[HYPOTHESIS]   generated_spec.loop (head :: tail) threshold score coins = generated_spec.loop tail threshold (head + score) coins
[HYPOTHESIS] h_within_threshold : coins < generated_spec.loop tail threshold (head + score) coins
[HYPOTHESIS] h_tail_len_0 : ¬tail.length ≤ 0
[HYPOTHESIS] h_tail_len_gt_0 : tail.length > 0
[HYPOTHESIS] i₁ : ℕ
[HYPOTHESIS] h_score_head_ge_threshold : score + (List.take (i₁ + 1) (head :: tail)).sum ≥ threshold
[HYPOTHESIS] h_perm_sum' : score + (head + (List.take i₁ tail).sum) = head + score + (List.take i₁ tail).sum
[HYPOTHESIS] h_to_prove : generated_spec.loop tail threshold (head + score) coins =
[HYPOTHESIS]   1 + generated_spec.loop (List.drop i₁ tail) threshold (head + score + (List.take i₁ tail).sum) coins
[HYPOTHESIS] h_1_le_i' : i₁ ≤ tail.length
[HYPOTHESIS] h_1_le_i'_lt_i₁ : 1 ≤ i₁
[HYPOTHESIS] i₁h : threshold ≤ head + score + (List.take i₁ tail).sum →
[HYPOTHESIS]   generated_spec.loop tail threshold (head + score) coins =
[HYPOTHESIS]       1 + generated_spec.loop (List.drop i₁ tail) threshold (head + score + (List.take i₁ tail).sum) coins →
[HYPOTHESIS]     ∀ (i : ℕ), 1 ≤ i → i < i₁ → head + score + (List.take i tail).sum < threshold
[HYPOTHESIS] h_threshold_head_score_i₁ : ¬threshold ≤ head + score + (List.take i₁ tail).sum

[GOAL] 4
∀ (i : ℕ), 1 ≤ i → i < i₁ + 1 → score + (List.take i (head :: tail)).sum < threshold
[HYPOTHESES] 1
[HYPOTHESIS] threshold head : ℤ
[HYPOTHESIS] tail : List ℤ
[HYPOTHESIS] score : ℤ
[HYPOTHESIS] coins : ℕ
[HYPOTHESIS] h_rounds_played : (head :: tail).length > 0
[HYPOTHESIS] h_head_ge_threshold : ¬head + score ≥ threshold
[HYPOTHESIS] h_simple_increment : head + score < threshold →
[HYPOTHESIS]   generated_spec.loop (head :: tail) threshold score coins = generated_spec.loop tail threshold (head + score) coins
[HYPOTHESIS] h_within_threshold : coins < generated_spec.loop tail threshold (head + score) coins
[HYPOTHESIS] h_tail_len_0 : ¬tail.length ≤ 0
[HYPOTHESIS] h_tail_len_gt_0 : tail.length > 0
[HYPOTHESIS] i₁ : ℕ
[HYPOTHESIS] i₁h : 1 ≤ i₁ →
[HYPOTHESIS]   i₁ ≤ tail.length →
[HYPOTHESIS]     threshold ≤ head + score + (List.take i₁ tail).sum →
[HYPOTHESIS]       generated_spec.loop tail threshold (head + score) coins =
[HYPOTHESIS]           1 + generated_spec.loop (List.drop i₁ tail) threshold (head + score + (List.take i₁ tail).sum) coins →
[HYPOTHESIS]         ∀ (i : ℕ), 1 ≤ i → i < i₁ → head + score + (List.take i tail).sum < threshold
[HYPOTHESIS] h_score_head_ge_threshold : score + (List.take (i₁ + 1) (head :: tail)).sum ≥ threshold
[HYPOTHESIS] h_perm_sum' : score + (head + (List.take i₁ tail).sum) = head + score + (List.take i₁ tail).sum
[HYPOTHESIS] h_to_prove : generated_spec.loop tail threshold (head + score) coins =
[HYPOTHESIS]   1 + generated_spec.loop (List.drop i₁ tail) threshold (head + score + (List.take i₁ tail).sum) coins
[HYPOTHESIS] h_1_le_i' : i₁ ≤ tail.length
[HYPOTHESIS] h_1_le_i'_lt_i₁ : ¬1 ≤ i₁

Throughout the proof, you can freely use any of the below helper lemmas, which you can assume to be true:
[HELPER LEMMAS]
[HELPER LEMMA]
lemma generated_spec_loop_threshold_invariant
(score_changes: List Int)
(threshold: Int)
(score: Int)
(coins: Nat)
(k: Int)
(h_rounds_played: score_changes.length > 0)
: generated_spec.loop score_changes (threshold - k) score coins
= generated_spec.loop score_changes threshold (score + k) coins :=
[HELPER LEMMA]
lemma generated_spec_loop_simple_increment
(head: Int)
(score_changes_tail: List Int)
(threshold: Int)
(score: Int)
(coins: Nat)
: (head + score < threshold →
generated_spec.loop (head :: score_changes_tail) threshold score coins =
generated_spec.loop (score_changes_tail) threshold (head + score) coins) ∧
(head + score ≥ threshold →
generated_spec.loop (head :: score_changes_tail) threshold score coins =
1 + generated_spec.loop (score_changes_tail) threshold (head + score) coins) :=
[HELPER LEMMA]
lemma generated_spec_loop_coin_monotonic_increasing
(score_changes: List Int)
(threshold: Int)
(score: Int)
(coins: Nat)
(h_rounds_played: score_changes.length > 0)
: coins ≤ generated_spec.loop score_changes threshold score coins :=
[HELPER LEMMA]
lemma generated_spec_loop_invariant_stop
(score_changes: List Int)
(threshold: Int)
(score: Int)
(coins: Nat)
(h_rounds_played: score_changes.length > 0)
(h_within_threshold: coins = generated_spec.loop score_changes threshold score coins)
: ∀ i, 1 ≤ i ∧ i ≤ score_changes.length →
score + (score_changes.take i).sum < threshold :=

[STEPS]
[STEP] induction' score_changes generalizing score coins
[STEP] simp at h_rounds_played
[STEP] rename_i head tail ih
[STEP] by_cases h_head_ge_threshold: head + score ≥ threshold
[STEP] -- Case 1: where head + score ≥ threshold
have h_threshold_lt_head_score: threshold ≤ score + head := by
[STEP]   linarith
[STEP] have h_simple_increment := (generated_spec_loop_simple_increment head tail threshold score coins).right h_head_ge_threshold
[STEP] have h_sum_perm: score + head = head + score := by
[STEP]   linarith
[STEP] use 1
[STEP] simp
[STEP] simp [h_threshold_lt_head_score]
[STEP] simp [h_simple_increment]
[STEP] simp [←h_sum_perm]
[STEP] intro i h_1_le_1 h_i_le_1
[STEP] linarith
[STEP] -- Case 2: where head + score < threshold
have h_simple_increment := (generated_spec_loop_simple_increment head tail threshold score coins).left
[STEP] simp [h_simple_increment (by linarith)] at h_within_threshold
[STEP] by_cases h_tail_len_0: tail.length ≤ 0
[STEP] -- Case 2.1: where tail.length ≤ 0
rw [Nat.le_zero] at h_tail_len_0
[STEP] have h_tail_nil := List.eq_nil_of_length_eq_zero h_tail_len_0
[STEP] simp [h_tail_nil] at h_within_threshold
[STEP] simp [generated_spec.loop] at h_within_threshold
[STEP] -- Case 2.2: where tail.length > 0
have h_tail_len_gt_0: tail.length > 0 := by
[STEP]   linarith
[STEP] simp [h_tail_len_gt_0] at ih
[STEP] specialize ih (head + score) coins
[STEP] simp [h_within_threshold ] at ih
[STEP] -- i₁
obtain ⟨i₁, i₁h⟩ := ih
[STEP] -- h_1_le_i', h_i'_le_len, h_to_prove
use i₁ + 1
[STEP] intro h_1_le_i'
[STEP] intro h_score_head_ge_threshold
[STEP] simp [h_simple_increment (by linarith)]
[STEP] have h_perm_sum': score + (head + (List.take i₁ tail).sum) = head + score + (List.take i₁ tail).sum := by
[STEP]   linarith
[STEP] simp [h_perm_sum']
[STEP] intro h_to_prove
[STEP] simp at h_1_le_i'
[STEP] by_cases h_1_le_i'_lt_i₁: 1 ≤ i₁
[STEP] -- Case 3: where 1 ≤ i₁
simp [h_1_le_i'_lt_i₁] at i₁h
[STEP] simp [h_1_le_i'] at i₁h
[STEP] by_cases h_threshold_head_score_i₁: threshold ≤ head + score + (List.take i₁ tail).sum
[STEP] -- Case 3.1: where threshold ≤ head + score + (List.take i₁ tail).sum
simp [h_threshold_head_score_i₁] at i₁h
[STEP] simp [h_to_prove] at i₁h
[STEP] intro i
[STEP] intro h_1_le_i
[STEP] intro h_i_lt_i₁_plus_1
[STEP] -- Case 3.1.1: where i < i₁
set i' := i - 1
[STEP] have h_1_le_i_plus_1: i = i' + 1 := by
[STEP]   simp [i']
[STEP]   rw [Nat.sub_add_cancel]
[STEP]   linarith
[STEP] simp [h_1_le_i_plus_1]
[STEP] simp [h_1_le_i_plus_1] at h_i_lt_i₁_plus_1
[STEP] by_cases h_1_le_i': 1 ≤ i'

[LAST STEP]
have h_i₁_h := i₁h i' h_1_le_i' h_i_lt_i₁_plus_1
[SUCCESS]
[END]

`example_assistant`
[RUN TACTIC]
rw [←Int.add_assoc]
[END]


`example_user`
Goals to prove:
[GOALS]
[GOAL] 1
impl (y * y) y = true
[HYPOTHESES] 1
[HYPOTHESIS] impl : ℤ → ℤ → Bool
[HYPOTHESIS] h_prob_spec : ∀ (x y : ℤ), problem_spec impl x y
[HYPOTHESIS] x y : ℤ
[HYPOTHESIS] h_specialized_spec : problem_spec impl x y
[HYPOTHESIS] h : x = y * y

[GOAL] 2
impl x y = decide (x = y * y)
[HYPOTHESES] 1
[HYPOTHESIS] impl : ℤ → ℤ → Bool
[HYPOTHESIS] h_prob_spec : ∀ (x y : ℤ), problem_spec impl x y
[HYPOTHESIS] x y : ℤ
[HYPOTHESIS] h_specialized_spec : problem_spec impl x y
[HYPOTHESIS] h : ¬x = y * y

[GOAL] 3
(∀ (x y : ℤ), generated_spec impl x y) → ∀ (x y : ℤ), problem_spec impl x y
[HYPOTHESES] 1
[HYPOTHESIS] impl : ℤ → ℤ → Bool

[STEPS]
[STEP] intro impl
[STEP] apply Iff.intro
[STEP] intro h_prob_spec
[STEP] intro x y
[STEP] have h_specialized_spec := h_prob_spec x y
[STEP] simp [generated_spec]
[STEP] by_cases h: x = y * y

[LAST STEP]
simp [h]
[SUCCESS]
[END]

`example_assistant`
[RUN TACTIC]
simp [problem_spec] at h_specialized_spec
[END]


`example_user`
Goals to prove:
[GOALS]
[GOAL] 1
impl x y = false
[HYPOTHESES] 1
[HYPOTHESIS] impl : ℤ → ℤ → Bool
[HYPOTHESIS] h_prob_spec : ∀ (x y : ℤ), problem_spec impl x y
[HYPOTHESIS] x y : ℤ
[HYPOTHESIS] h : ¬x = y * y
[HYPOTHESIS] h_specialized_spec : impl x y = true ↔ x = y ^ 2

[GOAL] 2
(∀ (x y : ℤ), generated_spec impl x y) → ∀ (x y : ℤ), problem_spec impl x y
[HYPOTHESES] 1
[HYPOTHESIS] impl : ℤ → ℤ → Bool

[STEPS]
[STEP] intro impl
[STEP] apply Iff.intro
[STEP] intro h_prob_spec
[STEP] intro x y
[STEP] have h_specialized_spec := h_prob_spec x y
[STEP] simp [generated_spec]
[STEP] by_cases h: x = y * y
[STEP] simp [h]
[STEP] simp [problem_spec] at h_specialized_spec
[STEP] rw [h] at h_specialized_spec
[STEP] simp [h_specialized_spec]
[STEP] ring
[STEP] simp [h]

[LAST STEP]
simp [problem_spec] at h_specialized_spec
[SUCCESS]
[END]

`example_assistant`
[RUN TACTIC]
have h_eq: y ^ 2 = y * y := by
[END]


`example_user`
Goals to prove:
[GOALS]
[DESCRIPTION]
IMPORTANT NOTE: Working on the sub-goal with have tactic:
have h_eq: y ^ 2 = y * y := by.

[GOAL] 1
y ^ 2 = y * y
[HYPOTHESES] 1
[HYPOTHESIS] impl : ℤ → ℤ → Bool
[HYPOTHESIS] h_prob_spec : ∀ (x y : ℤ), problem_spec impl x y
[HYPOTHESIS] x y : ℤ
[HYPOTHESIS] h : ¬x = y * y
[HYPOTHESIS] h_specialized_spec : impl x y = true ↔ x = y ^ 2

[STEPS]
[STEP] intro impl
[STEP] apply Iff.intro
[STEP] intro h_prob_spec
[STEP] intro x y
[STEP] have h_specialized_spec := h_prob_spec x y
[STEP] simp [generated_spec]
[STEP] by_cases h: x = y * y
[STEP] simp [h]
[STEP] simp [problem_spec] at h_specialized_spec
[STEP] rw [h] at h_specialized_spec
[STEP] simp [h_specialized_spec]
[STEP] ring
[STEP] simp [h]
[STEP] simp [problem_spec] at h_specialized_spec

[LAST STEP]
have h_eq: y ^ 2 = y * y := by
[SUCCESS]
[END]

`example_assistant`
[RUN TACTIC]
ring
[END]

`example_user`
Goals to prove:
[GOALS]
[GOAL] 1
generated_spec impl x y
[HYPOTHESES] 1
[HYPOTHESIS] impl : ℤ → ℤ → Bool
[HYPOTHESIS] h_prob_spec : ∀ (x y : ℤ), problem_spec impl x y
[HYPOTHESIS] x y : ℤ

[STEPS]
[STEP] intro impl
[STEP] apply Iff.intro
[STEP] intro h_prob_spec

[LAST STEP]
intro x y
[SUCCESS]
[END]

`example_assistant`
[RUN TACTIC]
have h_specialized_spec := h_prob_spec x y
[END]

`example_user`
Goals to prove:
[GOALS]
[GOAL] 1
∃ result, impl x y = result ∧ (result = true ↔ x = y ^ 2)
[HYPOTHESES] 1
[HYPOTHESIS] impl : ℤ → ℤ → Bool
[HYPOTHESIS] h_gen_spec : ∀ (x y : ℤ), generated_spec impl x y
[HYPOTHESIS] x y : ℤ

[STEPS]
[STEP] intro impl
[STEP] apply Iff.intro
[STEP] intro h_gen_spec
[STEP] intro x y
[STEP] unfold problem_spec
[STEP] simp only

[LAST STEP]
use y * y = x
[ERROR MESSAGE]
The proof-step does NOT simplify the goal. Try stepping back with different proof-step.
[END]

`example_assistant`
[RUN TACTIC]
-- let's use generic implementation rather than specific implementation 
use (impl x y)
[END]

`example_user`
Goals to prove:
[GOALS]
[GOAL] 1
impl x y = true ↔ x = y ^ 2
[HYPOTHESES] 1
[HYPOTHESIS] impl : ℤ → ℤ → Bool
[HYPOTHESIS] h_gen_spec : ∀ (x y : ℤ), generated_spec impl x y
[HYPOTHESIS] x y : ℤ

[STEPS]
[STEP] intro impl
[STEP] apply Iff.intro
[STEP] intro h_gen_spec
[STEP] intro x y
[STEP] unfold problem_spec
[STEP] simp only
[STEP] use (impl x y)
[STEP] simp

[LAST STEP]
simp
[SUCCESS]
[END]

`example_assistant`
[RUN TACTIC]
-- it is not possible to further simplify the goal without using the generated_spec, so let's expand it and see how it looks like
unfold generated_spec at h_gen_spec
[END]

`example_user`
Goals to prove:
[GOALS]
[GOAL] 1
(∀ (x y : ℤ), problem_spec impl x y) → ∀ (x y : ℤ), generated_spec impl x y

[STEPS]
[STEP] intro impl
[STEP] apply Iff.intro
[STEP] intro h_gen_spec
[STEP] intro x y
[STEP] unfold problem_spec
[STEP] simp only
[STEP] use (impl x y)
[STEP] simp
[STEP] unfold generated_spec at h_gen_spec
[STEP] have h_specialized_spec := h_gen_spec x y
[STEP] simp [h_specialized_spec]
[STEP] apply Iff.intro
[STEP] intro h_y_times_y
[STEP] linarith
[STEP] intro h_y_square
[STEP] simp [h_y_square]

[LAST STEP]
ring
[SUCCESS]
[END]

`example_assistant`
[RUN TACTIC]
-- we need to prove the reverse direction, so let's introduce the problem_spec
intro h_prob_spec
[END]

`conv end`