`example_user`
[FUNCTION IMPLEMENTATION]
def implementation (score_changes: List Int) (threshold: Int) : Nat :=
let rec loop (score_changes: List Int) (threshold: Int) (score: Int) (coins: Nat) : Nat :=
  match score_changes with
  | [] => coins
  | head :: tail =>
    let score' := head + score
    let coins' := if score' ≥ threshold then coins + 1 else coins
    loop tail threshold score' coins'
loop score_changes threshold 0 0
[END]

[PREVIOUS LEMMAS]
-- N/A
[END]

[CURRENT LEMMA]
lemma implementation_loop_threshold_invariant
(score_changes: List Int)
(threshold: Int)
(score: Int)
(coins: Nat)
(k: Int)
(h_rounds_played: score_changes.length > 0)
: implementation.loop score_changes (threshold - k) score coins
= implementation.loop score_changes threshold (score + k) coins := by
sorry
[END]

[PLAN]
Prove an `implementation_loop_threshold_invariant` lemma that states that for all integers `k`, decreasing the threshold by `k` yields the same output of `implementation.loop` as increasing the score by `k`.
  - Use induction and break the proof up into cases based on whether the head plus the cumulative score reaches the threshold.
[END]

`example_assistant`
lemma implementation_loop_threshold_invariant
(score_changes: List Int)
(threshold: Int)
(score: Int)
(coins: Nat)
(k: Int)
(h_rounds_played: score_changes.length > 0)
: implementation.loop score_changes (threshold - k) score coins
= implementation.loop score_changes threshold (score + k) coins := by
induction' score_changes generalizing score coins
simp at h_rounds_played
rename_i head tail ih
by_cases h_head_ge_threshold: head + score ≥ threshold - k
-- case where head + score ≥ threshold
simp [implementation.loop]
have h_head_ge_threshold': threshold ≤ head + score + k := by
  linarith
simp [h_head_ge_threshold']
have h_head_ge_threshold'': threshold ≤ head + (score + k) := by
  linarith
simp [h_head_ge_threshold'']
simp [←Int.add_assoc]
by_cases h_tail_len_0: tail.length ≤ 0
-- case where tail.length ≤ 0
rw [Nat.le_zero] at h_tail_len_0
have h_tail_nil := List.eq_nil_of_length_eq_zero h_tail_len_0
simp [h_tail_nil]
simp [implementation.loop]
-- case where tail.length > 0
have h_tail_len_gt_0: tail.length > 0 := by linarith
simp [h_tail_len_gt_0] at ih
specialize ih (head + score) (coins + 1)
simp [←ih]
-- case where head + score < threshold
have h_perm': head + score + k = head + (score + k) := by linarith
by_cases h_tail_len_0: tail.length ≤ 0
rw [Nat.le_zero] at h_tail_len_0
have h_tail_nil := List.eq_nil_of_length_eq_zero h_tail_len_0
simp [h_tail_nil]
simp [implementation.loop]
rw [h_perm']
have h_tail_len_gt_0: tail.length > 0 := by linarith
simp [h_tail_len_gt_0] at ih
specialize ih (head + score) coins
simp [implementation.loop]
simp at h_head_ge_threshold
have h_head_lt_threshold: ¬ (threshold ≤ head + score + k) := by
  linarith
rw [←h_perm']
simp [h_head_lt_threshold]
simp [ih]

`example_user`
[FUNCTION IMPLEMENTATION]
def implementation (score_changes: List Int) (threshold: Int) : Nat :=
let rec loop (score_changes: List Int) (threshold: Int) (score: Int) (coins: Nat) : Nat :=
  match score_changes with
  | [] => coins
  | head :: tail =>
    let score' := head + score
    let coins' := if score' ≥ threshold then coins + 1 else coins
    loop tail threshold score' coins'
loop score_changes threshold 0 0
[END]

[PREVIOUS LEMMAS]
lemma implementation_loop_threshold_invariant
(score_changes: List Int)
(threshold: Int)
(score: Int)
(coins: Nat)
(k: Int)
(h_rounds_played: score_changes.length > 0)
: implementation.loop score_changes (threshold - k) score coins
= implementation.loop score_changes threshold (score + k) coins := by
sorry
[END]

[CURRENT LEMMA]
lemma implementation_loop_simple_increment
(head: Int)
(score_changes_tail: List Int)
(threshold: Int)
(score: Int)
(coins: Nat)
: (head + score < threshold →
implementation.loop (head :: score_changes_tail) threshold score coins =
implementation.loop (score_changes_tail) threshold (head + score) coins) ∧
(head + score ≥ threshold →
implementation.loop (head :: score_changes_tail) threshold score coins =
1 + implementation.loop (score_changes_tail) threshold (head + score) coins) := by
sorry
[END]

[PLAN]
Prove an `implementation_loop_simple_increment` lemma that compares the value of `implementation.loop` across one iteration. It will either stay constant or increase by 1, depending on whether the score reaches the threshold; this lemma should prove both cases.
  - For the second case, use induction and break the proof up into cases based on whether the head plus the next head plus the cumulative score reaches the threshold.
[END]

`example_assistant`
lemma implementation_loop_simple_increment
(head: Int)
(score_changes_tail: List Int)
(threshold: Int)
(score: Int)
(coins: Nat)
: (head + score < threshold →
implementation.loop (head :: score_changes_tail) threshold score coins =
implementation.loop (score_changes_tail) threshold (head + score) coins) ∧
(head + score ≥ threshold →
implementation.loop (head :: score_changes_tail) threshold score coins =
1 + implementation.loop (score_changes_tail) threshold (head + score) coins) := by
apply And.intro
intros h_head_lt_threshold
simp [implementation.loop]
have h_head_lt_threshold': ¬ (threshold ≤ head + score) := by
  linarith
simp [h_head_lt_threshold']
rw [Int.add_comm]
intros h_head_ge_threshold
simp [implementation.loop]
have h_head_ge_threshold': threshold ≤ head + score := by
  linarith
simp [h_head_ge_threshold']
clear h_head_ge_threshold h_head_ge_threshold'
induction' score_changes_tail generalizing score coins
simp [implementation.loop]
rw [Nat.add_comm]
rename_i head' tail' ih
simp [implementation.loop]
specialize ih (head' + score)
rw [←Int.add_assoc] at ih
by_cases h_threshold_lt_score_head_head': threshold ≤ head + head' + score
-- case where threshold ≤ head + head' + score
have h_threshold_lt_score_head_head'': threshold ≤ head' + score + head := by
  linarith
have h_threshold_lt_score_head_head''': threshold ≤ head' + head + score := by
  linarith
simp [←Int.add_assoc]
simp [h_threshold_lt_score_head_head', h_threshold_lt_score_head_head'', h_threshold_lt_score_head_head''']
specialize ih (coins + 1)
simp [←ih]
have h_sum_perm: head + head' + score = head' + head + score:= by linarith
rw [h_sum_perm]
-- case where head + head' + score < threshold
simp [←Int.add_assoc]
have h_threshold_lt_score_head_head'': ¬ (threshold ≤ head' + head + score) := by
  linarith
have h_threshold_lt_score_head_head''': ¬ (threshold ≤ head' + score + head) := by
  linarith
simp [h_threshold_lt_score_head_head'', h_threshold_lt_score_head_head''']
specialize ih coins
have h_sum_perm: head' + head + score = head + score + head' := by linarith
simp [h_sum_perm]
simp [←ih]
have h_sum_perm: head + score + head' = head + head' + score := by linarith
rw [h_sum_perm]

`example_user`
[FUNCTION IMPLEMENTATION]
def implementation (score_changes: List Int) (threshold: Int) : Nat :=
let rec loop (score_changes: List Int) (threshold: Int) (score: Int) (coins: Nat) : Nat :=
  match score_changes with
  | [] => coins
  | head :: tail =>
    let score' := head + score
    let coins' := if score' ≥ threshold then coins + 1 else coins
    loop tail threshold score' coins'
loop score_changes threshold 0 0
[END]

[PREVIOUS LEMMAS]
lemma implementation_loop_threshold_invariant
(score_changes: List Int)
(threshold: Int)
(score: Int)
(coins: Nat)
(k: Int)
(h_rounds_played: score_changes.length > 0)
: implementation.loop score_changes (threshold - k) score coins
= implementation.loop score_changes threshold (score + k) coins := by
sorry

lemma implementation_loop_simple_increment
(head: Int)
(score_changes_tail: List Int)
(threshold: Int)
(score: Int)
(coins: Nat)
: (head + score < threshold →
implementation.loop (head :: score_changes_tail) threshold score coins =
implementation.loop (score_changes_tail) threshold (head + score) coins) ∧
(head + score ≥ threshold →
implementation.loop (head :: score_changes_tail) threshold score coins =
1 + implementation.loop (score_changes_tail) threshold (head + score) coins) := by
sorry
[END]

[CURRENT LEMMA]
lemma implementation_loop_coin_monotonic_increasing
(score_changes: List Int)
(threshold: Int)
(score: Int)
(coins: Nat)
(h_rounds_played: score_changes.length > 0)
: coins ≤ implementation.loop score_changes threshold score coins := by
sorry
[END]

[PLAN]
Prove an `implementation_loop_coin_monotonic_increasing` lemma that states that the output of `implementation.loop` will always be greater then or equal to the coin count input.
  - Use induction and break the proof up into cases based on whether the head plus the cumulative score reaches the threshold.
[END]

`example_assistant`
lemma implementation_loop_coin_monotonic_increasing
(score_changes: List Int)
(threshold: Int)
(score: Int)
(coins: Nat)
(h_rounds_played: score_changes.length > 0)
: coins ≤ implementation.loop score_changes threshold score coins := by
induction' score_changes generalizing score coins
simp at h_rounds_played
rename_i head tail ih
by_cases h_head_ge_threshold: head + score ≥ threshold
-- case where head + score ≥ threshold
have h_head_ge_threshold':= (implementation_loop_simple_increment head tail threshold score coins).right h_head_ge_threshold
rw [h_head_ge_threshold']
clear h_head_ge_threshold'
simp [implementation.loop]
by_cases h_tail_len_0: tail.length ≤ 0
rw [Nat.le_zero] at h_tail_len_0
have h_tail_nil := List.eq_nil_of_length_eq_zero h_tail_len_0
simp [h_tail_nil]
simp [implementation.loop]
have h_tail_len_gt_0: tail.length > 0 := by linarith
simp [h_tail_len_gt_0] at ih
have ih'_head_ge_threshold := ih (head + score) coins
linarith
-- case where head + score < threshold
simp [implementation.loop]
simp [h_head_ge_threshold]
by_cases h_tail_len_0: tail.length ≤ 0
rw [Nat.le_zero] at h_tail_len_0
have h_tail_nil := List.eq_nil_of_length_eq_zero h_tail_len_0
simp [h_tail_nil]
simp [implementation.loop]
have h_tail_len_gt_0: tail.length > 0 := by linarith
simp [h_tail_len_gt_0] at ih
have ih'_head_lt_threshold := ih (head + score) coins
linarith

`example_user`
[FUNCTION IMPLEMENTATION]
def implementation (score_changes: List Int) (threshold: Int) : Nat :=
let rec loop (score_changes: List Int) (threshold: Int) (score: Int) (coins: Nat) : Nat :=
  match score_changes with
  | [] => coins
  | head :: tail =>
    let score' := head + score
    let coins' := if score' ≥ threshold then coins + 1 else coins
    loop tail threshold score' coins'
loop score_changes threshold 0 0
[END]

[PREVIOUS LEMMAS]
lemma implementation_loop_threshold_invariant
(score_changes: List Int)
(threshold: Int)
(score: Int)
(coins: Nat)
(k: Int)
(h_rounds_played: score_changes.length > 0)
: implementation.loop score_changes (threshold - k) score coins
= implementation.loop score_changes threshold (score + k) coins := by
sorry

lemma implementation_loop_simple_increment
(head: Int)
(score_changes_tail: List Int)
(threshold: Int)
(score: Int)
(coins: Nat)
: (head + score < threshold →
implementation.loop (head :: score_changes_tail) threshold score coins =
implementation.loop (score_changes_tail) threshold (head + score) coins) ∧
(head + score ≥ threshold →
implementation.loop (head :: score_changes_tail) threshold score coins =
1 + implementation.loop (score_changes_tail) threshold (head + score) coins) := by
sorry

lemma implementation_loop_coin_monotonic_increasing
(score_changes: List Int)
(threshold: Int)
(score: Int)
(coins: Nat)
(h_rounds_played: score_changes.length > 0)
: coins ≤ implementation.loop score_changes threshold score coins := by
sorry
[END]

[CURRENT LEMMA]
lemma implementation_loop_invariant_stop
(score_changes: List Int)
(threshold: Int)
(score: Int)
(coins: Nat)
(h_rounds_played: score_changes.length > 0)
(h_within_threshold: coins = implementation.loop score_changes threshold score coins)
: ∀ i, 1 ≤ i ∧ i ≤ score_changes.length →
score + (score_changes.take i).sum < threshold := by
sorry
[END]

[PLAN]
Prove an `implementation_loop_invariant_stop` lemma that states that if the output of `implementation.loop` is exactly equal to the coin count input, then for all indices `i`, the input score plus the prefix sum of the score changes list up to index `i` must be less than the threshold.
  - Use induction and break the proof up into cases based on whether the head plus the cumulative score reaches the threshold.
  - For each case, break the proof up into more cases based on whether the tail has positive length.
  - Use the `implementation_loop_simple_increment` and `implementation_loop_coin_monotonic_increasing` lemmas in the proof.
[END]

`example_assistant`
lemma implementation_loop_invariant_stop
(score_changes: List Int)
(threshold: Int)
(score: Int)
(coins: Nat)
(h_rounds_played: score_changes.length > 0)
(h_within_threshold: coins = implementation.loop score_changes threshold score coins)
: ∀ i, 1 ≤ i ∧ i ≤ score_changes.length →
score + (score_changes.take i).sum < threshold := by
induction' score_changes generalizing score coins
simp at h_rounds_played
rename_i head tail ih
by_cases h_head_ge_threshold: head + score ≥ threshold
-- Case 1: case where head + score ≥ threshold
have h_head_ge_threshold':= (implementation_loop_simple_increment head tail threshold score coins).right h_head_ge_threshold
rw [h_head_ge_threshold'] at h_within_threshold
clear h_head_ge_threshold'
-- Case 1.1: case where tail.length ≤ 0
by_cases h_tail_len_0: tail.length ≤ 0
rw [Nat.le_zero] at h_tail_len_0
have h_tail_nil := List.eq_nil_of_length_eq_zero h_tail_len_0
simp [h_tail_nil] at h_within_threshold
simp [implementation.loop] at h_within_threshold
-- Case 1.2: case where tail.length > 0
have h_tail_len_gt_0: tail.length > 0 := by linarith
have h_coins_monotonic := implementation_loop_coin_monotonic_increasing tail threshold (head + score) coins h_tail_len_gt_0
linarith
-- Case 2: where head + score < threshold
by_cases h_tail_len_0: tail.length ≤ 0
-- Case 2.1: case where tail.length ≤ 0
rw [Nat.le_zero] at h_tail_len_0
have h_tail_nil := List.eq_nil_of_length_eq_zero h_tail_len_0
simp [h_tail_nil]
intro i h_1_le_1 h_i_le_1
have h_i_eq_1 := Nat.le_antisymm h_i_le_1 h_1_le_1
simp [h_i_eq_1]
simp at h_head_ge_threshold
linarith
-- Case 2.2: case where tail.length > 0
simp at h_head_ge_threshold
have h_tail_len_gt_0: tail.length > 0 := by linarith
have h_head_lt_threshold := (implementation_loop_simple_increment head tail threshold score coins).left h_head_ge_threshold
rw [h_head_lt_threshold] at h_within_threshold
simp [h_tail_len_gt_0] at ih
specialize ih (head + score) coins
apply ih at h_within_threshold
intro i h_1_le_i
set i' := i - 1
have h_i_eq_i'_add_1: i = i' + 1 := by
  simp [i']
  rw [Nat.sub_add_cancel]
  linarith
simp [h_i_eq_i'_add_1]
have h_sum_perm: score + (head + (List.take i' tail).sum) = head + score + (List.take i' tail).sum := by
  linarith
simp [h_sum_perm]
have h_i'_le_tail_len: i' ≤ tail.length := by
  simp [i']
  have h_temp':= h_1_le_i.right
  simp at h_temp'
  assumption
specialize h_within_threshold i'
by_cases h_1_le_i': 1 ≤ i'
-- Case 3: where 1 ≤ i'
simp [h_1_le_i'] at h_within_threshold
simp [h_i'_le_tail_len] at h_within_threshold
assumption
-- Case 3.1: where i' < 1
simp at h_1_le_i'
simp [h_1_le_i']
assumption

`example_user`
[FUNCTION IMPLEMENTATION]
def implementation (score_changes: List Int) (threshold: Int) : Nat :=
let rec loop (score_changes: List Int) (threshold: Int) (score: Int) (coins: Nat) : Nat :=
  match score_changes with
  | [] => coins
  | head :: tail =>
    let score' := head + score
    let coins' := if score' ≥ threshold then coins + 1 else coins
    loop tail threshold score' coins'
loop score_changes threshold 0 0
[END]

[PREVIOUS LEMMAS]
lemma implementation_loop_threshold_invariant
(score_changes: List Int)
(threshold: Int)
(score: Int)
(coins: Nat)
(k: Int)
(h_rounds_played: score_changes.length > 0)
: implementation.loop score_changes (threshold - k) score coins
= implementation.loop score_changes threshold (score + k) coins := by
sorry

lemma implementation_loop_simple_increment
(head: Int)
(score_changes_tail: List Int)
(threshold: Int)
(score: Int)
(coins: Nat)
: (head + score < threshold →
implementation.loop (head :: score_changes_tail) threshold score coins =
implementation.loop (score_changes_tail) threshold (head + score) coins) ∧
(head + score ≥ threshold →
implementation.loop (head :: score_changes_tail) threshold score coins =
1 + implementation.loop (score_changes_tail) threshold (head + score) coins) := by
sorry

lemma implementation_loop_coin_monotonic_increasing
(score_changes: List Int)
(threshold: Int)
(score: Int)
(coins: Nat)
(h_rounds_played: score_changes.length > 0)
: coins ≤ implementation.loop score_changes threshold score coins := by
sorry

lemma implementation_loop_invariant_stop
(score_changes: List Int)
(threshold: Int)
(score: Int)
(coins: Nat)
(h_rounds_played: score_changes.length > 0)
(h_within_threshold: coins = implementation.loop score_changes threshold score coins)
: ∀ i, 1 ≤ i ∧ i ≤ score_changes.length →
score + (score_changes.take i).sum < threshold := by
sorry
[END]

[CURRENT LEMMA]
lemma implementation_loop_invariant_continue
(score_changes: List Int)
(threshold: Int)
(score: Int)
(coins: Nat)
(h_rounds_played: score_changes.length > 0)
(h_within_threshold: coins < implementation.loop score_changes threshold score coins)
:∃ i', 1 ≤ i' ∧ i' ≤ score_changes.length →
(score + (score_changes.take i').sum ≥ threshold) →
implementation.loop score_changes threshold score coins =
1 + implementation.loop (score_changes.drop i') threshold
(score + (score_changes.take i').sum) coins →
∀ i, 1 ≤ i ∧ i < i' → score + (score_changes.take i).sum < threshold := by
sorry
[END]

[PLAN]
Prove an `implementation_loop_invariant_continue` lemma that states that if the output of `implementation.loop` is strictly greater than the coin count input, then there exists an index `i'` at which the coin count output by `implementation.loop` increased by 1 and all previous indices `i` did not change the coin count output of `implementation.loop`.
  - Use induction and break the proof up into cases based on whether the head plus the cumulative score reaches the threshold.
  - For the second case, break the proof up into more cases based on whether the tail has positive length.
  - Use the `implementation_loop_simple_increment` lemma in the proof.
[END]

`example_assistant`
lemma implementation_loop_invariant_continue
(score_changes: List Int)
(threshold: Int)
(score: Int)
(coins: Nat)
(h_rounds_played: score_changes.length > 0)
(h_within_threshold: coins < implementation.loop score_changes threshold score coins)
:∃ i', 1 ≤ i' ∧ i' ≤ score_changes.length →
(score + (score_changes.take i').sum ≥ threshold) →
implementation.loop score_changes threshold score coins =
1 + implementation.loop (score_changes.drop i') threshold
(score + (score_changes.take i').sum) coins →
∀ i, 1 ≤ i ∧ i < i' → score + (score_changes.take i).sum < threshold := by
induction' score_changes generalizing score coins
simp at h_rounds_played
rename_i head tail ih
by_cases h_head_ge_threshold: head + score ≥ threshold
-- Case 1: where head + score ≥ threshold
have h_threshold_lt_head_score: threshold ≤ score + head := by linarith
have h_simple_increment := (implementation_loop_simple_increment head tail threshold score coins).right h_head_ge_threshold
have h_sum_perm: score + head = head + score := by linarith
use 1
simp
simp [h_threshold_lt_head_score]
simp [h_simple_increment]
simp [←h_sum_perm]
intro i h_1_le_1 h_i_le_1
linarith
-- Case 2: where head + score < threshold
have h_simple_increment := (implementation_loop_simple_increment head tail threshold score coins).left
simp [h_simple_increment (by linarith)] at h_within_threshold
by_cases h_tail_len_0: tail.length ≤ 0
-- Case 2.1: where tail.length ≤ 0
rw [Nat.le_zero] at h_tail_len_0
have h_tail_nil := List.eq_nil_of_length_eq_zero h_tail_len_0
simp [h_tail_nil] at h_within_threshold
simp [implementation.loop] at h_within_threshold
-- Case 2.2: where tail.length > 0
have h_tail_len_gt_0: tail.length > 0 := by linarith
simp [h_tail_len_gt_0] at ih
specialize ih (head + score) coins
simp [h_within_threshold ] at ih
-- i₁
obtain ⟨i₁, i₁h⟩ := ih
-- h_1_le_i', h_i'_le_len, h_to_prove
use i₁ + 1
intro h_1_le_i'
intro h_score_head_ge_threshold
simp [h_simple_increment (by linarith)]
have h_perm_sum': score + (head + (List.take i₁ tail).sum) = head + score + (List.take i₁ tail).sum := by
  linarith
simp [h_perm_sum']
intro h_to_prove
simp at h_1_le_i'
by_cases h_1_le_i'_lt_i₁: 1 ≤ i₁
-- Case 3: where 1 ≤ i₁
simp [h_1_le_i'_lt_i₁] at i₁h
simp [h_1_le_i'] at i₁h
by_cases h_threshold_head_score_i₁: threshold ≤ head + score + (List.take i₁ tail).sum
-- Case 3.1: where threshold ≤ head + score + (List.take i₁ tail).sum
simp [h_threshold_head_score_i₁] at i₁h
simp [h_to_prove] at i₁h
intro i
intro h_1_le_i
intro h_i_lt_i₁_plus_1
-- Case 3.1.1: where i < i₁
set i' := i - 1
have h_1_le_i_plus_1: i = i' + 1 := by
  simp [i']
  rw [Nat.sub_add_cancel]
  linarith
simp [h_1_le_i_plus_1]
simp [h_1_le_i_plus_1] at h_i_lt_i₁_plus_1
by_cases h_1_le_i': 1 ≤ i'
have h_i₁_h := i₁h i' h_1_le_i' h_i_lt_i₁_plus_1
rw [←Int.add_assoc]
rw [Int.add_comm score]
assumption
simp at h_1_le_i'
simp [h_1_le_i']
linarith
simp at h_threshold_head_score_i₁
simp at h_score_head_ge_threshold
linarith
simp at h_1_le_i'_lt_i₁
intro i h_1_le_i h_i_lt_i₁_plus_1
simp [h_1_le_i'_lt_i₁] at h_i_lt_i₁_plus_1
linarith
