`conv start`

`example_user`
[NL DESCRIPTION]
def find_magnitude(x: int) -> int
"""
Given an integer x, your task is to find the magnitude of x.
The magnitude of an integer is defined as the absolute value of the integer.
"""

[SPECIFICATION]
def problem_spec
-- function signature
(impl: Int → Int)
-- inputs
(x: Int) :=
-- spec
let spec (result: Int) :=
(result ≥ 0) ∧
(impl (-x) = result) ∧
(result = 0 ↔ x = 0) ∧
(0 ≤ x → impl (-x) + result = 2 * x) ∧
(x ≤ 0 → impl (-x) + result = -2 * x)
-- program terminates
∃ result, impl x = result ∧
-- return value satisfies spec
spec result

[IMPLEMENTATION]
def implementation (x: Int) : Int :=
if x < 0 then -x else x

[CORRECTNESS THEOREM]
theorem correctness
(x: Int)
: problem_spec implementation x :=


`example_assistant`
[THOUGHTS]
We can start by unfolding the `problem_spec` and assigning the implementation's output to a temporary variable `result`.
Early on, we will want to break the proof up into cases based on whether `x` is positive, negative, or zero.
Many of the intermediate goals can likely be proven using `linarith`.
[END THOUGHTS]


[PROOF]
by
unfold problem_spec
let result := implementation x
use result
simp [result]
simp [implementation]
by_cases h_0_eq_x: x = 0
-- if x = 0 then
simp [h_0_eq_x]
by_cases h_x_lt_0: x < 0
-- if x < 0 then
simp [h_x_lt_0]
apply And.intro
linarith
apply And.intro
intro; linarith
have h_not_0_lt_x: ¬ (0 < x) := by
  linarith
intro h_x_le_0
simp [h_not_0_lt_x]
linarith
apply And.intro
simp [h_x_lt_0]
linarith
simp [h_x_lt_0]
apply And.intro
intro h_neg_x_sum
linarith
apply And.intro
have h_0_le_x: 0 ≤ x := by
  linarith
simp [h_0_le_x]
by_cases h_0_lt_x: 0 < x
-- if 0 < x then
simp [h_0_lt_x]
linarith
have h_x_eq_0: x = 0 := by
  linarith
simp [h_x_eq_0]
intro h_x_le_0
simp at h_x_lt_0
have h_x_eq_0: x = 0 := by
  linarith
contradiction
[END]

`example_user`
[NL DESCRIPTION]
def find_fibonacci(n: int) -> int
"""
Given an integer n, your task is to find the nth Fibonacci number.
The Fibonacci sequence is defined as follows:
- F(0) = 1
- F(1) = 1
- F(n) = F(n-1) + F(n-2) for n > 1
"""

[SPECIFICATION]
def problem_spec
-- function signature
(impl: Nat → Nat)
-- inputs
(n: Nat) :=
-- spec
let spec (result: Nat) :=
fibonacci_non_computable n result
-- program terminates
∃ result, impl n = result ∧
-- return value satisfies spec
spec result

[IMPLEMENTATION]
def implementation (n: Nat) : Nat :=
match n with
| 0 => 0
| 1 => 1
| n' + 2 => implementation n' + implementation (n' + 1)

[CORRECTNESS THEOREM]
theorem correctness
(n: Nat)
: problem_spec implementation n
:=


`example_assistant`
[THOUGHTS]
We should first prove a `fib_comp_to_non_comp` lemma that states that given a computable function `f : Nat → Nat` that follows the Fibonacci base cases (`f 0 = 1`, `f 1 = 1`) and recursive case (`∀ n, f (n + 2) = f n + f (n + 1)`), the built-in Lean 4 function `fibonacci_non_computable` called on `n` and `(f n)` outputs `True` (for all `n`).
Use induction and break the proof up into the base cases and the recursive case.
We can then prove the `correctness` theorem.
Start by unfolding the `problem_spec` and assigning the implementation's output to a temporary variable `result`.
Use the `have` keyword three times to show that `implementation` follows the three properties of the Fibonacci function:
  - `implementation 0 = 1`
  - `implementation 1 = 1`
  - `∀ n', implementation (n' + 2) = implementation n' + implementation (n' + 1)`
Then use these three hypotheses and the `fib_comp_to_non_comp` lemma to show that `implementation` satisfies `fibonacci_non_computable`, as required by the `spec`.
[END THOUGHTS]


[HELPER LEMMAS]
theorem fib_comp_to_non_comp (n : ℕ)
(f : Nat → Nat)
(h_f_0: f 0 = 0)
(h_f_1: f 1 = 1)
(h_f_step: ∀ n, f (n + 2) = f n + f (n + 1))
: fibonacci_non_computable n (f n) :=
by
induction' n using Nat.strong_induction_on with n' ih
by_cases h_n'_lt_1: n' < 2
-- if n' < 2 then
have h_n'_eq_0: n' = 0 ∨ n' = 1 := by
  interval_cases n'
  all_goals simp
cases h_n'_eq_0
rename_i h_n'_eq_0
simp [h_n'_eq_0, h_f_0, fibonacci_non_computable.base0]
rename_i h_n'_eq_1
simp [h_n'_eq_1, h_f_1, fibonacci_non_computable.base1]
set n'' := n' - 2
have h_n''_eq_n_plus_2: n' = n'' + 2 := by
  rw [Nat.sub_add_cancel]
  linarith
have h_n''_lt_n': n'' < n' := by
  linarith
have h_fib_n'':= h_f_step n''
have h_fib_n''_non_computable := ih n'' h_n''_lt_n'
have h_fib_n''_plus_1_non_computable := ih (n'' + 1) (by linarith)
have h_fib_n''_plus_2_non_computable :=
  fibonacci_non_computable.step _ _ _ h_fib_n''_non_computable h_fib_n''_plus_1_non_computable
rw [←h_fib_n''] at h_fib_n''_plus_2_non_computable
rw [←h_n''_eq_n_plus_2] at h_fib_n''_plus_2_non_computable
assumption
[END LEMMAS]

[PROOF]
by
unfold problem_spec
let result := implementation n
use result
simp [result]
have h_impl_n : ∀ n', implementation (n' + 2) = implementation n' + implementation (n' + 1) :=
by
  intro n'
  rw [implementation]
have h_impl_0 : implementation 0 = 0 := by
  rw [implementation]
have h_impl_1 : implementation 1 = 1 := by
  rw [implementation]
apply fib_comp_to_non_comp
all_goals assumption
[END]

`example_user`
[NL DESCRIPTION]
def coins_won(score_changes: List[int], threshold: int) -> int
"""
In a game, a player's score starts at 0 and is updated round by round using values from the list
score_changes (where positive numbers add to the score and negative numbers subtract).
After each round, as long as the player's cumulative score is greater than or equal to the given threshold,
the player wins a coin for that round.
Your task is to compute and return the total number of coins won by the player by the end of the game.
"""

[SPECIFICATION]
def problem_spec
-- function signature
(impl: List Int → Int → Nat)
-- inputs
(score_changes: List Int)
(threshold: Int) :=
-- spec
let spec (score_changes' : List Int) (threshold' : Int) (result: Nat) :=
score_changes'.length > 0 →
if result = 0 then
  ∀ i, 1 ≤ i ∧ i ≤ score_changes'.length →
  (score_changes'.take i).sum < threshold'
else
  (∃ i, 1 ≤ i ∧ i ≤ score_changes'.length →
  (score_changes'.take i).sum ≥ threshold' →
  ( let score_changes'' := score_changes'.drop i;
    let threshold'' := threshold' - (score_changes'.take i).sum;
    let result' := impl score_changes'' threshold'';
    result = 1 + result') →
  ∀ i', 1 ≤ i' ∧ i' < i → (score_changes'.take i').sum < threshold
  );
-- program terminates
∃ result, impl score_changes threshold = result ∧
-- return value satisfies spec
spec score_changes threshold result

[IMPLEMENTATION]
def implementation (score_changes: List Int) (threshold: Int) : Nat :=
let rec loop (score_changes: List Int) (threshold: Int) (score: Int) (coins: Nat) : Nat :=
  match score_changes with
  | [] => coins
  | head :: tail =>
    let score' := head + score
    let coins' := if score' ≥ threshold then coins + 1 else coins
    loop tail threshold score' coins'
loop score_changes threshold 0 0

[CORRECTNESS THEOREM]
theorem correctness
(score_changes: List Int)
(threshold: Int)
: problem_spec implementation score_changes threshold
:=


`example_assistant`
[THOUGHTS]
We should first prove an `implementation_loop_threshold_invariant` lemma that states that for all integers `k`, decreasing the threshold by `k` yields the same output of `implementation.loop` as increasing the score by `k`.
Use induction and break the proof up into cases based on whether the head plus the cumulative score reaches the threshold.
We should then prove an `implementation_loop_simple_increment` lemma that compares the value of `implementation.loop` across one iteration. It will either stay constant or increase by 1, depending on whether the score reaches the threshold; this lemma should prove both cases.
For the second case, use induction and break the proof up into cases based on whether the head plus the next head plus the cumulative score reaches the threshold.
We should then prove an `implementation_loop_coin_monotonic_increasing` lemma that states that the output of `implementation.loop` will always be greater then or equal to the coin count input.
Use induction and break the proof up into cases based on whether the head plus the cumulative score reaches the threshold.
We should then prove an `implementation_loop_invariant_stop` lemma that states that if the output of `implementation.loop` is exactly equal to the coin count input, then for all indices `i`, the input score plus the prefix sum of the score changes list up to index `i` must be less than the threshold.
Use induction and break the proof up into cases based on whether the head plus the cumulative score reaches the threshold.
For each case, break the proof up into more cases based on whether the tail has positive length.
Use the `implementation_loop_simple_increment` and `implementation_loop_coin_monotonic_increasing` lemmas in the proof.
We should then prove an `implementation_loop_invariant_continue` lemma that states that if the output of `implementation.loop` is strictly greater than the coin count input, then there exists an index `i'` at which the coin count output by `implementation.loop` increased by 1 and all previous indices `i` did not change the coin count output of `implementation.loop`.
Use induction and break the proof up into cases based on whether the head plus the cumulative score reaches the threshold.
For the second case, break the proof up into more cases based on whether the tail has positive length.
Use the `implementation_loop_simple_increment` lemma in the proof.
We can then prove the `correctness` theorem.
Start by unfolding the `problem_spec` and assigning the implementation's output to a temporary variable `result`.
Early on, you will want to break the proof up into cases based on whether the output of `implementation_loop` (with initial values as input) is 0.
Use the `implementation_loop_threshold_invariant`, `implementation_loop_invariant_stop`, and `implementation_loop_invariant_continue` lemmas in the proof.
[END THOUGHTS]

[HELPER LEMMAS]
lemma implementation_loop_threshold_invariant
(score_changes: List Int)
(threshold: Int)
(score: Int)
(coins: Nat)
(k: Int)
(h_rounds_played: score_changes.length > 0)
: implementation.loop score_changes (threshold - k) score coins
= implementation.loop score_changes threshold (score + k) coins :=
by
induction' score_changes generalizing score coins
simp at h_rounds_played
rename_i head tail ih
by_cases h_head_ge_threshold: head + score ≥ threshold - k
-- case where head + score ≥ threshold
simp [implementation.loop]
have h_head_ge_threshold': threshold ≤ head + score + k := by
  linarith
simp [h_head_ge_threshold']
have h_head_ge_threshold'': threshold ≤ head + (score + k) := by
  linarith
simp [h_head_ge_threshold'']
simp [←Int.add_assoc]
by_cases h_tail_len_0: tail.length ≤ 0
-- case where tail.length ≤ 0
rw [Nat.le_zero] at h_tail_len_0
have h_tail_nil := List.eq_nil_of_length_eq_zero h_tail_len_0
simp [h_tail_nil]
simp [implementation.loop]
-- case where tail.length > 0
have h_tail_len_gt_0: tail.length > 0 := by linarith
simp [h_tail_len_gt_0] at ih
specialize ih (head + score) (coins + 1)
simp [←ih]
-- case where head + score < threshold
have h_perm': head + score + k = head + (score + k) := by linarith
by_cases h_tail_len_0: tail.length ≤ 0
rw [Nat.le_zero] at h_tail_len_0
have h_tail_nil := List.eq_nil_of_length_eq_zero h_tail_len_0
simp [h_tail_nil]
simp [implementation.loop]
rw [h_perm']
have h_tail_len_gt_0: tail.length > 0 := by linarith
simp [h_tail_len_gt_0] at ih
specialize ih (head + score) coins
simp [implementation.loop]
simp at h_head_ge_threshold
have h_head_lt_threshold: ¬ (threshold ≤ head + score + k) := by
  linarith
rw [←h_perm']
simp [h_head_lt_threshold]
simp [ih]

lemma implementation_loop_simple_increment
(head: Int)
(score_changes_tail: List Int)
(threshold: Int)
(score: Int)
(coins: Nat)
: (head + score < threshold →
implementation.loop (head :: score_changes_tail) threshold score coins =
implementation.loop (score_changes_tail) threshold (head + score) coins) ∧
(head + score ≥ threshold →
implementation.loop (head :: score_changes_tail) threshold score coins =
1 + implementation.loop (score_changes_tail) threshold (head + score) coins) :=
by
apply And.intro
intros h_head_lt_threshold
simp [implementation.loop]
have h_head_lt_threshold': ¬ (threshold ≤ head + score) := by
  linarith
simp [h_head_lt_threshold']
rw [Int.add_comm]
intros h_head_ge_threshold
simp [implementation.loop]
have h_head_ge_threshold': threshold ≤ head + score := by
  linarith
simp [h_head_ge_threshold']
clear h_head_ge_threshold h_head_ge_threshold'
induction' score_changes_tail generalizing score coins
simp [implementation.loop]
rw [Nat.add_comm]
rename_i head' tail' ih
simp [implementation.loop]
specialize ih (head' + score)
rw [←Int.add_assoc] at ih
by_cases h_threshold_lt_score_head_head': threshold ≤ head + head' + score
-- case where threshold ≤ head + head' + score
have h_threshold_lt_score_head_head'': threshold ≤ head' + score + head := by
  linarith
have h_threshold_lt_score_head_head''': threshold ≤ head' + head + score := by
  linarith
simp [←Int.add_assoc]
simp [h_threshold_lt_score_head_head', h_threshold_lt_score_head_head'', h_threshold_lt_score_head_head''']
specialize ih (coins + 1)
simp [←ih]
have h_sum_perm: head + head' + score = head' + head + score:= by linarith
rw [h_sum_perm]
-- case where head + head' + score < threshold
simp [←Int.add_assoc]
have h_threshold_lt_score_head_head'': ¬ (threshold ≤ head' + head + score) := by
  linarith
have h_threshold_lt_score_head_head''': ¬ (threshold ≤ head' + score + head) := by
  linarith
simp [h_threshold_lt_score_head_head'', h_threshold_lt_score_head_head''']
specialize ih coins
have h_sum_perm: head' + head + score = head + score + head' := by linarith
simp [h_sum_perm]
simp [←ih]
have h_sum_perm: head + score + head' = head + head' + score := by linarith
rw [h_sum_perm]

lemma implementation_loop_coin_monotonic_increasing
(score_changes: List Int)
(threshold: Int)
(score: Int)
(coins: Nat)
(h_rounds_played: score_changes.length > 0)
: coins ≤ implementation.loop score_changes threshold score coins :=
by
induction' score_changes generalizing score coins
simp at h_rounds_played
rename_i head tail ih
by_cases h_head_ge_threshold: head + score ≥ threshold
-- case where head + score ≥ threshold
have h_head_ge_threshold':= (implementation_loop_simple_increment head tail threshold score coins).right h_head_ge_threshold
rw [h_head_ge_threshold']
clear h_head_ge_threshold'
simp [implementation.loop]
by_cases h_tail_len_0: tail.length ≤ 0
rw [Nat.le_zero] at h_tail_len_0
have h_tail_nil := List.eq_nil_of_length_eq_zero h_tail_len_0
simp [h_tail_nil]
simp [implementation.loop]
have h_tail_len_gt_0: tail.length > 0 := by linarith
simp [h_tail_len_gt_0] at ih
have ih'_head_ge_threshold := ih (head + score) coins
linarith
-- case where head + score < threshold
simp [implementation.loop]
simp [h_head_ge_threshold]
by_cases h_tail_len_0: tail.length ≤ 0
rw [Nat.le_zero] at h_tail_len_0
have h_tail_nil := List.eq_nil_of_length_eq_zero h_tail_len_0
simp [h_tail_nil]
simp [implementation.loop]
have h_tail_len_gt_0: tail.length > 0 := by linarith
simp [h_tail_len_gt_0] at ih
have ih'_head_lt_threshold := ih (head + score) coins
linarith

lemma implementation_loop_invariant_stop
(score_changes: List Int)
(threshold: Int)
(score: Int)
(coins: Nat)
(h_rounds_played: score_changes.length > 0)
(h_within_threshold: coins = implementation.loop score_changes threshold score coins)
: ∀ i, 1 ≤ i ∧ i ≤ score_changes.length →
score + (score_changes.take i).sum < threshold :=
by
induction' score_changes generalizing score coins
simp at h_rounds_played
rename_i head tail ih
by_cases h_head_ge_threshold: head + score ≥ threshold
-- Case 1: case where head + score ≥ threshold
have h_head_ge_threshold':= (implementation_loop_simple_increment head tail threshold score coins).right h_head_ge_threshold
rw [h_head_ge_threshold'] at h_within_threshold
clear h_head_ge_threshold'
-- Case 1.1: case where tail.length ≤ 0
by_cases h_tail_len_0: tail.length ≤ 0
rw [Nat.le_zero] at h_tail_len_0
have h_tail_nil := List.eq_nil_of_length_eq_zero h_tail_len_0
simp [h_tail_nil] at h_within_threshold
simp [implementation.loop] at h_within_threshold
-- Case 1.2: case where tail.length > 0
have h_tail_len_gt_0: tail.length > 0 := by linarith
have h_coins_monotonic := implementation_loop_coin_monotonic_increasing tail threshold (head + score) coins h_tail_len_gt_0
linarith
-- Case 2: where head + score < threshold
by_cases h_tail_len_0: tail.length ≤ 0
-- Case 2.1: case where tail.length ≤ 0
rw [Nat.le_zero] at h_tail_len_0
have h_tail_nil := List.eq_nil_of_length_eq_zero h_tail_len_0
simp [h_tail_nil]
intro i h_1_le_1 h_i_le_1
have h_i_eq_1 := Nat.le_antisymm h_i_le_1 h_1_le_1
simp [h_i_eq_1]
simp at h_head_ge_threshold
linarith
-- Case 2.2: case where tail.length > 0
simp at h_head_ge_threshold
have h_tail_len_gt_0: tail.length > 0 := by linarith
have h_head_lt_threshold := (implementation_loop_simple_increment head tail threshold score coins).left h_head_ge_threshold
rw [h_head_lt_threshold] at h_within_threshold
simp [h_tail_len_gt_0] at ih
specialize ih (head + score) coins
apply ih at h_within_threshold
intro i h_1_le_i
set i' := i - 1
have h_i_eq_i'_add_1: i = i' + 1 := by
  simp [i']
  rw [Nat.sub_add_cancel]
  linarith
simp [h_i_eq_i'_add_1]
have h_sum_perm: score + (head + (List.take i' tail).sum) = head + score + (List.take i' tail).sum := by
  linarith
simp [h_sum_perm]
have h_i'_le_tail_len: i' ≤ tail.length := by
  simp [i']
  have h_temp':= h_1_le_i.right
  simp at h_temp'
  assumption
specialize h_within_threshold i'
by_cases h_1_le_i': 1 ≤ i'
-- Case 3: where 1 ≤ i'
simp [h_1_le_i'] at h_within_threshold
simp [h_i'_le_tail_len] at h_within_threshold
assumption
-- Case 3.1: where i' < 1
simp at h_1_le_i'
simp [h_1_le_i']
assumption

lemma implementation_loop_invariant_continue
(score_changes: List Int)
(threshold: Int)
(score: Int)
(coins: Nat)
(h_rounds_played: score_changes.length > 0)
(h_within_threshold: coins < implementation.loop score_changes threshold score coins)
:∃ i', 1 ≤ i' ∧ i' ≤ score_changes.length →
(score + (score_changes.take i').sum ≥ threshold) →
implementation.loop score_changes threshold score coins =
1 + implementation.loop (score_changes.drop i') threshold
(score + (score_changes.take i').sum) coins →
∀ i, 1 ≤ i ∧ i < i' → score + (score_changes.take i).sum < threshold :=
by
induction' score_changes generalizing score coins
simp at h_rounds_played
rename_i head tail ih
by_cases h_head_ge_threshold: head + score ≥ threshold
-- Case 1: where head + score ≥ threshold
have h_threshold_lt_head_score: threshold ≤ score + head := by linarith
have h_simple_increment := (implementation_loop_simple_increment head tail threshold score coins).right h_head_ge_threshold
have h_sum_perm: score + head = head + score := by linarith
use 1
simp
simp [h_threshold_lt_head_score]
simp [h_simple_increment]
simp [←h_sum_perm]
intro i h_1_le_1 h_i_le_1
linarith
-- Case 2: where head + score < threshold
have h_simple_increment := (implementation_loop_simple_increment head tail threshold score coins).left
simp [h_simple_increment (by linarith)] at h_within_threshold
by_cases h_tail_len_0: tail.length ≤ 0
-- Case 2.1: where tail.length ≤ 0
rw [Nat.le_zero] at h_tail_len_0
have h_tail_nil := List.eq_nil_of_length_eq_zero h_tail_len_0
simp [h_tail_nil] at h_within_threshold
simp [implementation.loop] at h_within_threshold
-- Case 2.2: where tail.length > 0
have h_tail_len_gt_0: tail.length > 0 := by linarith
simp [h_tail_len_gt_0] at ih
specialize ih (head + score) coins
simp [h_within_threshold ] at ih
-- i₁
obtain ⟨i₁, i₁h⟩ := ih
-- h_1_le_i', h_i'_le_len, h_to_prove
use i₁ + 1
intro h_1_le_i'
intro h_score_head_ge_threshold
simp [h_simple_increment (by linarith)]
have h_perm_sum': score + (head + (List.take i₁ tail).sum) = head + score + (List.take i₁ tail).sum := by
  linarith
simp [h_perm_sum']
intro h_to_prove
simp at h_1_le_i'
by_cases h_1_le_i'_lt_i₁: 1 ≤ i₁
-- Case 3: where 1 ≤ i₁
simp [h_1_le_i'_lt_i₁] at i₁h
simp [h_1_le_i'] at i₁h
by_cases h_threshold_head_score_i₁: threshold ≤ head + score + (List.take i₁ tail).sum
-- Case 3.1: where threshold ≤ head + score + (List.take i₁ tail).sum
simp [h_threshold_head_score_i₁] at i₁h
simp [h_to_prove] at i₁h
intro i
intro h_1_le_i
intro h_i_lt_i₁_plus_1
-- Case 3.1.1: where i < i₁
set i' := i - 1
have h_1_le_i_plus_1: i = i' + 1 := by
  simp [i']
  rw [Nat.sub_add_cancel]
  linarith
simp [h_1_le_i_plus_1]
simp [h_1_le_i_plus_1] at h_i_lt_i₁_plus_1
by_cases h_1_le_i': 1 ≤ i'
have h_i₁_h := i₁h i' h_1_le_i' h_i_lt_i₁_plus_1
rw [←Int.add_assoc]
rw [Int.add_comm score]
assumption
simp at h_1_le_i'
simp [h_1_le_i']
linarith
simp at h_threshold_head_score_i₁
simp at h_score_head_ge_threshold
linarith
simp at h_1_le_i'_lt_i₁
intro i h_1_le_i h_i_lt_i₁_plus_1
simp [h_1_le_i'_lt_i₁] at h_i_lt_i₁_plus_1
linarith
[END LEMMAS]

[PROOF]
by
-- sometimes we have to create a temporary variable to use in the proof
unfold problem_spec
let result := implementation score_changes threshold
use result
simp [result]
simp [implementation]
intros h_rounds_played
have h_stop := implementation_loop_invariant_stop score_changes threshold 0 0 h_rounds_played
by_cases h_implementation_stop: implementation.loop score_changes threshold 0 0 = 0
-- Case 1: where implementation.loop score_changes threshold 0 0 = 0
simp [h_implementation_stop]
simp [h_implementation_stop] at h_stop
exact h_stop
-- Case 2: where implementation.loop score_changes threshold 0 0 ≠ 0
simp [h_implementation_stop]
have h_implementation_stop': 0 < implementation.loop score_changes threshold 0 0 := by
  by_contra
  rename_i h_implementation_stop_false
  simp at h_implementation_stop_false
  contradiction
have h_continue := implementation_loop_invariant_continue score_changes threshold 0 0 h_rounds_played h_implementation_stop'
simp at h_continue
obtain ⟨i₁⟩ := h_continue
rename_i h_continue_i₁
use i₁
intro h_1_le_i₁ h_iᵢ_score_len h_threshold
simp [h_1_le_i₁, h_iᵢ_score_len, h_threshold] at h_continue_i₁
by_cases h_drop_i₁: (List.drop i₁ score_changes).length > 0
have h_threshold' := implementation_loop_threshold_invariant (List.drop i₁ score_changes) threshold 0 0 (List.take i₁ score_changes).sum h_drop_i₁
simp at h_threshold'
simp [h_threshold']
intro h_drop_impl
simp [h_drop_impl] at h_continue_i₁
intro i''
intro h_i''_le_i₁
have h'' := h_continue_i₁ i''
by_cases h_1_le_i'': 1 ≤ i''
simp [h_1_le_i''] at h''
assumption
simp at h_1_le_i''
linarith
simp at h_drop_i₁
have h_i₁_eq_score_changes_len : i₁ = score_changes.length := by
  linarith
simp [h_i₁_eq_score_changes_len] at h_continue_i₁
simp [implementation.loop] at h_continue_i₁
simp [h_i₁_eq_score_changes_len]
simp [implementation.loop]
exact h_continue_i₁
[END]

`conv end`