`conv start`

`example_user`
[NL Description]
def find_magnitude(x: int) -> int
"""
Given an integer x, your task is to find the magnitude of x.
The magnitude of an integer is defined as the absolute value of the integer.
"""

[GROUND TRUTH SPECIFICATION]
def problem_spec
-- function signature
(impl: Int → Int)
-- inputs
(x: Int) :=
-- spec
let spec (result: Int) :=
(result ≥ 0) ∧
(impl (-x) = result) ∧
(result = 0 ↔ x = 0) ∧
(0 ≤ x → impl (-x) + result = 2 * x) ∧
(x ≤ 0 → impl (-x) + result = -2 * x)
-- program terminates
∃ result, impl x = result ∧
-- return value satisfies spec
spec result

[GENERATED SPECIFICATION]
def generated_spec
-- function signature
(impl: Int → Int)
-- inputs
(x: Int) : Prop :=
-- end_def generated_spec
--start_def generated_spec_body
impl x = if x < 0 then -x else x

[ISOMORPHISM STATEMENT]
theorem spec_isomorphism:
∀ impl,
(∀ x, problem_spec impl x) ↔
(∀ x, generated_spec impl x) :=


`example_assistant`
[THOUGHTS]
To prove the equivalence of the two specifications, we can start by analyzing the generated specification. 
The original specification doesn't reveal the implementation details, but we can see that the generated specification is a simple if-else statement that checks if x is less than 0.
We can use this information to write a proof that shows that the two specifications are equivalent.
The idea is to try different cases for x, and show that the properties of the generated specification hold true for the original specification as well.
[END THOUGHTS]


[PROOF]
by
unfold problem_spec
unfold generated_spec
simp
intro impl
apply Iff.intro
intro h_prob_spec
intro x
by_cases h_x_lt_0: x < 0
-- if x < 0 then
have h_x_le_0: x ≤ 0 := by
  linarith
simp [h_x_lt_0]
have h_impl := h_prob_spec x
simp [h_x_lt_0 ] at h_impl
have h_neg_impl := h_impl.2.2.2
simp [h_x_le_0] at h_neg_impl
linarith
simp [h_x_lt_0]
have h_impl := h_prob_spec x
simp at h_x_lt_0
simp [h_x_lt_0] at h_impl
have h_pos_impl := h_impl.2.2.2.1
linarith
intro h_generated_spec
intro x
by_cases h_x_lt_0: x < 0
-- if x < 0 then
have h_not_0_lt_x: ¬ (0 < x) := by
  linarith
have h_impl := h_generated_spec x
simp [h_x_lt_0] at h_impl
have h_0_le_impl_x: 0 ≤ impl x := by
  simp [h_impl]
  linarith
simp [h_0_le_impl_x]
have h_impl_neg_x := h_generated_spec (-x)
simp [h_x_lt_0] at h_impl_neg_x
simp [h_not_0_lt_x] at h_impl_neg_x
rw [←h_impl_neg_x] at h_impl
simp [h_impl]
apply And.intro
apply Iff.intro
intro h_impl_neg_x_eq_0
rw [h_impl_neg_x_eq_0] at h_impl_neg_x
linarith
intro h_x_eq_0
simp [h_x_eq_0]
simp [h_x_eq_0] at h_impl_neg_x
assumption
apply And.intro
intro h_0_leq_impl_x
linarith
intro h_x_le_0
simp [h_impl_neg_x]
linarith
have h_impl := h_generated_spec x
have h_0_le_x: 0 ≤ x := by
  linarith
simp [h_x_lt_0] at h_impl
have h_0_le_impl_x: 0 ≤ impl x := by
  simp [h_impl]
  linarith
simp [h_0_le_impl_x]
have h_impl_neg_x := h_generated_spec (-x)
simp [h_x_lt_0] at h_impl_neg_x
by_cases h_0_lt_x: 0 < x
simp [h_0_lt_x] at h_impl_neg_x
simp [h_impl_neg_x, h_impl]
apply And.intro
simp [h_0_le_x]
linarith
intro h_x_le_0
have h_x_eq_0: x = 0 := by
  linarith
simp [h_x_eq_0]
simp at h_0_lt_x
have h_x_eq_0: x = 0 := by
  linarith
simp [h_x_eq_0]
rw [h_x_eq_0] at h_impl
linarith
[END]

`example_user`
[NL Description]
def find_fibonacci(n: int) -> int
"""
Given an integer n, your task is to find the nth Fibonacci number.
The Fibonacci sequence is defined as follows:
- F(0) = 1
- F(1) = 1
- F(n) = F(n-1) + F(n-2) for n > 1
"""

[HELPER DEFINITIONS]
inductive fibonacci_non_computable : ℕ → ℕ → Prop
| base0 : fibonacci_non_computable 0 0
| base1 : fibonacci_non_computable 1 1
| step  : ∀ n f₁ f₂, fibonacci_non_computable n f₁ →
fibonacci_non_computable (n + 1) f₂ →
fibonacci_non_computable (n + 2) (f₁ + f₂)

[GROUND TRUTH SPECIFICATION]
def problem_spec
-- function signature
(impl: Nat → Nat)
-- inputs
(n: Nat) :=
-- spec
let spec (result: Nat) :=
fibonacci_non_computable n result
-- program terminates
∃ result, impl n = result ∧
-- return value satisfies spec
spec result

[GENERATED SPECIFICATION]
def generated_spec
-- function signature
(impl: Nat → Nat)
-- inputs
(n: Nat) : Prop :=
-- spec
let spec (result: Nat) :=
match n with
| 0 => result = 0
| 1 => result = 1
| n' + 2 => result = impl n' + impl (n' + 1)
-- return value satisfies spec
∃ result, impl n = result ∧
spec result

[ISOMORPHISM STATEMENT]
theorem spec_isomorphism:
∀ impl,
(∀ n, problem_spec impl n) ↔
(∀ n, generated_spec impl n) :=


`example_assistant`
[THOUGHTS]
The Fibonacci sequence is defined recursively, and the generated specification captures this recursive structure.
However, the inductive definition of `fibonacci_non_computable` is a non-computational definition, which means it does not provide a direct way to compute Fibonacci numbers. So we define multiple helper lemmas like `fib0_unique`, `fib1_unique`, and `fib_rec_unique` to help us prove the isomorphism. The `fib_inversion` lemma is used to show that if two Fibonacci numbers are equal, then their corresponding indices must also be equal. This is crucial for proving the uniqueness of Fibonacci numbers.
The proof uses the helper lemmas to show that the generated specification is equivalent to the problem specification. The proof is structured in a way that it first shows the implication from the problem specification to the generated specification and then vice versa. The use of `by_cases` allows us to handle different cases for the input `n`, which is essential for proving the equivalence of the two specifications. Notice the use of `Nat.strong_induction_on` to handle the recursive nature of the Fibonacci sequence. This is often necessary when recursive definitions uses more than one recursive call to compute the result.
[END THOUGHTS]


[HELPER LEMMAS]
-- start_def iso_helper_lemmas
theorem fib0_unique (n : ℕ) (h : fibonacci_non_computable 0 n) : n = 0 :=
-- end_def iso_helper_lemmas
-- start_def iso_helper_lemmas_proof
by
cases h
rfl
-- end_def iso_helper_lemmas_proof

-- start_def iso_helper_lemmas
theorem fib1_unique (n : ℕ) (h : fibonacci_non_computable 1 n) : n = 1 :=
-- end_def iso_helper_lemmas
-- start_def iso_helper_lemmas_proof
by
cases h
rfl
-- end_def iso_helper_lemmas_proof

-- start_def iso_helper_lemmas
theorem fib_rec_unique (n m : ℕ):
  fibonacci_non_computable (n + 2) m ↔
  ∃ f₁ f₂, fibonacci_non_computable n f₁ ∧
  fibonacci_non_computable (n + 1) f₂ ∧
  m = f₁ + f₂ :=
-- end_def iso_helper_lemmas
-- start_def iso_helper_lemmas_proof
by
apply Iff.intro
intro h
cases h
rename_i f₁ f₂ h₁ h₂
use f₁
use f₂
intro h
obtain ⟨f₁, f₂, h₁, h₂, h_eq⟩ := h
rw [h_eq]
exact fibonacci_non_computable.step _ _ _ h₁ h₂
-- end_def iso_helper_lemmas_proof

-- start_def iso_helper_lemmas
theorem fib_inversion (n f₁ f₂ : ℕ)
(h : fibonacci_non_computable n f₁) (h' : fibonacci_non_computable n f₂) :
  f₁ = f₂ :=
-- end_def iso_helper_lemmas
-- start_def iso_helper_lemmas_proof
by
revert f₁ f₂
induction' n using Nat.strong_induction_on with n' ih
intro f₁ f₂
by_cases h_n'_lt_1: n' < 2
intro h h'
-- if n' < 1 then
have h_n'_eq_0: n' = 0 ∨ n' = 1:= by
  interval_cases n'
  all_goals simp
cases h_n'_eq_0
rename_i h_n'_eq_0
simp [h_n'_eq_0] at *
cases h
cases h'
rfl
rename_i h_n'_eq_1
simp [h_n'_eq_1] at *
clear h_n'_eq_1
cases h
cases h'
rfl
set n'' := n' - 2
have h_n''_eq_n_plus_2: n' = n'' + 2 := by
  rw [Nat.sub_add_cancel]
  linarith
simp [h_n''_eq_n_plus_2] at *
clear h_n''_eq_n_plus_2 h_n'_lt_1
intro h h'
rw [fib_rec_unique] at h
obtain ⟨f₁', f₂', h₁, h₂, h_eq⟩ := h
rw [fib_rec_unique] at h'
obtain ⟨f₁'', f₂'', h₁', h₂', h_eq'⟩ := h'
have h_fib_inv_n'' := ih n'' (by linarith) f₁'' f₁' h₁' h₁
have h_fib_inv_n''_plus_1 := ih (n'' + 1) (by linarith) f₂'' f₂' h₂' h₂
linarith
-- end_def iso_helper_lemmas_proof
[END LEMMAS]

[PROOF]
by
unfold problem_spec
unfold generated_spec
intro impl
apply Iff.intro
intro h_prob_spec
intro n
have h_impl_n_eq_0 := h_prob_spec n
simp at h_impl_n_eq_0
simp
by_cases h_n_lt_1: n < 2
-- if n = 0 then
have h_n_eq_0_or_1: n = 0 ∨ n = 1 := by
  interval_cases n
  all_goals simp
cases h_n_eq_0_or_1
rename_i h_n_eq_0
simp [h_n_eq_0] at *
apply fib0_unique
assumption
rename_i h_n_eq_1
simp [h_n_eq_1] at *
apply fib1_unique
assumption
set n' := n - 2
have h_n'_eq_n_plus_2: n = n' + 2 := by
  rw [Nat.sub_add_cancel]
  linarith
simp [h_n'_eq_n_plus_2] at *
clear h_n'_eq_n_plus_2 h_n_lt_1
have h_fib_n' := h_prob_spec n'
have h_fib_n'_1 := h_prob_spec (n' + 1)
simp at h_fib_n'
simp at h_fib_n'_1
have h_fib_combination := fibonacci_non_computable.step _ _ _ h_fib_n' h_fib_n'_1
have h_fib_inv := fib_inversion (n' + 2) _ _ h_fib_combination h_impl_n_eq_0
linarith
intro h_generated_spec
simp
intro n
have h_impl_n': ∀ n, impl (n + 2) = impl n + impl (n + 1) := by
  intro n
  have h_impl_temp := h_generated_spec (n + 2)
  simp at h_impl_temp
  assumption
have h_impl_0 := h_generated_spec 0
have h_impl_1 := h_generated_spec 1
simp at h_impl_0
simp at h_impl_1
simp [(fib_rec_unique_seq n impl h_impl_0 h_impl_1 h_impl_n')]
[END]


`conv end`